make guard a parameter
adapt consistency

adapt safetemplatechecker

fix plugin in SafeChecker

WIP in erasure

Update reduction_test.v

adapt consistency after rebase

Revert "WIP in erasure"

This reverts commit 919b6446aa814625d16c9643aeac6159480cc8d2.

progress in erasurefunction

finish pass on erasureFunction

define abstract interface for erasure

adapt erasure

add fake guard correctness axiom when needed

erasure/theories/ETransform.v
@@ -19,15 +19,16 @@ Definition build_wf_env_from_env {cf : checker_flags} (Σ : global_env_map) (wf�
      wf_env_map_repr := Σ.(trans_env_repr);
  |}.
 
-Program Definition erase_pcuic_program (p : pcuic_program) 
+Program Definition erase_pcuic_program {guard : abstract_guard_impl} (p : pcuic_program) 
   (wfΣ : ∥ PCUICTyping.wf_ext (H := config.extraction_checker_flags) p.1 ∥)
   (wt : ∥ ∑ T, PCUICTyping.typing (H := config.extraction_checker_flags) p.1 [] p.2 T ∥) : eprogram_env :=
   let wfe := build_wf_env_from_env p.1.1 (map_squash (PCUICTyping.wf_ext_wf _) wfΣ) in
-  let wfext := ErasureFunction.make_wf_env_ext wfe p.1.2 wfΣ in
-  let t := ErasureFunction.erase wfext nil p.2
+  let wfext := optim_make_wf_env_ext (guard:=guard) wfe p.1.2 _ in
+  let t := ErasureFunction.erase (nor:=PCUICSN.extraction_normalizing) optimized_abstract_env_ext_impl wfext nil p.2
     (fun Σ wfΣ => let '(sq (T; ty)) := wt in PCUICTyping.iswelltyped ty) in
-  let Σ' := ErasureFunction.erase_global_fast (EAstUtils.term_global_deps t) wfe in
-  (EEnvMap.GlobalContextMap.make Σ' _, t).
+  let Σ' := ErasureFunction.erase_global_fast optimized_abstract_env_impl
+    (EAstUtils.term_global_deps t) wfe (p.1.(PCUICAst.PCUICEnvironment.declarations)) _ in
+    (EEnvMap.GlobalContextMap.make Σ' _, t).
 
 Next Obligation.
   eapply wf_glob_fresh.
@@ -38,17 +39,20 @@ Obligation Tactic := idtac.
 
 Import Extract.
   
-Definition erase_program (p : pcuic_program) (wtp : ∥ wt_pcuic_program (cf:=config.extraction_checker_flags) p ∥) : eprogram_env :=
-  erase_pcuic_program p (map_squash fst wtp) (map_squash snd wtp).
+Definition erase_program {guard : abstract_guard_impl} (p : pcuic_program) 
+  (wtp : ∥ wt_pcuic_program (cf:=config.extraction_checker_flags) p ∥) : eprogram_env :=
+  erase_pcuic_program (guard := guard) p (map_squash fst wtp) (map_squash snd wtp).
 
-Lemma expanded_erase_program (cf := config.extraction_checker_flags) p (wtp : ∥ wt_pcuic_program p ∥) :
+Lemma expanded_erase_program {guard : abstract_guard_impl} 
+  (cf := config.extraction_checker_flags) p (wtp : ∥ wt_pcuic_program p ∥) :
   PCUICEtaExpand.expanded_pcuic_program p ->
-  EEtaExpandedFix.expanded_eprogram_env (erase_program p wtp).
+  EEtaExpandedFix.expanded_eprogram_env (erase_program (guard:=guard) p wtp).
 Proof.
-  intros [etaenv etat]. split.
-  unfold erase_program, erase_pcuic_program.
-  eapply ErasureFunction.expanded_erase_global_fast, etaenv.
-  eapply ErasureFunction.expanded_erase_fast, etat.
+  intros [etaenv etat]. split;
+  unfold erase_program, erase_pcuic_program; cbn.
+  eapply ErasureFunction.expanded_erase_global_fast, etaenv; reflexivity.
+  eapply (ErasureFunction.expanded_erase_fast (X_type:=optimized_abstract_env_impl)).
+  reflexivity. eapply etat.
 Qed.
 
 Lemma expanded_eprogram_env_expanded_eprogram_cstrs p :
@@ -62,41 +66,43 @@ Proof.
   - eapply EEtaExpanded.isEtaExpFix_isEtaExp. now eapply EEtaExpandedFix.expanded_isEtaExp.
 Qed.
 
-Program Definition erase_transform : Transform.t pcuic_program eprogram_env PCUICAst.term EAst.term 
+Program Definition erase_transform {guard : abstract_guard_impl}  : Transform.t pcuic_program eprogram_env PCUICAst.term EAst.term 
   eval_pcuic_program (eval_eprogram_env EWcbvEval.default_wcbv_flags) :=
  {| name := "erasure";
     pre p :=  
       ∥ wt_pcuic_program (cf := config.extraction_checker_flags) p ∥ /\ PCUICEtaExpand.expanded_pcuic_program p ;
-    transform p hp := erase_program p (proj1 hp) ;
+    transform p hp := erase_program (guard:=guard) p (proj1 hp) ;
     post p := [/\ wf_eprogram_env all_env_flags p & EEtaExpandedFix.expanded_eprogram_env p];
     obseq g g' v v' := let Σ := g.1 in Σ ;;; [] |- v ⇝ℇ v' |}.
 Next Obligation.
   cbn -[erase_program].
-  intros p [wtp etap].
+  intros ? p [wtp etap].
   destruct erase_program eqn:e.
   split; cbn.
   - unfold erase_program, erase_pcuic_program in e. simpl. cbn in e. injection e. intros <- <-.
     split. 
     eapply ErasureFunction.erase_global_fast_wf_glob.
-    eapply ErasureFunction.erase_wellformed_fast.
+    eapply (ErasureFunction.erase_wellformed_fast (X_type:=optimized_abstract_env_impl)).
   - rewrite -e. cbn.
     now eapply expanded_erase_program.
 Qed.
 
 Next Obligation.
-  red. move=> [Σ t] v [[wf [T HT]]]. unfold eval_pcuic_program, eval_eprogram.
+  red. move=> guard [Σ t] v [[wf [T HT]]]. unfold eval_pcuic_program, eval_eprogram.
   intros [ev].
   destruct erase_program eqn:e.
   unfold erase_program, erase_pcuic_program in e. simpl in e. injection e; intros <- <-.
   simpl. clear e. cbn in *.
   set (Σ' := build_wf_env_from_env _ _).
-  eapply (ErasureFunction.erase_correct Σ' Σ.2 _ _ _ _ _ (EAstUtils.term_global_deps _)) in ev.
-  4:{ rewrite -ErasureFunction.erase_global_fast_spec. reflexivity. }
+  assert (ev' :forall Σ0 : PCUICAst.PCUICEnvironment.global_env, Σ0 = Σ' -> PCUICWcbvEval.eval Σ0 t v).
+  { intros; now subst. }
+  eapply (ErasureFunction.erase_correct optimized_abstract_env_impl Σ' Σ.2 _ _ _ _ _ (EAstUtils.term_global_deps _)) in ev'.
+  4:{ erewrite <- ErasureFunction.erase_global_deps_fast_spec. reflexivity. }
   all:trea.
   2:eapply Kernames.KernameSet.subset_spec; reflexivity.
-  destruct ev as [v' [he [hev]]]. exists v'; split => //.
+  destruct ev' as [v' [he [hev]]]. exists v'; split => //.
   red. cbn.
-  sq. eexact hev.
+  sq. exact hev. Unshelve. cbn; intros. now subst.
 Qed.
 
 (** This transformation is the identity on terms but changes the evaluation relation to one
