erasure/theories/ErasureFunction.v
@@ -15,7 +15,7 @@ From MetaCoq.PCUIC Require Import PCUICAst PCUICAstUtils PCUICPrimitive
   PCUICValidity PCUICPrincipality PCUICElimination 
   PCUICOnFreeVars PCUICWellScopedCumulativity PCUICSN PCUICEtaExpand.
      
-From MetaCoq.SafeChecker Require Import PCUICErrors PCUICWfEnv PCUICWfEnvImpl PCUICSafeReduce PCUICSafeRetyping.
+From MetaCoq.SafeChecker Require Import PCUICErrors PCUICWfEnv PCUICSafeReduce PCUICSafeRetyping.
 From MetaCoq.Erasure Require Import EAstUtils EArities Extract Prelim EDeps ErasureProperties ErasureCorrectness.
 
 Local Open Scope string_scope.
@@ -77,28 +77,30 @@ Section OnInductives.
 End OnInductives.
 
 Local Existing Instance extraction_checker_flags.
-Definition wf_ext_wf Σ : wf_ext Σ -> wf Σ := fst.
+(* Definition wf_ext_wf Σ : wf_ext Σ -> wf Σ := fst.
 #[global]
-Hint Resolve wf_ext_wf : core.
+Hint Resolve wf_ext_wf : core. *)
 
 Ltac specialize_Σ wfΣ :=
   repeat match goal with | h : _ |- _ => specialize (h _ wfΣ) end. 
 
 Section fix_sigma.
-  Variable Σ : wf_env_ext.
 
-  Local Definition HΣ : ∥ wf Σ ∥.
-  Proof.
-    exact (map_squash (wf_ext_wf _) Σ).
-  Qed.
+  Context {cf : checker_flags} {nor : normalizing_flags}.
+  Context (X_type : abstract_env_ext_impl).
+  Context (X : X_type.π1).
+  
+  Local Definition heΣ Σ (wfΣ : abstract_env_ext_rel X Σ) : 
+    ∥ wf_ext Σ ∥ :=  abstract_env_ext_wf _ wfΣ.
+  Local Definition HΣ Σ (wfΣ : abstract_env_ext_rel X Σ) :
+    ∥ wf Σ ∥ := abstract_env_ext_sq_wf _ _ _ wfΣ. 
 
-  Definition abstract_env_rel' := @abstract_env_ext_rel _ _ optimized_abstract_env_ext_struct.
-
-  Definition term_rel : Relation_Definitions.relation (∑ Γ t, forall Σ0 : global_env_ext, abstract_env_rel' Σ Σ0 -> welltyped Σ0 Γ t) :=
+  Definition term_rel : Relation_Definitions.relation 
+    (∑ Γ t, forall Σ : global_env_ext, abstract_env_ext_rel X Σ -> welltyped Σ Γ t) :=
     fun '(Γ2; B; H) '(Γ1; t1; H2) =>
-    forall Σ0 : global_env_ext, abstract_env_rel' Σ Σ0 -> 
-      ∥∑ na A, red Σ0 Γ1 t1 (tProd na A B) × (Γ1,, vass na A) = Γ2∥.
-
+  forall Σ : global_env_ext, abstract_env_ext_rel X Σ -> 
+    ∥∑ na A, red Σ Γ1 t1 (tProd na A B) × (Γ1,, vass na A) = Γ2∥.
+  
   Definition cod B t := match t with tProd _ _ B' => B = B' | _ => False end.
 
   Lemma wf_cod : WellFounded cod.
@@ -111,7 +113,7 @@ Section fix_sigma.
     eapply Subterm.WellFounded_trans_clos. exact wf_cod.
   Defined.
 
-  Lemma Acc_no_loop X (R : X -> X -> Prop) t : Acc R t -> R t t -> False.
+  Lemma Acc_no_loop A (R : A -> A -> Prop) t : Acc R t -> R t t -> False.
   Proof.
     induction 1. intros. eapply H0; eauto.
   Qed.
@@ -124,7 +126,7 @@ Section fix_sigma.
   Definition wf_reduction_aux : WellFounded term_rel.
   Proof.
     intros (Γ & s & H). sq'.
-    assert (wfΣ' : abstract_env_rel' Σ Σ) by reflexivity.
+    destruct (abstract_env_ext_exists X) as [[Σ wfΣ']]. 
     pose proof (abstract_env_ext_wf _ wfΣ') as wf. sq. 
     set (H' := H _ wfΣ'). 
     induction (normalisation Σ _ Γ s H') as [s _ IH]. cbn in IH.
@@ -144,19 +146,25 @@ Section fix_sigma.
         * eapply red_neq_cored.
           eapply Relation_Properties.clos_rtn1_rt. exact r.
           intros ?. subst.
-          eapply Relation_Properties.clos_rtn1_rt in X0.
-          eapply cored_red_trans in X; [| exact X0 ].
-          eapply Acc_no_loop in X. eauto.
+          eapply Relation_Properties.clos_rtn1_rt in X1.
+          eapply cored_red_trans in X0; [| exact X1 ].
+          eapply Acc_no_loop in X0. eauto.
           eapply @normalisation; eauto.
         * constructor. do 2 eexists. now split.
   Unshelve.
-  - intros. cbn in H2; subst. destruct H' as [].
-    eapply inversion_Prod in X as (? & ? & ? & ? & ?) ; auto.
+  - intros. destruct H' as [].
+    rewrite <- (abstract_env_ext_irr _ H2) in X0; eauto.  
+    rewrite <- (abstract_env_ext_irr _ H2) in wf; eauto.  
+    eapply inversion_Prod in X0 as (? & ? & ? & ? & ?) ; auto.
     eapply cored_red in H0 as [].
     econstructor. econstructor. econstructor. eauto.
     2:reflexivity. econstructor; pcuic. 
+    rewrite <- (abstract_env_ext_irr _ H2) in X0; eauto.  
     eapply subject_reduction; eauto.
-  - intros. cbn in H0; subst.  eapply red_welltyped; sq.
+  - intros. rewrite <- (abstract_env_ext_irr _ H0) in wf; eauto.  
+    rewrite <- (abstract_env_ext_irr _ H0) in X0; eauto.  
+    rewrite <- (abstract_env_ext_irr _ H0) in r; eauto.  
+    eapply red_welltyped; sq.
     3:eapply Relation_Properties.clos_rtn1_rt in r; eassumption. 
     all:eauto.
   Defined.
@@ -170,13 +178,14 @@ Section fix_sigma.
   Opaque wf_reduction.
   
   #[tactic="idtac"]
-  Equations? is_arity Γ (HΓ : forall Σ0 : global_env_ext, abstract_env_rel' Σ Σ0 -> ∥wf_local Σ0 Γ∥) T (HT : forall Σ0 : global_env_ext, abstract_env_rel' Σ Σ0 -> welltyped Σ0 Γ T) : bool
-    by wf ((Γ;T;HT) : (∑ Γ t, forall Σ0 : global_env_ext, abstract_env_rel' Σ Σ0 -> welltyped Σ0 Γ t)) term_rel :=
+  Equations? is_arity Γ (HΓ : forall Σ : global_env_ext, abstract_env_ext_rel X Σ -> ∥wf_local Σ Γ∥) T 
+    (HT : forall Σ : global_env_ext, abstract_env_ext_rel X Σ -> welltyped Σ Γ T) : bool
+    by wf ((Γ;T;HT) : (∑ Γ t, forall Σ : global_env_ext, abstract_env_ext_rel X Σ -> welltyped Σ Γ t)) term_rel := 
       {
-        is_arity Γ HΓ T HT with inspect (@reduce_to_sort _ _ optimized_abstract_env_ext_impl Σ Γ T HT) => {
+        is_arity Γ HΓ T HT with inspect (@reduce_to_sort _ _ X_type X Γ T HT) => {
         | exist (Checked_comp H) rsort => true ;
         | exist (TypeError_comp _) rsort with 
-            inspect (reduce_to_prod (X_type:=optimized_abstract_env_ext_impl) (X:=Σ) Γ T HT) => {
+            inspect (@reduce_to_prod _ _ X_type X Γ T HT) => {
           | exist (Checked_comp (na; A; B; H)) rprod := is_arity (Γ,, vass na A) _ B _
           | exist (TypeError_comp e) rprod => false } }
       }.
@@ -202,7 +211,7 @@ Section fix_sigma.
     - cbn. clear rsort is_arity rprod.
       intros Σ' wfΣ'; specialize (H Σ' wfΣ').
       pose proof (abstract_env_ext_wf _ wfΣ') as [wf].
-      repeat specialize_Σ wfΣ'. subst Σ'. 
+      repeat specialize_Σ wfΣ'. 
       destruct HT as [s HT].
       sq.
       eapply subject_reduction_closed in HT; tea. 2:pcuic.
@@ -211,40 +220,50 @@ Section fix_sigma.
       eapply H.
   Defined.
   
-  Lemma is_arityP Γ (HΓ : forall Σ0 : global_env_ext, abstract_env_rel' Σ Σ0 -> ∥wf_local Σ0 Γ∥) T (HT : forall Σ0 : global_env_ext, abstract_env_rel' Σ Σ0 -> welltyped Σ0 Γ T) :
-    reflect (Is_conv_to_Arity Σ Γ T) (is_arity Γ HΓ T HT).
+  Lemma is_arityP Γ (HΓ : forall Σ : global_env_ext, abstract_env_ext_rel X Σ -> ∥wf_local Σ Γ∥) T 
+    (HT : forall Σ : global_env_ext, abstract_env_ext_rel X Σ -> welltyped Σ Γ T) :
+    reflect (forall Σ : global_env_ext, abstract_env_ext_rel X Σ -> 
+              Is_conv_to_Arity Σ Γ T) (is_arity Γ HΓ T HT).
   Proof.
     funelim (is_arity Γ HΓ T HT).
     - constructor.
-      destruct H as [s Hs].
-      clear H0 rsort. specialize (Hs _ eq_refl) as [Hs].
-      exists (tSort s) ; split => //.
-    - clear H0 H1. destruct X; constructor; clear rprod rsort;
-      specialize (H _ eq_refl) as [Hp].
+      destruct H as [s Hs]. clear H0 rsort. 
+      pose proof (abstract_env_ext_exists X) as [[Σ wfΣ]].
+      specialize (Hs _ wfΣ) as [Hs]. 
+      intros. rewrite (abstract_env_ext_irr _ H wfΣ).
+      exists (tSort s); split => //.
+    - clear H0 H1. 
+      destruct X0; constructor; clear rprod rsort.
       * red.
+        pose proof (abstract_env_ext_exists X) as [[Σ wfΣ]].
+        specialize_Σ wfΣ. sq.
+        intros. rewrite (abstract_env_ext_irr _ H0 wfΣ).
         destruct i as [T' [[HT'] isa]].
         exists (tProd na A T'); split => //. split.
         etransitivity; tea. now eapply closed_red_prod_codom.
-      * intros [T' [[HT'] isa]].
-        assert (wfΣ' : abstract_env_rel' Σ Σ) by reflexivity.
-        pose proof (abstract_env_ext_wf _ wfΣ') as [wf].
-        destruct (PCUICContextConversion.closed_red_confluence Hp HT') as (? & ? & ?); eauto.
+      * pose proof (abstract_env_ext_exists X) as [[Σ wfΣ]].
+        pose proof (abstract_env_ext_wf X wfΣ) as [wfΣ'].
+        specialize_Σ wfΣ. sq. 
+        intros [T' [[HT'] isa]]; eauto.
+        destruct (PCUICContextConversion.closed_red_confluence H HT') as (? & ? & ?); eauto.
         eapply invert_red_prod in c as (? & ? & []); eauto. subst.
-        apply n. red. exists x1.
+        apply n. intros. rewrite (abstract_env_ext_irr _ H0 wfΣ).
+        red. exists x1.
         split => //.
         eapply isArity_red in isa. 2:exact c0.
         now cbn in isa.
     - constructor.
-      clear H H0.
+      clear H H0. pose proof (abstract_env_ext_exists X) as [[Σ wfΣ]].
+      pose proof (abstract_env_ext_wf X wfΣ) as [wfΣ'].      
       symmetry in rprod. symmetry in rsort.
-      assert (wfΣ' : abstract_env_rel' Σ Σ) by reflexivity.
-      pose proof (abstract_env_ext_wf _ wfΣ') as [wf].
-      specialize_Σ wfΣ'.
-      intros isc. eapply Is_conv_to_Arity_inv in isc as [].
+      intros isc. specialize_Σ wfΣ.
+      eapply Is_conv_to_Arity_inv in isc as [].
       * destruct H as [na [A [B [Hr]]]].
-        apply e. exists na, A, B. intros. cbn in wfΣ. subst Σ0. now sq.
+        apply e. exists na, A, B. 
+        intros ? H. now rewrite (abstract_env_ext_irr _ H wfΣ).
       * destruct H as [u [Hu]].
-        apply a0. exists u. intros. cbn in wfΣ. subst Σ0. now sq.
+        apply a0. exists u. 
+        intros ? H. now rewrite (abstract_env_ext_irr _ H wfΣ).
   Qed.
   
 End fix_sigma.
@@ -306,87 +325,87 @@ Equations inspect_bool (b : bool) : { b } + { ~~ b } :=
   inspect_bool false := right eq_refl.
 
 #[tactic="idtac"]
-Equations? is_erasableb (Σ : wf_env_ext) (Γ : context) (T : PCUICAst.term) 
-  (wt : forall Σ0 : global_env_ext, abstract_env_rel' Σ Σ0 -> welltyped Σ0 Γ T) : bool :=
-  is_erasableb Σ Γ t wt with @type_of_typing extraction_checker_flags _ optimized_abstract_env_ext_impl Σ Γ t wt :=
-    { | T with is_arity Σ Γ _ T.π1 _ := 
+Equations? is_erasableb X_type X (Γ : context) (T : PCUICAst.term) 
+  (wt : forall Σ : global_env_ext, abstract_env_ext_rel X Σ -> welltyped Σ Γ T) : bool :=
+  is_erasableb X_type X Γ t wt with @type_of_typing extraction_checker_flags _ X_type X Γ t wt :=
+    { | T with is_arity X_type X Γ _ T.π1 _ := 
       { | true => true
-        | false => let s := @sort_of_type extraction_checker_flags _ optimized_abstract_env_ext_impl Σ Γ T.π1 _ in
+        | false => let s := @sort_of_type extraction_checker_flags _ X_type X Γ T.π1 _ in
           is_propositional s.π1 } }.
   Proof.
-    - intros.
-      destruct (wt _ H); sq; eauto.
-      cbn in H. subst Σ0. pcuic.
-    - intros. destruct T as [T Ht].
-      cbn. specialize (Ht Σ0 H) as [[tT Hp]].
-      assert (wfΣ' : abstract_env_rel' Σ Σ) by reflexivity.
-      pose proof (abstract_env_ext_wf _ wfΣ') as [wf].
-      cbn in H; subst Σ0.
+    - intros. specialize_Σ H. destruct wt; sq. 
+      pcuic.
+    - intros. specialize_Σ H. destruct T as [T Ht].
+      cbn. destruct (Ht Σ H) as [[tT Hp]].
+      pose proof (abstract_env_ext_wf X H) as [wf].
       eapply validity in tT. pcuic.
     - intros. destruct T as [T Ht].
-      cbn in *. specialize (Ht Σ0 H) as [[tT Hp]].
-      assert (wfΣ' : abstract_env_rel' Σ Σ) by reflexivity.
-      pose proof (abstract_env_ext_wf _ wfΣ') as [wf].
-      cbn in H; subst Σ0.
+      cbn in *. specialize (Ht Σ H) as [[tT Hp]].
+      pose proof (abstract_env_ext_wf X H) as [wf].
       eapply validity in tT. now sq.
   Qed.
 Transparent is_arity type_of_typing.
 
-Lemma is_erasableP {Σ : wf_env_ext} {Γ : context} {t : PCUICAst.term}
-  {wt : forall Σ0 : global_env_ext, abstract_env_rel' Σ Σ0 -> welltyped Σ0 Γ t} : 
-  reflect (∥ isErasable Σ Γ t ∥) (is_erasableb Σ Γ t wt).
+Lemma is_erasableP {X_type X} {Γ : context} {t : PCUICAst.term}
+  {wt : forall Σ : global_env_ext, abstract_env_ext_rel X Σ -> welltyped Σ Γ t} : 
+  reflect (forall Σ : global_env_ext, abstract_env_ext_rel X Σ -> 
+           ∥ isErasable Σ Γ t ∥) (is_erasableb X_type X Γ t wt).
 Proof.
-  funelim (is_erasableb Σ Γ t wt).
-  - constructor. destruct type_of_typing as [x Hx]. cbn -[is_arity sort_of_type] in *.  
-    assert (wfΣ' : abstract_env_rel' Σ Σ) by reflexivity.
-    pose proof (abstract_env_ext_wf _ wfΣ') as [wf].
-    specialize_Σ wfΣ'. destruct (Hx _ eq_refl) as [[HT ?]]. 
-    move/is_arityP: Heq => [T' [redT' isar]].
-    destruct (wt _ eq_refl) as [T ht].
-    sq. red. exists T'. eapply type_reduction_closed in HT; eauto.
+  funelim (is_erasableb X_type X Γ t wt).
+  - constructor. intros. pose proof (abstract_env_ext_wf _ H) as [wf].
+    destruct type_of_typing as [x Hx]. cbn -[is_arity sort_of_type] in *.  
+    destruct (Hx _ H) as [[HT ?]]. 
+    move/is_arityP: Heq => / (_ _ H) [T' [redT' isar]]. specialize_Σ H. 
+    sq. red. exists T'. eapply type_reduction_closed in HT.
+    2: eassumption. eauto.  
   - destruct type_of_typing as [x Hx]. cbn -[sort_of_type is_arity] in *.  
-    assert (wfΣ' : abstract_env_rel' Σ Σ) by reflexivity.
     destruct (sort_of_type _ _ _ _). cbn.
-    specialize_Σ wfΣ'.
     destruct (is_propositional x0) eqn:isp; constructor.
-    * clear Heq. pose proof (abstract_env_ext_wf _ wfΣ') as [wf]. 
-      specialize_Σ wfΣ'. 
+    * clear Heq. intros. 
+      pose proof (abstract_env_ext_wf _ H) as [wf]. 
+      specialize_Σ H. 
       destruct Hx as [[HT ?]].
       destruct s as [Hs]. sq.
       exists x; split => //. right.
       exists x0. now split.
-    * intros [[T' [HT' er]]].
-      pose proof (abstract_env_ext_wf _ wfΣ') as [wf].
+    * pose proof (abstract_env_ext_exists X) as [[Σ wfΣ]].
+      move => / (_ _ wfΣ) [[T' [HT' er]]].
+      pose proof (abstract_env_ext_wf _ wfΣ) as [wf].
       move/is_arityP: Heq => nisa. 
-      specialize_Σ wfΣ'. 
+      specialize_Σ wfΣ. 
       destruct Hx as [[HT ?]].
       specialize (p _ HT').
       destruct er as [isa|[u' [Hu' isp']]].
-      { apply nisa. eapply invert_cumul_arity_r; tea. }
-      { destruct s as [Hs]. unshelve epose proof (H := unique_sorting_equality_propositional _ _ wf Hs Hu' p) => //. reflexivity. reflexivity. congruence. }
-Qed.
-    
-Equations? is_erasable (Σ : wf_env_ext) (Γ : context) (t : PCUICAst.term) 
-  (wt : forall Σ0 : global_env_ext, abstract_env_rel' Σ Σ0 -> welltyped Σ0 Γ t) : 
-  { ∥ isErasable Σ Γ t ∥ } + { ∥ isErasable Σ Γ t -> False ∥ } :=
-  is_erasable Σ Γ T wt with inspect_bool (is_erasableb Σ Γ T wt) :=
+      { apply nisa. intros. rewrite (abstract_env_ext_irr _ H wfΣ). 
+        eapply invert_cumul_arity_r; tea. }
+      { destruct s as [Hs].
+        unshelve epose proof (H := unique_sorting_equality_propositional _ _ wf Hs Hu' p) => //. reflexivity. reflexivity. congruence. }
+  Qed.
+
+Equations? is_erasable {X_type X} (Γ : context) (t : PCUICAst.term) 
+  (wt : forall Σ : global_env_ext, abstract_env_ext_rel X Σ -> welltyped Σ Γ t) : 
+  forall Σ : global_env_ext, abstract_env_ext_rel X Σ -> 
+    { ∥ isErasable Σ Γ t ∥ } + { ∥ isErasable Σ Γ t -> False ∥ } :=
+  is_erasable Γ T wt Σ wfΣ with inspect_bool (is_erasableb X_type X Γ T wt) :=
     { | left ise => left _
       | right nise => right _ }.
 Proof.
-  assert (wfΣ' : abstract_env_rel' Σ Σ) by reflexivity.
-  pose proof (abstract_env_ext_wf _ wfΣ') as [wf].
-  move/is_erasableP: ise => //.
+  pose proof (abstract_env_ext_wf _ wfΣ) as [wf].
+  now move/is_erasableP: ise => //.
   move/(elimN is_erasableP): nise.
-  intros; sq => ise. apply nise. now sq.
+  intros; sq => ise. apply nise. 
+  intros. now rewrite (abstract_env_ext_irr _ H wfΣ).
 Qed.
 
 Section Erase.
-  Variable (Σ : wf_env_ext).
+  Context {nor : normalizing_flags}.
+  Context (X_type : abstract_env_ext_impl (cf := extraction_checker_flags)).
+  Context (X : X_type.π1).
 
-  Ltac sq' := 
+  (* Ltac sq' := 
              repeat match goal with
                     | H : ∥ _ ∥ |- _ => destruct H; try clear H
-                    end; try eapply sq.
+                    end; try eapply sq. *)
 
   (* Bug in equationa: it produces huge goals leading to stack overflow if we
     don't try reflexivity here. *)
@@ -406,9 +425,9 @@ Section Erase.
   
   #[tactic="idtac"]
   Equations? erase (Γ : context) (t : term) 
-    (Ht : forall Σ0 : global_env_ext, abstract_env_rel' Σ Σ0 -> welltyped Σ0 Γ t) : E.term
+    (Ht : forall Σ : global_env_ext, abstract_env_ext_rel X Σ -> welltyped Σ Γ t) : E.term
       by struct t :=
-  { erase Γ t Ht with inspect_bool (is_erasableb Σ Γ t Ht) :=
+  { erase Γ t Ht with inspect_bool (is_erasableb X_type X Γ t Ht) :=
   { | left he := E.tBox; 
     | right he with t := {
       | tRel i := E.tRel i
@@ -446,7 +465,7 @@ Section Erase.
         E.tCoFix mfix' n }
       (* erase Γ (tPrim p) Ht _ := E.tPrim (erase_prim p) *)
     } } 
-  where erase_terms (Γ : context) (l : list term) (Hl : forall Σ0 : global_env_ext, abstract_env_rel' Σ Σ0 -> ∥ All (welltyped Σ0 Γ) l ∥) : list E.term :=
+  where erase_terms (Γ : context) (l : list term) (Hl : forall Σ : global_env_ext, abstract_env_ext_rel X Σ -> ∥ All (welltyped Σ Γ) l ∥) : list E.term :=
   { erase_terms Γ [] _ := [];
     erase_terms Γ (t :: ts) _ := 
       let t' := erase Γ t _ in
@@ -456,8 +475,8 @@ Section Erase.
   In particular, note that #|br.(bcontext)| = context_assumptions br.(bcontext) when no lets are present.
   *)
   where erase_brs (Γ : context) p (brs : list (branch term)) 
-    (Ht : forall Σ0 : global_env_ext, abstract_env_rel' Σ Σ0 ->
-          ∥ All (fun br => welltyped Σ0 (Γ ,,, inst_case_branch_context p br) (bbody br)) brs ∥) :
+    (Ht : forall Σ : global_env_ext, abstract_env_ext_rel X Σ ->
+          ∥ All (fun br => welltyped Σ (Γ ,,, inst_case_branch_context p br) (bbody br)) brs ∥) :
     list (list name × E.term) := 
   { erase_brs Γ p [] Ht := [];
     erase_brs Γ p (br :: brs) Hbrs := 
@@ -466,8 +485,8 @@ Section Erase.
       (erase_context br.(bcontext), br') :: brs' }
   
   where erase_fix (Γ : context) (mfix : mfixpoint term)
-    (Ht : forall Σ0 : global_env_ext, abstract_env_rel' Σ Σ0 ->
-          ∥ All (fun d => isLambda d.(dbody) /\ welltyped Σ0 Γ d.(dbody)) mfix ∥) : E.mfixpoint E.term :=
+    (Ht : forall Σ : global_env_ext, abstract_env_ext_rel X Σ ->
+          ∥ All (fun d => isLambda d.(dbody) /\ welltyped Σ Γ d.(dbody)) mfix ∥) : E.mfixpoint E.term :=
   { erase_fix Γ [] _ := [];
     erase_fix Γ (d :: mfix) Hmfix := 
       let dbody' := erase Γ d.(dbody) _ in
@@ -482,8 +501,8 @@ Section Erase.
       d' :: erase_fix Γ mfix _ }
 
   where erase_cofix (Γ : context) (mfix : mfixpoint term)
-      (Ht : forall Σ0 : global_env_ext, abstract_env_rel' Σ Σ0 ->
-            ∥ All (fun d => welltyped Σ0 Γ d.(dbody)) mfix ∥) : E.mfixpoint E.term :=
+      (Ht : forall Σ : global_env_ext, abstract_env_ext_rel X Σ ->
+            ∥ All (fun d => welltyped Σ Γ d.(dbody)) mfix ∥) : E.mfixpoint E.term :=
     { erase_cofix Γ [] _ := [];
       erase_cofix Γ (d :: mfix) Hmfix := 
         let dbody' := erase Γ d.(dbody) _ in
@@ -496,9 +515,8 @@ Section Erase.
       try clear brs'; try clear c'; try clear br'; 
       try clear d' dbody'; try clear erase; try clear erase_terms; try clear erase_brs; try clear erase_mfix.
     all: cbn; intros; subst; lazymatch goal with [ |- False ] => idtac | _ => try clear he end.
-    all: assert (wfΣ' : abstract_env_rel' Σ Σ) by reflexivity;
-         pose proof (abstract_env_ext_wf _ wfΣ') as [wf];
-         specialize_Σ wfΣ'.
+    all: try pose proof (abstract_env_ext_wf _ H) as [wf];
+         specialize_Σ H.
     all: try destruct Ht as [ty Ht]; try destruct s0; simpl in *.
     - now eapply inversion_Evar in Ht.
     - discriminate.
@@ -514,8 +532,9 @@ Section Erase.
       eexists; eauto.
     - eapply inversion_App in Ht as (? & ? & ? & ? & ? & ?); auto.
       eexists; eauto.
-    - move/is_erasableP: he.
-      specialize_Σ wfΣ'. destruct Ht as [ty Ht]. intros ne. sq. apply ne. sq.
+    - move/is_erasableP: he. intro. apply he. intros.   
+      pose proof (abstract_env_ext_wf _ H) as [wf].
+      specialize_Σ H. destruct Ht as [ty Ht]. sq. 
       eapply inversion_Ind in Ht as (? & ? & ? & ? & ? & ?) ; auto.
       red. eexists. split. econstructor; eauto. left.
       eapply isArity_subst_instance.
@@ -535,55 +554,55 @@ Section Erase.
     - sq. now depelim Hbrs.
     - sq. now depelim Hbrs.
     - sq. now depelim Hmfix.
-    - clear dbody'0. specialize (Hmfix _ wfΣ'). sq. now depelim Hmfix.
+    - clear dbody'0. specialize_Σ H. sq. now depelim Hmfix.
     - sq. now depelim Hmfix.
     - sq. now depelim Hmfix.
   Qed.
   
 End Erase.
 
-Lemma is_erasableb_irrel {Σ Γ t} wt wt' : is_erasableb Σ Γ t wt = is_erasableb Σ Γ t wt'.
+Lemma is_erasableb_irrel {X_type X Γ t} wt wt' : is_erasableb X_type X Γ t wt = is_erasableb X_type X Γ t wt'.
 Proof.
-  destruct (@is_erasableP Σ Γ t wt);
-  destruct (@is_erasableP Σ Γ t wt') => //.
+  destruct (@is_erasableP X_type X Γ t wt);
+  destruct (@is_erasableP X_type X Γ t wt') => //.
 Qed.
 
 Ltac iserasableb_irrel :=
   match goal with
-  [ H : context [is_erasableb ?Σ ?Γ ?t ?wt], Heq : inspect_bool _ = _ |- context [ is_erasableb _ _ _ ?wt'] ] => 
+  [ H : context [is_erasableb ?X_type ?X ?Γ ?t ?wt], Heq : inspect_bool _ = _ |- context [ is_erasableb _ _ _ _ ?wt'] ] => 
     generalize dependent H; rewrite (is_erasableb_irrel wt wt'); intros; rewrite Heq
   end.
 
 Ltac simp_erase := simp erase; rewrite -?erase_equation_1.
 
-Lemma erase_irrel (Σ : wf_env_ext) : 
-  (forall Γ t wt, forall wt', erase Σ Γ t wt = erase Σ Γ t wt') ×
-  (forall Γ l wt, forall wt', erase_terms Σ Γ l wt = erase_terms Σ Γ l wt') ×
-  (forall Γ p l wt, forall wt', erase_brs Σ Γ p l wt = erase_brs Σ Γ p l wt') ×
-  (forall Γ l wt, forall wt', erase_fix Σ Γ l wt = erase_fix Σ Γ l wt') ×
-  (forall Γ l wt, forall wt', erase_cofix Σ Γ l wt = erase_cofix Σ Γ l wt').
+Lemma erase_irrel X_type X : 
+  (forall Γ t wt, forall wt', erase X_type X Γ t wt = erase X_type X Γ t wt') ×
+  (forall Γ l wt, forall wt', erase_terms X_type X Γ l wt = erase_terms X_type X Γ l wt') ×
+  (forall Γ p l wt, forall wt', erase_brs X_type X Γ p l wt = erase_brs X_type X Γ p l wt') ×
+  (forall Γ l wt, forall wt', erase_fix X_type X Γ l wt = erase_fix X_type X Γ l wt') ×
+  (forall Γ l wt, forall wt', erase_cofix X_type X Γ l wt = erase_cofix X_type X Γ l wt').
 Proof.
-  apply: (erase_elim Σ
+  apply: (erase_elim X_type X
     (fun Γ t wt e => 
-      forall wt' : forall Σ0 : global_env_ext, abstract_env_rel' Σ Σ0 ->  welltyped Σ0 Γ t, e = erase Σ Γ t wt')
-    (fun Γ l awt e => forall wt', e = erase_terms Σ Γ l wt')
-    (fun Γ p l awt e => forall wt', e = erase_brs Σ Γ p l wt')
-    (fun Γ l awt e => forall wt', e = erase_fix Σ Γ l wt')
-    (fun Γ l awt e => forall wt', e = erase_cofix Σ Γ l wt')); clear.
+      forall wt' : forall Σ : global_env_ext, abstract_env_ext_rel X Σ ->  welltyped Σ Γ t, e = erase X_type X Γ t wt')
+    (fun Γ l awt e => forall wt', e = erase_terms X_type X Γ l wt')
+    (fun Γ p l awt e => forall wt', e = erase_brs X_type X Γ p l wt')
+    (fun Γ l awt e => forall wt', e = erase_fix X_type X Γ l wt')
+    (fun Γ l awt e => forall wt', e = erase_cofix X_type X Γ l wt')); clear.
   all:intros *; intros; simp_erase.
   all:try simp erase; try iserasableb_irrel; simp_erase => //.
   all:try clear he Heq.
   all:try bang.
   all:try solve [cbn; f_equal; eauto].
   all:try solve [cbn; repeat (f_equal; eauto)].
-  cbn. f_equal. f_equal. now rewrite (H (erase_obligation_19 Σ Γ d mfix wt')).
-  now rewrite (H0 (erase_obligation_20 Σ Γ d mfix wt')).
+  cbn. f_equal. f_equal. now rewrite (H (erase_obligation_19 X_type X Γ d mfix wt')).
+  now rewrite (H0 (erase_obligation_20 X_type X Γ d mfix wt')).
 Qed.
 
-Lemma erase_terms_eq Σ Γ ts wt : 
-  erase_terms Σ Γ ts wt = map_All (erase Σ Γ) ts wt.
+Lemma erase_terms_eq X_type X Γ ts wt : 
+  erase_terms X_type X Γ ts wt = map_All (erase X_type X Γ) ts wt.
 Proof.
-  funelim (map_All (erase Σ Γ) ts wt); cbn; auto.
+  funelim (map_All (erase X_type X Γ) ts wt); cbn; auto.
   f_equal => //. apply erase_irrel.
   rewrite -H. eapply erase_irrel.
 Qed.
@@ -593,14 +612,15 @@ Opaque wf_reduction.
 #[global]
 Hint Constructors typing erases : core.
 
-Lemma erase_to_box {Σ : wf_env_ext} {Γ t} (wt : forall Σ0 : global_env_ext, abstract_env_rel' Σ Σ0 -> welltyped Σ0 Γ t) :
-  let et := erase Σ Γ t wt in 
+Lemma erase_to_box {X_type X} {Γ t} (wt : forall Σ : global_env_ext, abstract_env_ext_rel X Σ -> welltyped Σ Γ t) :
+  forall Σ : global_env_ext, abstract_env_ext_rel X Σ -> 
+  let et := erase X_type X Γ t wt in 
   if is_box et then ∥ isErasable Σ Γ t ∥
   else ~ ∥ isErasable Σ Γ t ∥.
 Proof.
-  cbn.
+  cbn. intros. 
   revert Γ t wt.
-  apply (erase_elim Σ
+  apply (erase_elim X_type X
     (fun Γ t wt e => 
       if is_box e then ∥ isErasable Σ Γ t ∥ else ∥ isErasable Σ Γ t ∥ -> False)
     (fun Γ l awt e => True)
@@ -610,29 +630,30 @@ Proof.
 
   all:try discriminate; auto.
   all:cbn -[isErasable].
-  all:try solve [match goal with 
-    [ H : context [ is_erasableb ?Σ ?Γ ?t ?Ht ] |- _ ] => 
-      destruct (@is_erasableP Σ Γ t Ht) => //
-  end].
+  all:try solve [  match goal with 
+  [ H : context [ is_erasableb ?X_type ?X ?Γ ?t ?Ht ] |- _ ] => 
+    destruct (@is_erasableP X_type X Γ t Ht)  => //
+  end; intro; 
+    match goal with n : ~ _ |- _  => apply n end; intros ? HH; now rewrite (abstract_env_ext_irr _ HH H) ].
   all:try bang.
-  - cbn. rewrite is_box_tApp.
-    destruct (@is_erasableP Σ Γ (tApp f u) Ht) => //.
+  - destruct (@is_erasableP X_type X Γ t Ht) => //. apply s; eauto. 
+  - cbn in *. rewrite is_box_tApp.
+    destruct (@is_erasableP X_type X Γ (tApp f u) Ht) => //.
     destruct is_box.
-    * cbn in *. clear H0. 
-      assert (wfΣ' : abstract_env_rel' Σ Σ) by reflexivity;
-      pose proof (abstract_env_ext_wf _ wfΣ') as [wf]. 
-      specialize_Σ wfΣ'. destruct Ht, H.
+    * cbn in *. clear H1.
+      pose proof (abstract_env_ext_wf _ H) as [wf]. cbn in *. 
+      specialize_Σ H. destruct Ht, H0.
       eapply (EArities.Is_type_app _ _ _ [_]); eauto.
       eauto using typing_wf_local.
-    * assumption.
+    * intro; apply n; intros. now rewrite (abstract_env_ext_irr _ H3 H).
 Defined.
 
-Lemma erases_erase {Σ : wf_env_ext} {Γ t} 
-(wt : forall Σ0 : global_env_ext, abstract_env_rel' Σ Σ0 -> welltyped Σ0 Γ t) :
-  erases Σ Γ t (erase Σ Γ t wt).
+Lemma erases_erase {X_type X Γ t} 
+(wt : forall Σ : global_env_ext, abstract_env_ext_rel X Σ -> welltyped Σ Γ t) :
+forall Σ : global_env_ext, abstract_env_ext_rel X Σ -> erases Σ Γ t (erase X_type X Γ t wt).
 Proof.
-  revert Γ t wt.
-  apply (erase_elim Σ
+  intros. revert Γ t wt.
+  apply (erase_elim X_type X
     (fun Γ t wt e => Σ;;; Γ |- t ⇝ℇ e)
     (fun Γ l awt e => All2 (erases Σ Γ) l e)
     (fun Γ p l awt e => 
@@ -654,46 +675,46 @@ Proof.
     all:try discriminate.
     all:try bang.
     all:try match goal with 
-      [ H : context [is_erasableb ?Σ ?Γ ?t ?Ht ] |- _ ] => 
-        destruct (@is_erasableP Σ Γ t Ht) as [[H']|H'] => //;
+      [ H : context [is_erasableb ?X_type ?X ?Γ ?t ?Ht ] |- _ ] => 
+        destruct (@is_erasableP X_type X Γ t Ht) as [[H']|H'] => //; eauto ;
         try now eapply erases_box
     end.
     all: try solve [constructor; eauto].
-  all:try destruct Σ.(wf_env_ext_wf) as [wfΣ].
-  all: cbn in *; assert (wfΣ' : abstract_env_rel' Σ Σ) by reflexivity;
-  try constructor; auto;
-  try pose proof (abstract_env_ext_wf _ wfΣ') as [wf];
-  specialize_Σ wfΣ'.
+  all:try destruct (abstract_env_ext_wf X H) as [wfΣ].
+  all: cbn in *; try constructor; auto;
+  specialize_Σ H.
   
   - clear Heq.
     eapply nisErasable_Propositional in Ht; auto.
-
+    intro; eapply H'; intros. now rewrite (abstract_env_ext_irr _ H0 H).  
   - cbn.
-    destruct (Ht _ wfΣ').
-    destruct (inversion_Case _ _ X0) as [mdecl [idecl []]]; eauto.
+    destruct (Ht _ H).
+    destruct (inversion_Case _ _ X1) as [mdecl [idecl []]]; eauto.
     eapply elim_restriction_works; eauto.
-    intros isp. eapply isErasable_Proof in isp. eauto.
+    intros isp. eapply isErasable_Proof in isp.
+    eapply H'; intros. now rewrite (abstract_env_ext_irr _ H1 H).
 
   - clear Heq.
-    destruct (Ht _ wfΣ') as [? Ht'].
-    clear H. eapply inversion_Proj in Ht' as (?&?&?&?&?&?&?&?&?&?); auto.
+    destruct (Ht _ H) as [? Ht'].
+    clear H0. eapply inversion_Proj in Ht' as (?&?&?&?&?&?&?&?&?&?); auto.
     eapply elim_restriction_works_proj; eauto. exact d.
-    intros isp. eapply isErasable_Proof in isp; eauto.
+    intros isp. eapply isErasable_Proof in isp.
+    eapply H'; intros. now rewrite (abstract_env_ext_irr _ H0 H).
 
-  - cbn.
+  - cbn. pose proof (abstract_env_ext_wf _ H) as [wf].
     pose proof Hmfix as Hmfix'.
-    specialize (Hmfix' Σ eq_refl). destruct Hmfix'.
-    depelim X0. destruct a.
+    specialize (Hmfix' _ H). destruct Hmfix'.
+    depelim X1. destruct a.
     assert (exists na ty bod, dbody d = tLambda na ty bod).
-    { clear -H0. destruct (dbody d) => //. now do 3 eexists. }
-    destruct H2 as [na [ty [bod eq]]]. rewrite {1 3}eq /= //.
-    move: H. rewrite {1}eq.
-    set (et := erase _ _ _ _). clearbody et.
+    { clear -H1. destruct (dbody d) => //. now do 3 eexists. }
+    destruct H3 as [na [ty [bod eq]]]. rewrite {1 3}eq /= //.
+    move: H0. rewrite {1}eq.
+    set (et := erase _ _ _ _ _). clearbody et.
     intros He. depelim He. cbn.
     split => //. cbn. rewrite eq. now constructor.
     split => //. cbn. rewrite eq.
-    destruct H1.
-    eapply Is_type_lambda in X1; tea. 2:pcuic. destruct X1.
+    destruct H2.
+    eapply Is_type_lambda in X2; tea. 2:pcuic. destruct X2.
     now constructor.
 Qed.
 
@@ -704,20 +725,20 @@ Transparent wf_reduction.
   term.
 *)
 
-
-Program Definition erase_constant_body (Σ : wf_env_ext) (cb : constant_body)
-  (Hcb : ∥ on_constant_decl (lift_typing typing) Σ cb ∥) : E.constant_body * KernameSet.t :=  
+Program Definition erase_constant_body X_type X 
+  (cb : constant_body) 
+  (Hcb : forall Σ : global_env_ext, abstract_env_ext_rel X Σ -> ∥ on_constant_decl (lift_typing typing) Σ cb ∥) : E.constant_body * KernameSet.t :=  
   let '(body, deps) := match cb.(cst_body) with
           | Some b => 
-            let b' := erase Σ [] b _ in
+            let b' := erase X_type X [] b _ in
             (Some b', term_global_deps b')
           | None => (None, KernameSet.empty)
           end in
   ({| E.cst_body := body; |}, deps).
 Next Obligation.
 Proof.
-  sq. red in Hcb. rewrite <-Heq_anonymous in Hcb. simpl in Hcb, H. cbn in H. subst Σ0.
-  eexists; eauto.
+  specialize_Σ H. sq. red in Hcb. 
+  rewrite <-Heq_anonymous in Hcb. now eexists.
 Qed.
 
 Definition erase_one_inductive_body (oib : one_inductive_body) : E.one_inductive_body :=
@@ -742,1526 +763,16 @@ Definition erase_mutual_inductive_body (mib : mutual_inductive_body) : E.mutual_
   let bodies := map erase_one_inductive_body bds in
   {| E.ind_npars := mib.(ind_npars);
      E.ind_bodies := bodies; |}.
- 
-Program Definition remove_kn (kn : kername) (Σ : wf_env) decls (prf : exists d, Σ.(referenced_impl_env).(declarations) = (kn, d) :: decls) : wf_env :=
- {| wf_env_referenced := {| referenced_impl_env := {| universes := Σ.(referenced_impl_env).(universes); declarations := decls |} |};
-    wf_env_map := EnvMap.EnvMap.remove kn Σ.(wf_env_map); 
-    |}.
 
-Import EnvMap.
-Next Obligation.
-  destruct Σ.(referenced_impl_wf). sq.
-  destruct X as [onu ond]; split => //. rewrite H in ond.
-  now depelim ond.
-Qed.
-Next Obligation.
-  pose proof Σ.(wf_env_map_repr). red in H0.
-  rewrite H in H0.
-  set (Σ0 := EnvMap.of_global_env decls).
-  epose proof (EnvMap.remove_add_eq decls kn prf Σ0).
-  forward_keep H1.
-  { pose proof (Σf := wf_env_fresh Σ). rewrite H in Σf. now depelim Σf. }
-  forward_keep H1.
-  { pose proof (Σf := wf_env_fresh Σ). rewrite H in Σf. now depelim Σf. }
-  forward_keep H1.
-  { red. unfold EnvMap.equal. reflexivity. }
-  unfold EnvMap.repr.
-  rewrite H0 /=. unfold KernameMapFact.uncurry; cbn.
-  unfold EnvMap.add in H1. rewrite H1. reflexivity.
-Qed.
-  
-Program Definition make_wf_env_ext (Σ : wf_env) (univs : universes_decl) (prf : ∥ wf_ext (Σ, univs) ∥) : wf_env_ext :=
-  {| wf_env_ext_referenced := {| referenced_impl_env_ext := (Σ, univs);|} ;
-     wf_env_ext_map := Σ.(wf_env_map);
-     wf_env_ext_map_repr := Σ.(wf_env_map_repr) |}.
+Definition Hlookup {cf} (X_type : abstract_env_ext_impl) (X : X_type.π1) (X_type' : abstract_env_ext_impl)
+  (X' : X_type'.π1) := 
+  forall Σ : global_env_ext, abstract_env_ext_rel X Σ ->
+  forall Σ' : global_env_ext, abstract_env_ext_rel X' Σ' ->
+  forall kn decl decl',
+    lookup_env Σ kn = Some decl ->
+    lookup_env Σ' kn = Some decl' ->
+    abstract_env_lookup X kn = abstract_env_lookup X' kn.
 
-Require Import Morphisms.
-From MetaCoq.Template Require Import uGraph.
-
-Program Fixpoint erase_global_decls (deps : KernameSet.t) (Σ : wf_env) (decls : global_declarations) 
-  (prop : Σ.(referenced_impl_env).(declarations) = decls) : E.global_declarations :=
-  match decls with
-  | [] => []
-  | (kn, ConstantDecl cb) :: decls =>
-    let wfΣ' := remove_kn kn Σ decls _ in
-    if KernameSet.mem kn deps then
-      let wfΣext' := make_wf_env_ext wfΣ' (cst_universes cb) _ in
-      let cb' := erase_constant_body wfΣext' cb _ in
-      let deps := KernameSet.union deps (snd cb') in
-      let Σ' := erase_global_decls deps wfΣ' decls _ in
-      ((kn, E.ConstantDecl (fst cb')) :: Σ')
-    else
-      erase_global_decls deps wfΣ' decls _
-
-  | (kn, InductiveDecl mib) :: decls =>
-    let wfΣ' := remove_kn kn Σ decls _ in
-    if KernameSet.mem kn deps then
-      let mib' := erase_mutual_inductive_body mib in
-      let Σ' := erase_global_decls deps wfΣ' decls _ in
-      ((kn, E.InductiveDecl mib') :: Σ')
-    else erase_global_decls deps wfΣ' decls _
-  end.
-Next Obligation.
-  now eexists.
-Qed.
-Next Obligation.
-  epose proof Σ.(referenced_impl_wf).
-  sq. destruct H as [onu ond]. rewrite -Heq_decls in ond. depelim ond. split => //.
-Qed.
-Next Obligation.
-  epose proof Σ.(referenced_impl_wf).
-  sq. destruct H as [onu ond]. rewrite -Heq_decls in ond. now depelim ond.
-Qed.
-Next Obligation.
-  now eexists.
-Qed.
-
-Definition erase_global deps Σ :=
-  erase_global_decls deps Σ Σ.(declarations) eq_refl.
-
-Definition global_erased_with_deps (Σ : global_env) (Σ' : EAst.global_declarations) kn :=
-  (exists cst, declared_constant Σ kn cst /\
-   exists cst' : EAst.constant_body,
-    EGlobalEnv.declared_constant Σ' kn cst' /\
-    erases_constant_body (Σ, cst_universes cst) cst cst' /\
-    (forall body : EAst.term,
-     EAst.cst_body cst' = Some body -> erases_deps Σ Σ' body)) \/
-  (exists mib mib', declared_minductive Σ kn mib /\ 
-    EGlobalEnv.declared_minductive Σ' kn mib' /\
-    erases_mutual_inductive_body mib mib').
-
-Definition includes_deps (Σ : global_env) (Σ' : EAst.global_declarations) deps :=  
-  forall kn, 
-    KernameSet.In kn deps ->
-    global_erased_with_deps Σ Σ' kn.
-
-Lemma includes_deps_union (Σ : global_env) (Σ' : EAst.global_declarations) deps deps' :
-  includes_deps Σ Σ' (KernameSet.union deps deps') ->
-  includes_deps Σ Σ' deps /\ includes_deps Σ Σ' deps'.
-Proof.
-  intros.
-  split; intros kn knin; eapply H; rewrite KernameSet.union_spec; eauto.
-Qed.
-
-Lemma includes_deps_fold {A} (Σ : global_env) (Σ' : EAst.global_declarations) brs deps (f : A -> EAst.term) :
-  includes_deps Σ Σ'
-  (fold_left
-    (fun (acc : KernameSet.t) (x : A) =>
-      KernameSet.union (term_global_deps (f x)) acc) brs
-      deps) ->
-  includes_deps Σ Σ' deps /\
-  (forall x, In x brs ->
-    includes_deps Σ Σ' (term_global_deps (f x))).
-Proof.
-  intros incl; split.
-  intros kn knin; apply incl.
-  rewrite knset_in_fold_left. left; auto.
-  intros br brin. intros kn knin. apply incl.
-  rewrite knset_in_fold_left. right.
-  now exists br.
-Qed.
-
-Definition declared_kn Σ kn :=
-  ∥ ∑ decl, lookup_env Σ kn = Some decl ∥.
-
-Lemma term_global_deps_spec {cf} {Σ : global_env_ext} {Γ t et T} : 
-  wf Σ.1 ->
-  Σ ;;; Γ |- t : T ->
-  Σ;;; Γ |- t ⇝ℇ et ->
-  forall x, KernameSet.In x (term_global_deps et) -> declared_kn Σ x.
-Proof.
-  intros wf wt er.
-  induction er in T, wt |- * using erases_forall_list_ind;
-    cbn in *; try solve [constructor]; intros kn' hin;
-    repeat match goal with 
-    | [ H : KernameSet.In _ KernameSet.empty |- _ ] =>
-      now apply KernameSet.empty_spec in hin
-    | [ H : KernameSet.In _ (KernameSet.union _ _) |- _ ] =>
-      apply KernameSet.union_spec in hin as [?|?]
-    end.
-  - apply inversion_Lambda in wt as (? & ? & ? & ? & ?); eauto.
-  - apply inversion_LetIn in wt as (? & ? & ? & ? & ? & ?); eauto.
-  - apply inversion_LetIn in wt as (? & ? & ? & ? & ? & ?); eauto.
-  - apply inversion_App in wt as (? & ? & ? & ? & ? & ?); eauto.
-  - apply inversion_App in wt as (? & ? & ? & ? & ? & ?); eauto.
-  - apply inversion_Const in wt as (? & ? & ? & ? & ?); eauto.
-    eapply KernameSet.singleton_spec in hin; subst.
-    red in d. red. sq. rewrite d. intuition eauto.
-  - apply inversion_Construct in wt as (? & ? & ? & ? & ? & ? & ?); eauto.
-    destruct kn.
-    eapply KernameSet.singleton_spec in hin; subst.
-    destruct d as [[H' _] _]. red in H'. simpl in *.
-    red. sq. rewrite H'. intuition eauto.
-  - apply inversion_Case in wt as (? & ? & ? & ? & [] & ?); eauto.
-    destruct ci as [kn i']; simpl in *.
-    eapply KernameSet.singleton_spec in H1; subst.
-    destruct x1 as [d _]. red in d.
-    simpl in *. eexists; intuition eauto.
-
-  - apply inversion_Case in wt as (? & ? & ? & ? & [] & ?); eauto.
-    eapply knset_in_fold_left in H1.
-    destruct H1. eapply IHer; eauto.
-    destruct H1 as [br [inbr inkn]].
-    eapply Forall2_All2 in H0.
-    assert (All (fun br => ∑ T, Σ ;;; Γ ,,, inst_case_branch_context p br |- br.(bbody) : T) brs).
-    eapply All2i_All_right. eapply brs_ty.
-    simpl. intuition auto. eexists ; eauto.
-    now rewrite -(PCUICCasesContexts.inst_case_branch_context_eq a).
-    eapply All2_All_mix_left in H0; eauto. simpl in H0.
-    eapply All2_In_right in H0; eauto.
-    destruct H0.
-    destruct X1 as [br' [[T' HT] ?]].
-    eauto.
-  
-  - eapply KernameSet.singleton_spec in H0; subst.
-    apply inversion_Proj in wt as (?&?&?&?&?&?&?&?&?&?); eauto.
-    destruct d as [[[d _] _] _]. red in d. eexists; eauto.
-
-  - apply inversion_Proj in wt as (?&?&?&?&?&?&?&?&?); eauto.
-
-  - apply inversion_Fix in wt as (?&?&?&?&?&?&?); eauto.
-    eapply knset_in_fold_left in hin as [|].
-    now eapply KernameSet.empty_spec in H0.
-    destruct H0 as [? [ina indeps]].
-    eapply Forall2_All2 in H.
-    eapply All2_All_mix_left in H; eauto.
-    eapply All2_In_right in H; eauto.
-    destruct H as [[def [Hty Hdef]]].
-    eapply Hdef; eauto.
-
-  - apply inversion_CoFix in wt as (?&?&?&?&?&?&?); eauto.
-    eapply knset_in_fold_left in hin as [|].
-    now eapply KernameSet.empty_spec in H0.
-    destruct H0 as [? [ina indeps]].
-    eapply Forall2_All2 in H.
-    eapply All2_All_mix_left in H; eauto.
-    eapply All2_In_right in H; eauto.
-    destruct H as [[def [Hty Hdef]]].
-    eapply Hdef; eauto.
-Qed.
-
-Global Remove Hints erases_deps_eval : core.
-
-Lemma erase_global_erases_deps {Σ} {Σ' : EAst.global_declarations} {Γ t et T} : 
-  wf_ext Σ ->
-  Σ;;; Γ |- t : T ->
-  Σ;;; Γ |- t ⇝ℇ et ->
-  includes_deps Σ Σ' (term_global_deps et) ->
-  erases_deps Σ Σ' et.
-Proof.
-  intros wf wt er.
-  induction er in er, t, T, wf, wt |- * using erases_forall_list_ind;
-    cbn in *; try solve [constructor]; intros Σer;
-    repeat match goal with 
-    | [ H : includes_deps _ _ (KernameSet.union _ _ ) |- _ ] =>
-      apply includes_deps_union in H as [? ?]
-    end.
-  - now apply inversion_Evar in wt.
-  - constructor.
-    now apply inversion_Lambda in wt as (? & ? & ? & ? & ?); eauto.
-  - apply inversion_LetIn in wt as (? & ? & ? & ? & ? & ?); eauto.
-    constructor; eauto.
-  - apply inversion_App in wt as (? & ? & ? & ? & ? & ?); eauto.
-    now constructor; eauto.
-  - apply inversion_Const in wt as (? & ? & ? & ? & ?); eauto.
-    specialize (Σer kn).
-    forward Σer. rewrite KernameSet.singleton_spec //.
-    destruct Σer as [[c' [declc' (? & ? & ? & ?)]]|].
-    pose proof (declared_constant_inj _ _ d declc'). subst x.
-    now econstructor; eauto.
-    destruct H as [mib [mib' [declm declm']]].
-    red in declm, d. rewrite d in declm. noconf declm.
-  - apply inversion_Construct in wt as (? & ? & ? & ? & ? & ?); eauto.
-    red in Σer. destruct kn.
-    setoid_rewrite KernameSetFact.singleton_iff in Σer.
-    destruct (Σer _ eq_refl) as [ (? & ? & ? & ? & ? & ?) | (? & ? & ? & ? & ?) ].
-    + red in H0. destruct d as [[]]. red in H4. cbn in *. unfold PCUICEnvironment.fst_ctx in *. congruence.
-    + pose proof H2 as H2'. destruct d. cbn in *. destruct H3. cbn in *. red in H3. red in H0. rewrite H0 in H3. invs H3.
-      destruct H2.
-      red in H1.
-      eapply Forall2_nth_error_Some_l in H2 as (? & ? & ?); eauto. pose proof H6 as H6'. destruct H6 as (? & ? & ? & ? & ?); eauto.
-      eapply Forall2_nth_error_Some_l in H6 as ([] & ? & ? & ?); subst; eauto.
-      econstructor. repeat eapply conj; eauto.
-      repeat eapply conj; cbn; eauto. eauto. eauto.
-  - apply inversion_Case in wt as (? & ? & ? & ? & [] & ?); eauto.
-    destruct ci as [[kn i'] ? ?]; simpl in *.
-    apply includes_deps_fold in H2 as [? ?].
-
-    specialize (H1 kn). forward H1.
-    now rewrite KernameSet.singleton_spec. red in H1. destruct H1.
-    elimtype False. destruct H1 as [cst [declc _]].
-    { red in declc. destruct x1 as [d _]. red in d. rewrite d in declc. noconf declc. }
-    destruct H1 as [mib [mib' [declm [declm' em]]]].
-    pose proof em as em'. destruct em'.
-    destruct x1 as [x1 hnth].
-    red in x1, declm. rewrite x1 in declm. noconf declm.
-    eapply Forall2_nth_error_left in H1; eauto. destruct H1 as [? [? ?]].
-    eapply erases_deps_tCase; eauto. 
-    split; eauto. split; eauto.
-    destruct H1.
-    eapply In_Forall in H3.
-    eapply All_Forall. eapply Forall_All in H3.
-    eapply Forall2_All2 in H0.
-    eapply All2_All_mix_right in H0; eauto.
-    assert (All (fun br => ∑ T, Σ ;;; Γ ,,, inst_case_branch_context p br |- br.(bbody) : T) brs).
-    eapply All2i_All_right. eapply brs_ty.
-    simpl. intuition auto. eexists ; eauto.
-    now rewrite -(PCUICCasesContexts.inst_case_branch_context_eq a).
-    ELiftSubst.solve_all. destruct a0 as [T' HT]. eauto.
-    
-  - apply inversion_Proj in wt as (?&?&?&?&?&?&?&?&?&?); eauto.
-    destruct (proj1 d).
-    specialize (H0 (inductive_mind p.(proj_ind))). forward H0.
-    now rewrite KernameSet.singleton_spec. red in H0. destruct H0.
-    elimtype False. destruct H0 as [cst [declc _]].
-    { red in declc. destruct d as [[[d _] _] _]. red in d. rewrite d in declc. noconf declc. }
-    destruct H0 as [mib [mib' [declm [declm' em]]]].
-    assert (mib = x0).
-    { destruct d as [[[]]].
-      red in H0, declm. rewrite H0 in declm. now noconf declm. } 
-    subst x0.
-    pose proof em as em'. destruct em'.
-    eapply Forall2_nth_error_left in H0 as (x' & ? & ?); eauto.
-    2:{ apply d. }
-    simpl in *.
-    destruct (ind_ctors x1) => //. noconf H3.
-    set (H1' := H5). destruct H1' as [].
-    set (d' := d). destruct d' as [[[]]].
-    eapply Forall2_All2 in H3. eapply All2_nth_error_Some in H3 as [? [? []]]; tea.
-    destruct H6 as [Hprojs _].
-    eapply Forall2_All2 in Hprojs. eapply All2_nth_error_Some in Hprojs as [? []]; tea.
-    2:eapply d.
-    econstructor; tea. all:eauto.
-    split => //. 2:split; eauto.
-    split; eauto. split; eauto.
-    rewrite -H4. symmetry; apply d.
-    
-  - constructor.
-    apply inversion_Fix in wt as (?&?&?&?&?&?&?); eauto.
-    eapply All_Forall. eapply includes_deps_fold in Σer as [_ Σer].
-    eapply In_Forall in Σer.
-    eapply Forall_All in Σer.
-    eapply Forall2_All2 in H.
-    ELiftSubst.solve_all.
-  - constructor.
-    apply inversion_CoFix in wt as (?&?&?&?&?&?&?); eauto.
-    eapply All_Forall. eapply includes_deps_fold in Σer as [_ Σer].
-    eapply In_Forall in Σer.
-    eapply Forall_All in Σer.
-    eapply Forall2_All2 in H.
-    ELiftSubst.solve_all. Unshelve. 
-Qed.
-
-Lemma erases_weakeninv_env {Σ Σ' : global_env_ext} {Γ t t' T} :
-  wf Σ' -> extends_decls Σ Σ' -> 
-  Σ ;;; Γ |- t : T ->
-  erases Σ Γ t t' -> erases (Σ'.1, Σ.2) Γ t t'.
-Proof.
-  intros wfΣ' ext Hty.
-  eapply (env_prop_typing ESubstitution.erases_extends); tea.
-  eapply extends_decls_wf; tea.
-Qed.  
- 
-Lemma erases_deps_weaken kn d (Σ : global_env) (Σ' : EAst.global_declarations) t : 
-  wf (add_global_decl Σ (kn, d)) ->
-  erases_deps Σ Σ' t ->
-  erases_deps (add_global_decl Σ (kn, d)) Σ' t.
-Proof.
-  intros wfΣ er.
-  induction er using erases_deps_forall_ind; try solve [now constructor].
-  - assert (kn <> kn0).
-    { inv wfΣ. inv X. intros <-.
-      eapply lookup_env_Some_fresh in H. contradiction. }
-    eapply erases_deps_tConst with cb cb'; eauto.
-    red. rewrite /lookup_env lookup_env_cons_fresh //.
-    red.
-    red in H1.
-    destruct (cst_body cb) eqn:cbe;
-    destruct (E.cst_body cb') eqn:cbe'; auto.
-    specialize (H3 _ eq_refl).
-    eapply on_declared_constant in H; auto.
-    2:{ inv wfΣ. now inv X. }
-    red in H. rewrite cbe in H. simpl in H.
-    eapply (erases_weakeninv_env (Σ := (Σ, cst_universes cb))
-       (Σ' := (add_global_decl Σ (kn, d), cst_universes cb))); eauto.
-    simpl.
-    split => //; eexists [(kn, d)]; intuition eauto.
-  - econstructor; eauto. eapply weakening_env_declared_constructor; eauto.
-    eapply extends_decls_extends. econstructor; try reflexivity. eexists [(_, _)]; reflexivity. 
-  - econstructor; eauto.
-    red. destruct H. split; eauto.
-    red in H. red.
-    inv wfΣ. inv X.
-    rewrite -H. simpl. unfold lookup_env; simpl. destruct (eqb_spec (inductive_mind p.1) kn); try congruence.
-    eapply lookup_env_Some_fresh in H. subst kn; contradiction.
-  - econstructor; eauto.
-    red. destruct H. split; eauto.
-    destruct d0; split; eauto.
-    destruct d0; split; eauto.
-    inv wfΣ. inv X.
-    red in H |- *.
-    rewrite -H. simpl. unfold lookup_env; simpl; destruct (eqb_spec (inductive_mind p.(proj_ind)) kn); try congruence.
-    eapply lookup_env_Some_fresh in H. subst kn. contradiction.
-Qed.
-
-Lemma lookup_env_ext {Σ kn kn' d d'} : 
-  wf (add_global_decl Σ (kn', d')) ->
-  lookup_env Σ kn = Some d ->
-  kn <> kn'.
-Proof.
-  intros wf hl. 
-  eapply lookup_env_Some_fresh in hl.
-  inv wf. inv X.
-  destruct (eqb_spec kn kn'); subst; congruence.
-Qed.
-
-Lemma lookup_env_cons_disc {Σ kn kn' d} : 
-  kn <> kn' ->
-  lookup_env (add_global_decl Σ (kn', d)) kn = lookup_env Σ kn.
-Proof.
-  intros Hk. simpl; unfold lookup_env; simpl.
-  destruct (eqb_spec kn kn'); congruence.
-Qed.
-
-Lemma elookup_env_cons_disc {Σ kn kn' d} : 
-  kn <> kn' ->
-  EGlobalEnv.lookup_env ((kn', d) :: Σ) kn = EGlobalEnv.lookup_env Σ kn.
-Proof.
-  intros Hk. simpl.
-  destruct (eqb_spec kn kn'); congruence.
-Qed.
-
-Lemma global_erases_with_deps_cons kn kn' d d' Σ Σ' : 
-  wf (add_global_decl Σ (kn', d)) ->
-  global_erased_with_deps Σ Σ' kn ->
-  global_erased_with_deps (add_global_decl Σ (kn', d)) ((kn', d') :: Σ') kn.
-Proof.
-  intros wf [[cst [declc [cst' [declc' [ebody IH]]]]]|].
-  red. inv wf. inv X. left.
-  exists cst. split.
-  red in declc |- *. unfold lookup_env in *.
-  rewrite lookup_env_cons_fresh //.
-  { eapply lookup_env_Some_fresh in declc.
-    intros <-; contradiction. }
-  exists cst'.
-  unfold EGlobalEnv.declared_constant. rewrite EGlobalEnv.elookup_env_cons_fresh //.
-  { eapply lookup_env_Some_fresh in declc.
-    intros <-; contradiction. }
-  red in ebody. unfold erases_constant_body.
-  destruct (cst_body cst) eqn:bod; destruct (E.cst_body cst') eqn:bod' => //.
-  intuition auto.
-  eapply (erases_weakeninv_env (Σ  := (_, cst_universes cst)) (Σ' := (add_global_decl Σ (kn', d), cst_universes cst))); eauto.
-  constructor; eauto. constructor; eauto.
-  split => //. exists [(kn', d)]; intuition eauto.
-  eapply on_declared_constant in declc; auto.
-  red in declc. rewrite bod in declc. eapply declc.
-  split => //.
-  noconf H0.
-  eapply erases_deps_cons; eauto.
-  constructor; auto.
-
-  right. destruct H as [mib [mib' [? [? ?]]]].
-  exists mib, mib'. intuition eauto.
-  * red. red in H. pose proof (lookup_env_ext wf H).
-    now rewrite lookup_env_cons_disc.
-  * red. pose proof (lookup_env_ext wf H).
-    now rewrite elookup_env_cons_disc.
-Qed.
-
-Lemma global_erases_with_deps_weaken kn kn' d Σ Σ' : 
-  wf (add_global_decl Σ (kn', d)) ->
-  global_erased_with_deps Σ Σ' kn ->
-  global_erased_with_deps (add_global_decl Σ (kn', d)) Σ' kn.
-Proof.
-  intros wf [[cst [declc [cst' [declc' [ebody IH]]]]]|].
-  red. inv wf. inv X. left.
-  exists cst. split.
-  red in declc |- *.
-  unfold lookup_env in *.
-  rewrite lookup_env_cons_fresh //.
-  { eapply lookup_env_Some_fresh in declc.
-    intros <-. contradiction. }
-  exists cst'.
-  unfold EGlobalEnv.declared_constant.
-  red in ebody. unfold erases_constant_body.
-  destruct (cst_body cst) eqn:bod; destruct (E.cst_body cst') eqn:bod' => //.
-  intuition auto.
-  eapply (erases_weakeninv_env (Σ  := (Σ, cst_universes cst)) (Σ' := (add_global_decl Σ (kn', d), cst_universes cst))). 4:eauto.
-  split; auto. constructor; eauto.
-  split; auto; exists [(kn', d)]; intuition eauto.
-  eapply on_declared_constant in declc; auto.
-  red in declc. rewrite bod in declc. eapply declc. split => //.
-  noconf H0.
-  apply erases_deps_weaken.
-  { split; auto. cbn. constructor; auto. }
-  auto.
-
-  right. destruct H as [mib [mib' [Hm [? ?]]]].
-  exists mib, mib'; intuition auto.
-  red. unfold lookup_env in *.
-  rewrite lookup_env_cons_fresh //.
-  now epose proof (lookup_env_ext wf Hm).
-Qed.
-
-Lemma erase_constant_body_correct (Σ : wf_env_ext) Σ' cb (onc : ∥ on_constant_decl (lift_typing typing) Σ cb ∥) :
-  wf Σ' -> extends_decls Σ Σ' ->
-  erases_constant_body (Σ', Σ.(referenced_impl_env_ext).2) cb (fst (erase_constant_body Σ cb onc)).
-Proof.
-  red. sq. destruct cb as [name [bod|] univs]; simpl. intros.
-  eapply (erases_weakeninv_env (Σ := Σ) (Σ' := (Σ', univs))); simpl; auto.
-  eapply onc. eapply erases_erase. auto.
-Qed.
-
-Lemma erase_constant_body_correct' {Σ : wf_env_ext} {cb} {onc : ∥ on_constant_decl (lift_typing typing) Σ cb ∥} {body} :
-  EAst.cst_body (fst (erase_constant_body Σ cb onc)) = Some body ->
-  ∥ ∑ t T, (Σ ;;; [] |- t : T) * (Σ ;;; [] |- t ⇝ℇ body) *
-    (term_global_deps body = snd (erase_constant_body Σ cb onc)) ∥.
-Proof.
-  intros. destruct cb as [name [bod|] univs]; simpl. intros.
-  simpl in H. noconf H.
-  set (obl :=(erase_constant_body_obligation_1 Σ
-  {|
-  cst_type := name;
-  cst_body := Some bod;
-  cst_universes := univs |} onc bod eq_refl)). clearbody obl.
-  assert (wfΣ' : abstract_env_rel' Σ Σ) by reflexivity.
-  destruct (obl _ wfΣ'). sq.
-  exists bod, A; intuition auto. simpl.
-  eapply erases_erase. now simpl in H.
-Qed.
-
-Lemma erases_mutual {Σ mdecl m} : 
-  on_inductive (lift_typing typing) (Σ, ind_universes m) mdecl m ->
-  erases_mutual_inductive_body m (erase_mutual_inductive_body m).
-Proof.
-  intros oni.
-  destruct m; constructor; simpl; auto.
-  eapply onInductives in oni; simpl in *.
-  assert (Alli (fun i oib => 
-    match destArity [] oib.(ind_type) with Some _ => True | None => False end) 0 ind_bodies0).
-  { eapply Alli_impl; eauto.
-    simpl. intros n x []. simpl in *. rewrite ind_arity_eq.
-    rewrite !destArity_it_mkProd_or_LetIn /= //. } clear oni.
-  induction X; constructor; auto.
-  destruct hd; constructor; simpl; auto.
-  clear.
-  induction ind_ctors0; constructor; auto.
-  cbn in *.
-  intuition auto.
-  induction ind_projs0; constructor; auto.
-  unfold isPropositionalArity.
-  destruct destArity as [[? ?]|] eqn:da; auto.
-Qed.
-
-Lemma erase_global_includes (Σ : wf_env) deps deps' :
-  (forall d, KernameSet.In d deps' -> ∥ ∑ decl, lookup_env Σ d = Some decl ∥) ->
-  KernameSet.subset deps' deps ->
-  let Σ' := erase_global deps Σ in
-  includes_deps Σ Σ' deps'.
-Proof.
-  sq. unfold erase_global.
-  set (e := eq_refl). clearbody e.
-  move: e. generalize (declarations Σ) at 2 3.
-  induction g in deps, deps', Σ |- *.
-  - simpl; intros eq H.
-    intros sub i hin. elimtype False.
-    specialize (H i hin) as [[decl Hdecl]].
-    rewrite /lookup_env eq in Hdecl. noconf Hdecl.
-  - intros e H sub i hin.
-    destruct Σ.(referenced_impl_wf) as [wfΣ].
-    destruct a as [kn d].
-    eapply KernameSet.subset_spec in sub.
-    destruct (H i hin) as [[decl Hdecl]]. unfold lookup_env in Hdecl.
-    cbn in Hdecl.
-    pose proof (eqb_spec i kn).
-    rewrite e in Hdecl. move: Hdecl. cbn -[erase_global_decls].
-    elim: H0. intros -> [= <-].
-    * destruct d as [|]; [left|right].
-      { exists c. split; auto. red.
-        unfold lookup_env; simpl; rewrite e. cbn. rewrite eq_kername_refl //.
-        pose proof (sub _ hin) as indeps.
-        eapply KernameSet.mem_spec in indeps.
-        unfold EGlobalEnv.declared_constant.
-        destruct (H _ hin) as [[decl hd]].
-        eexists; intuition eauto.
-        cbn. 
-        rewrite indeps. cbn.
-        rewrite eq_kername_refl. reflexivity.
-        eapply erase_constant_body_correct; eauto.
-        set (obl2 := erase_global_decls_obligation_2 _ _ _ _ _ _ _). clearbody obl2.
-        set (obl1 := erase_global_decls_obligation_1 _ _ _ _ _ _ _) in *.
-        clearbody obl1. 
-        red. simpl.
-        split => //. exists [(kn, ConstantDecl c)]; intuition auto.
-        cbn.
-        set (obl2 := erase_global_decls_obligation_2 _ _ _ _ _ _ _) in *. 
-        set (obl1 := erase_global_decls_obligation_1 _ _ _ _ _ _ _) in *. 
-        cbn [erase_global_decls].
-        rewrite indeps.
-        rewrite -wf_env_eta e.
-        set (Σp := {| universes := Σ.(universes); declarations := g |}).
-        eapply (erases_deps_cons Σp); eauto.
-        apply wfΣ. destruct wfΣ. now rewrite e in o0.
-        pose proof (erase_constant_body_correct' H0).
-        sq. destruct H1 as [bod [bodty [[Hbod Hebod] Heqdeps]]].
-        set (wfΣp := make_wf_env_ext _ _ _) in *.
-        assert ((Σp, cst_universes c) = wfΣp :> global_env_ext) by reflexivity.
-        eapply (erase_global_erases_deps (Σ := (Σp, cst_universes c))); simpl; auto.
-        { constructor; simpl; auto. depelim wfΣ. rewrite e in o0. now depelim o0.
-           depelim wfΣ. rewrite e in o0. now depelim o0. }
-        all:eauto.
-        assert (wfuΣ : wf {| universes := Σ.(universes); declarations := g |}).
-        { split => //. cbn. apply wfΣ. cbn. destruct wfΣ.
-          rewrite e in o0. now depelim o0. }
-        eapply (IHg (remove_kn kn Σ g obl1)).
-        { intros.
-          eapply term_global_deps_spec in Hebod; eauto. }
-        { eapply KernameSet.subset_spec.
-          intros x hin'. eapply KernameSet.union_spec. right; auto.
-          set (obl2' := erase_global_decls_obligation_2 _ _ _ _ _ _ _) in *.
-          set (obl1' := erase_global_decls_obligation_1 _ _ _ _ _ _ _) in *.
-          set (obl3' := erase_global_decls_obligation_3 _ _ _ _ _ _ _) in *.
-          now rewrite -Heqdeps. } }
-        { eexists m, _; intuition eauto.
-          simpl. rewrite /declared_minductive /lookup_env e.
-          simpl. rewrite eq_kername_refl. reflexivity.
-          specialize (sub _ hin).
-          eapply KernameSet.mem_spec in sub.
-          simpl. rewrite sub.
-          red. cbn. rewrite eq_kername_refl.
-          reflexivity.
-          assert (declared_minductive Σ kn m).
-          { red. unfold lookup_env. rewrite e. cbn. now rewrite eqb_refl. }
-          eapply on_declared_minductive in H0; tea.
-          now eapply erases_mutual. }
-
-    * intros ikn Hi.
-      set (Σp := {| universes := Σ.(universes); declarations := g |}).
-      assert (wfΣp : wf {| universes := Σ.(universes); declarations := g |}).
-      { split => //. cbn. apply wfΣ. cbn. destruct wfΣ.
-        rewrite e in o0. now depelim o0. }
-      destruct d as [|].
-      ++ simpl. destruct (KernameSet.mem kn deps) eqn:eqkn.
-        rewrite -wf_env_eta e.
-        eapply (global_erases_with_deps_cons _ kn (ConstantDecl _) _ Σp); eauto.
-        unfold add_global_decl; cbn. now rewrite -e wf_env_eta.
-        eapply (IHg (remove_kn kn Σ g _) _ (KernameSet.singleton i)); auto.
-        3:{ eapply KernameSet.singleton_spec => //. }
-        intros.
-        eapply KernameSet.singleton_spec in H0. subst.
-        constructor; exists decl; auto.
-        eapply KernameSet.subset_spec. intros ? ?.
-        eapply KernameSet.union_spec. left.
-        eapply KernameSet.singleton_spec in H0; subst.
-        now eapply sub.
-      
-        rewrite -wf_env_eta e.
-        eapply (global_erases_with_deps_weaken _ kn (ConstantDecl _) Σp). eauto.
-        rewrite /add_global_decl /= -e wf_env_eta //.
-        eapply (IHg (remove_kn _ _ _ _) deps (KernameSet.singleton i)) => //.
-        3:now eapply KernameSet.singleton_spec.
-        intros d ind%KernameSet.singleton_spec.
-        subst. constructor; eexists; eauto.
-        eapply KernameSet.subset_spec.
-        intros ? hin'. eapply sub. eapply KernameSet.singleton_spec in hin'. now subst.        
-
-      ++ simpl. 
-        destruct (KernameSet.mem kn deps) eqn:eqkn.
-        { rewrite -wf_env_eta e.
-          eapply (global_erases_with_deps_cons _ kn (InductiveDecl _) _ Σp); eauto.
-          { rewrite /add_global_decl /= -e wf_env_eta //. }
-          eapply (IHg (remove_kn _ _ _ _) _ (KernameSet.singleton i)); auto.
-          3:{ eapply KernameSet.singleton_spec => //. }
-          intros.
-          eapply KernameSet.singleton_spec in H0. subst.
-          constructor; exists decl; auto.
-          eapply KernameSet.subset_spec. intros ? ?.
-          eapply KernameSet.singleton_spec in H0; subst.
-          now eapply sub. }
-    
-        { rewrite -wf_env_eta e.
-          eapply (global_erases_with_deps_weaken _ kn (InductiveDecl _) Σp). eauto.
-          { rewrite /add_global_decl /= -e wf_env_eta //. }
-          eapply (IHg (remove_kn _ _ _ _) deps (KernameSet.singleton i)) => //.
-          3:now eapply KernameSet.singleton_spec.
-          intros d ind%KernameSet.singleton_spec.
-          subst. constructor; eexists; eauto.
-          eapply KernameSet.subset_spec.
-          intros ? hin'. eapply sub. eapply KernameSet.singleton_spec in hin'. now subst. }
-Qed.
-
-Lemma erase_correct (wfl := Ee.default_wcbv_flags) (Σ : wf_env) univs wfext t v Σ' t' deps :
-  let Σext := make_wf_env_ext Σ univs wfext in
-  forall wt : forall Σ0 : global_env_ext, abstract_env_rel' Σext Σ0 -> welltyped Σ0 [] t,
-  erase Σext [] t wt = t' ->
-  KernameSet.subset (term_global_deps t') deps ->
-  erase_global deps Σ = Σ' ->
-  Σ |-p t ▷ v ->
-  exists v', Σext;;; [] |- v ⇝ℇ v' /\ ∥ Σ' ⊢ t' ▷ v' ∥.
-Proof.
-  intros Σext wt.
-  intros HΣ' Hsub Ht' ev.
-  pose proof (erases_erase (Σ := Σext) wt); eauto.
-  rewrite HΣ' in H.
-  assert (wfΣ' : abstract_env_rel' Σext Σext) by reflexivity.
-  destruct (wt _ wfΣ') as [T wt'].
-  destruct Σext.(referenced_impl_ext_wf) as [wfΣ].
-  unshelve epose proof (erase_global_erases_deps (Σ' := Σ') wfΣ wt' H _); cycle 2.
-  intros.
-  rewrite <- Ht'.
-  eapply erase_global_includes.
-  intros.
-  eapply term_global_deps_spec in H; eauto.
-  assumption.
-  eapply erases_correct; tea.
-Qed.
-
-Lemma global_env_ind (P : global_env -> Type) (Pnil : forall univs, P {| universes := univs; declarations := [] |})
-  (Pcons : forall (Σ : global_env) d, P Σ -> P (add_global_decl Σ d))
-  (Σ : global_env) : P Σ.
-Proof.
-  destruct Σ as [univs Σ].
-  induction Σ; cbn. apply Pnil.
-  now apply (Pcons {| universes := univs; declarations := Σ |} a).
-Qed.
-
-Lemma on_global_env_ind (P : forall Σ : global_env, wf Σ -> Type)
-  (Pnil : forall univs (onu : on_global_univs univs), P {| universes := univs; declarations := [] |}
-    (onu, globenv_nil _ _))
-  (Pcons : forall (Σ : global_env) kn d (wf : wf Σ) 
-    (Hfresh : fresh_global kn Σ.(declarations))
-    (udecl := PCUICLookup.universes_decl_of_decl d)
-    (onud : on_udecl Σ.(universes) udecl)
-    (pd : on_global_decl (lift_typing typing) ({| universes := Σ.(universes); declarations := Σ.(declarations) |}, udecl) kn d),
-    P Σ wf -> P (add_global_decl Σ (kn, d)) 
-    (fst wf, globenv_decl _ Σ.(universes) Σ.(declarations) kn d (snd wf) Hfresh onud pd))
-  (Σ : global_env) (wfΣ : wf Σ) : P Σ wfΣ.
-Proof.
-  destruct Σ as [univs Σ]. destruct wfΣ; cbn in *.
-  induction o0. apply Pnil.
-  apply (Pcons {| universes := univs; declarations := Σ |} kn d (o, o0)).
-  exact IHo0.
-Qed.
-
-Ltac inv_eta :=
-  lazymatch goal with
-  | [ H : PCUICEtaExpand.expanded _ _ |- _ ] => depelim H
-  end.
-
-Fixpoint map_erase (Σ : wf_env_ext) Γ (ts : list term) (H2 : Forall (welltyped Σ Γ) ts) : list E.term.
-destruct ts as [ | t ts].
-- exact [].
-- eapply cons. refine (erase Σ Γ t _). 
-  2: eapply (map_erase Σ Γ ts).
-  all: now inversion H2; subst.
-Defined.
-
-Lemma map_erase_irrel Σ Γ t H1 H2 : map_erase Σ Γ t H1 = map_erase Σ Γ t H2.
-Proof.
-  induction t.
-  - cbn. reflexivity.
-  - cbn. depelim H1; cbn. depelim H2; cbn.
-    f_equal.
-    + eapply erase_irrel.
-    + eapply IHt.
-Qed.
-
-Arguments map_erase _ _ _ _, _ _ _ {_}.
-
-Lemma erase_mkApps {Σ : wf_env_ext} Γ t args H2 Ht Hargs :
-  wf_local Σ Γ ->
-  ~ ∥ isErasable Σ Γ (mkApps t args) ∥ ->
-  erase Σ Γ (mkApps t args) H2 = 
-  E.mkApps (erase Σ Γ t Ht) (map_erase Σ Γ args Hargs).
-Proof.
-  pose proof (referenced_impl_ext_wf Σ) as [wf]. 
-  intros Hwflocal Herasable. induction args in t, H2, Ht, Hargs, Herasable |- *.
-  - cbn. eapply erase_irrel.
-  - cbn [mkApps]. 
-    rewrite IHargs. 
-    1: inversion Hargs; eauto.
-    2: eauto.
-    2:{ intros ? wfΣ'. destruct (H2 _ wfΣ'). cbn in X. eapply inversion_mkApps in X as (? & ? & ?).
-        econstructor. eauto. }
-    intros Happ Hargs'.
-    etransitivity. simp erase. reflexivity. unfold erase_clause_1.
-    unfold inspect. unfold erase_clause_1_clause_2.
-    elim: is_erasableP.
-    + intros. exfalso. 
-      eapply Herasable. destruct p.
-      cbn. destruct (H2 _ eq_refl). eapply Is_type_app; eauto.
-    + cbn [map_erase]. 
-      epose proof (fst (erase_irrel _)). cbn.
-      intros he. f_equal => //. f_equal.
-      eapply erase_irrel. eapply erase_irrel.
-      eapply map_erase_irrel. 
-      Unshelve. cbn in wfΣ'; subst; eauto.  exact Σ.
-Qed.
-
-Lemma map_erase_length Σ Γ t H1 : length (map_erase Σ Γ t H1) = length t.
-Proof.
-  induction t; cbn; f_equal; [ | inversion H1; subst ]; eauto.
-Qed.
-
-Local Hint Constructors expanded : expanded.
-
-Local Arguments erase_global_decls _ _ _ : clear implicits.
-
-(* Lemma make_wf_env_ext_remove_kn kn decl univs decls : *)
-  (* make_wf_env_ext (remove_kn kn (add_global_decl  )) *)
-
-Lemma lookup_env_erase (Σ : wf_env) deps kn d :
-  KernameSet.In kn deps -> 
-  lookup_env Σ kn = Some (InductiveDecl d) ->
-  EGlobalEnv.lookup_env (erase_global deps Σ) kn = Some (EAst.InductiveDecl (erase_mutual_inductive_body d)).
-Proof.
-  intros hin.
-  rewrite /lookup_env. 
-  unfold erase_global.
-  set (e := eq_refl).
-  clearbody e.
-  move: e. generalize (declarations Σ) at 2 3 4.
-  induction g in Σ, deps, hin |- *.
-  - move=> /= //.
-  - intros e. destruct a as [kn' d'].
-    cbn -[erase_global_decls].
-    case: (eqb_spec kn kn'); intros e'; subst.
-    intros [= ->].
-    unfold erase_global_decls.
-    eapply KernameSet.mem_spec in hin. rewrite hin /=.
-    now rewrite eq_kername_refl.
-    intros hl. destruct d'. simpl.
-    destruct KernameSet.mem. cbn.
-    rewrite (negbTE (proj2 (neqb _ _) e')).
-    eapply IHg => //. eapply KernameSet.union_spec. left => //.
-    eapply IHg => //.
-    simpl.
-    destruct KernameSet.mem. cbn.
-    rewrite (negbTE (proj2 (neqb _ _) e')).
-    eapply IHg => //.
-    eapply IHg => //. 
-Qed.
-
-Lemma erase_global_declared_constructor (Σ : wf_env) ind c mind idecl cdecl deps :
-   declared_constructor Σ (ind, c) mind idecl cdecl ->
-   KernameSet.In ind.(inductive_mind) deps -> 
-   EGlobalEnv.declared_constructor (erase_global deps Σ) (ind, c) 
-    (erase_mutual_inductive_body mind) (erase_one_inductive_body idecl) 
-    (EAst.mkConstructor cdecl.(cstr_name) cdecl.(cstr_arity)).
-Proof.
-  intros [[]] Hin.
-  cbn in *. split. split. 
-  - red in H |- *. now eapply lookup_env_erase.
-  - cbn. now eapply map_nth_error.
-  - cbn. erewrite map_nth_error; eauto.
-Qed.
-
-Import EGlobalEnv.
-Lemma erase_global_decls_fresh kn deps Σ decls heq : 
-  let Σ' := erase_global_decls deps Σ decls heq in
-  PCUICTyping.fresh_global kn decls ->
-  fresh_global kn Σ'.
-Proof.
-  cbn.
-  revert deps Σ heq.
-  induction decls; [cbn; auto|].
-  - intros. red. constructor.
-  - destruct a as [kn' d]. intros. depelim H.
-    cbn in H, H0.
-    destruct d as []; simpl; destruct KernameSet.mem.
-    + cbn [EGlobalEnv.closed_env forallb]. cbn.
-      constructor => //. eapply IHdecls => //.
-    + eapply IHdecls => //.
-    + constructor; auto.
-      eapply IHdecls => //.
-    + eapply IHdecls => //.
-Qed.
-
-Lemma erase_global_fresh kn deps Σ : 
-  let Σ' := erase_global deps Σ in
-  PCUICTyping.fresh_global kn Σ.(declarations) ->
-  fresh_global kn Σ'.
-Proof.
-  unfold erase_global.
-  intros fr. now eapply erase_global_decls_fresh.
-Qed.
-
-From MetaCoq.Erasure Require Import EEtaExpandedFix.
-
-Lemma erase_brs_eq Σ Γ p ts wt : 
-  erase_brs Σ Γ p ts wt = map_All (fun br wt => (erase_context (bcontext br), erase Σ _ (bbody br) wt)) ts wt.
-Proof.
-  funelim (map_All _ ts wt); cbn; auto.
-  f_equal => //. f_equal => //. apply erase_irrel.
-  rewrite -H. eapply erase_irrel.
-Qed.
-
-Lemma erase_fix_eq Σ Γ ts wt : 
-  erase_fix Σ Γ ts wt = map_All (fun d wt => 
-    let dbody' := erase Σ _ (dbody d) (fun Σ abs => proj2 (wt Σ abs)) in
-    let dbody' := if isBox dbody' then
-        match d.(dbody) with
-        | tLambda na _ _ => E.tLambda (binder_name na) E.tBox
-        | _ => dbody'
-        end else dbody' 
-    in
-    {| E.dname := d.(dname).(binder_name); E.rarg := d.(rarg); E.dbody := dbody' |}) ts wt.
-Proof.
-  funelim (map_All _ ts wt); cbn; auto.
-  f_equal => //. f_equal => //.
-  rewrite (fst (erase_irrel _) _ _ _ (fun (Σ0 : global_env_ext) (abs : Σ0 = Σ) =>
-    (map_All_obligation_1 x xs h Σ0 abs).p2)).
-  destruct erase => //.
-  rewrite -H. eapply erase_irrel.
-Qed.
-
-Lemma erase_cofix_eq Σ Γ ts wt : 
-  erase_cofix Σ Γ ts wt = map_All (fun d wt => 
-    let dbody' := erase Σ _ (dbody d) wt in
-    {| E.dname := d.(dname).(binder_name); E.rarg := d.(rarg); E.dbody := dbody' |}) ts wt.
-Proof.
-  funelim (map_All _ ts wt); cbn; auto.
-  f_equal => //. f_equal => //.
-  apply erase_irrel.
-  rewrite -H. eapply erase_irrel.
-Qed.
-
-Lemma isConstruct_erase Σ Γ t wt : 
-  ~ (PCUICEtaExpand.isConstruct t || PCUICEtaExpand.isFix t || PCUICEtaExpand.isRel t) ->
-  ~ (isConstruct (erase Σ Γ t wt) || isFix (erase Σ Γ t wt) || isRel (erase Σ Γ t wt)).
-Proof.
-  apply (erase_elim Σ
-    (fun Γ t wt e => ~ (PCUICEtaExpand.isConstruct t || PCUICEtaExpand.isFix t || PCUICEtaExpand.isRel t) -> ~ (isConstruct e || isFix e || isRel e))
-    (fun Γ l awt e => True)
-    (fun Γ p l awt e => True)
-    (fun Γ l awt e => True)
-    (fun Γ l awt e => True)); intros => //. bang.
-Qed.
-
-Lemma apply_expanded Σ Γ Γ' t t' :
-  expanded Σ Γ t -> Γ = Γ' -> t = t' -> expanded Σ Γ' t'.
-Proof. intros; now subst. Qed.
-
-Lemma erases_deps_erase (cf := config.extraction_checker_flags) {Σ : wf_env} univs (wfΣ : ∥ wf_ext (Σ, univs) ∥)
-  (Σ' := make_wf_env_ext Σ univs wfΣ) Γ t 
-  (wt : forall Σ0 : global_env_ext, abstract_env_rel' Σ' Σ0 -> welltyped Σ0 Γ t) :
-  let et := erase Σ' Γ t wt in
-  let deps := EAstUtils.term_global_deps et in
-  erases_deps Σ (erase_global deps Σ) et.
-Proof.
-  intros et deps. destruct wfΣ.
-  pose proof (wt Σ' eq_refl). destruct H.
-  eapply (erase_global_erases_deps w); tea.
-  eapply (erases_erase (Σ := Σ') (Γ := Γ)).
-  eapply erase_global_includes.
-  intros.
-  eapply term_global_deps_spec in H; eauto.
-  assumption.
-  eapply (erases_erase (Σ := Σ') (Γ := Γ)).
-  eapply KernameSet.subset_spec. reflexivity. 
-Qed.
-
-Lemma erases_deps_erase_weaken (cf := config.extraction_checker_flags) {Σ : wf_env} univs
-  (wfΣ : ∥ wf_ext (Σ, univs) ∥) Γ
-  (Σ' := make_wf_env_ext Σ univs wfΣ) t 
-  (wt : forall Σ0 : global_env_ext, abstract_env_rel' Σ' Σ0 -> welltyped Σ0 Γ t) 
-  deps :
-  let et := erase Σ' Γ t wt in
-  let tdeps := EAstUtils.term_global_deps et in
-  erases_deps Σ (erase_global (KernameSet.union deps tdeps) Σ) et.
-Proof.
-  intros et tdeps. destruct wfΣ.
-  pose proof (wt Σ' eq_refl). destruct H.
-  eapply (erase_global_erases_deps w); tea.
-  eapply (erases_erase (Σ := Σ') (Γ := Γ)).
-  eapply erase_global_includes.
-  intros.
-  eapply term_global_deps_spec in H; eauto.
-  assumption.
-  eapply (erases_erase (Σ := Σ') (Γ := Γ)).
-  eapply KernameSet.subset_spec. intros x hin. eapply KernameSet.union_spec. now right.
-Qed.
-
-Lemma eta_expand_erase {Σ : wf_env_ext} Σ' {Γ t} 
-  (wt : forall Σ0 : global_env_ext, abstract_env_rel' Σ Σ0 -> welltyped Σ0 Γ t) Γ' :
-  PCUICEtaExpand.expanded Σ Γ' t ->
-  erases_global Σ Σ' ->
-  expanded Σ' Γ' (@erase Σ Γ t wt).
-Proof.
-  pose proof (referenced_impl_ext_wf Σ) as [wf]. 
-  intros exp deps.
-  eapply expanded_erases. apply wf.
-  eapply erases_erase. assumption.
-  pose proof (wt Σ eq_refl). destruct H as [T ht].
-  eapply erases_global_erases_deps; tea.
-  eapply erases_erase.
-Qed.
-
-Lemma erase_global_closed Σ deps :
-  let Σ' := erase_global deps Σ in
-  EGlobalEnv.closed_env Σ'.
-Proof.
-  sq.
-  unfold erase_global.
-  set (decls := declarations Σ).
-  set (e := eq_refl). clearbody e.
-  unfold decls at 1 in e. clearbody decls.
-  revert Σ e deps.
-  induction decls; [cbn; auto|].
-  intros Σ e deps.
-  destruct Σ.(referenced_impl_wf).
-  destruct a as [kn d].
-  destruct d as []; simpl; destruct KernameSet.mem.
-  assert (wfs : PCUICTyping.wf {| universes := Σ.(universes); declarations := decls |}).
-  { depelim X. rewrite e in o0. depelim o0; now split. }
-  + cbn [EGlobalEnv.closed_env forallb]. cbn.
-    rewrite [forallb _ _](IHdecls) // andb_true_r.
-    rewrite /test_snd /EGlobalEnv.closed_decl /=.
-    set (er := erase_global_decls_obligation_1 _ _ _ _ _ _ _).
-    set (er' := erase_global_decls_obligation_2 _ _ _ _ _ _ _).
-    clearbody er er'.
-    destruct c as [ty [] univs]; cbn.
-    set (obl := erase_constant_body_obligation_1 _ _ _ _ _).
-    set (wfe := make_wf_env_ext _ _ _).
-    unfold erase_constant_body. cbn. clearbody obl.
-    2:auto.
-    unshelve epose proof (erases_erase (Σ := wfe) obl); eauto.
-    cbn in H.
-    eapply erases_closed in H => //.
-    cbn. destruct (obl _ eq_refl). clear H. now eapply PCUICClosedTyp.subject_closed in X0.
-  + eapply IHdecls => //.
-  + cbn [EGlobalEnv.closed_env forallb].
-    rewrite {1}/test_snd {1}/EGlobalEnv.closed_decl /=.
-    eapply IHdecls => //.
-  + eapply IHdecls => //.
-Qed.
-
-Import EWellformed.
-
-Section wffix.
-  Import EAst.
-  Fixpoint wf_fixpoints (t : term) : bool :=
-    match t with
-    | tRel i => true
-    | tEvar ev args => List.forallb (wf_fixpoints) args
-    | tLambda N M => wf_fixpoints M
-    | tApp u v => wf_fixpoints u && wf_fixpoints v
-    | tLetIn na b b' => wf_fixpoints b && wf_fixpoints b'
-    | tCase ind c brs => 
-      let brs' := forallb (wf_fixpoints ∘ snd) brs in
-      wf_fixpoints c && brs'
-    | tProj p c => wf_fixpoints c
-    | tFix mfix idx => 
-      (idx <? #|mfix|) && List.forallb (fun d => (isLambda d.(dbody) || isBox d.(dbody)) && wf_fixpoints d.(dbody)) mfix
-    | tCoFix mfix idx =>
-      (idx <? #|mfix|) && List.forallb (wf_fixpoints ∘ dbody) mfix
-    | tConst kn => true
-    | tConstruct ind c => true
-    | tVar _ => true
-    | tBox => true
-    end.
-
-End wffix.
-
-Lemma erases_deps_wellformed (cf := config.extraction_checker_flags) (efl := all_env_flags) {Σ} {Σ'} et :
-  erases_deps Σ Σ' et ->
-  forall n, ELiftSubst.closedn n et ->
-  wf_fixpoints et ->
-  wellformed Σ' n et.
-Proof.
-  intros ed.
-  induction ed using erases_deps_forall_ind; intros => //; 
-   try solve [cbn in *; unfold wf_fix in *; rtoProp; intuition eauto; solve_all].
-  - cbn. red in H0. rewrite H0 //.
-  - cbn -[lookup_constructor].
-    cbn. now destruct H0 as [[-> ->] ->].
-  - cbn in *. move/andP: H5 => [] cld clbrs.
-    cbn. apply/andP; split. apply/andP; split. 
-    * now destruct H0 as [-> ->].
-    * now move/andP: H6.
-    * move/andP: H6; solve_all.
-  - cbn -[lookup_projection] in *. apply/andP; split; eauto.
-    now rewrite (declared_projection_lookup H0).
-Qed.
-
-Lemma erases_wf_fixpoints Σ Γ t t' : Σ;;; Γ |- t ⇝ℇ t' -> 
-  ErasureProperties.wellformed Σ t -> wf_fixpoints t'.
-Proof.
-  induction 1 using erases_forall_list_ind; cbn; auto; try solve [rtoProp; repeat solve_all].
-  - move/andP => []. rewrite (All2_length X) => -> /=. unfold test_def in *.
-    eapply Forall2_All2 in H.
-    eapply All2_All2_mix in X; tea. solve_all.
-    destruct b0; eapply erases_isLambda in H1; tea.
-  - move/andP => []. rewrite (All2_length X) => -> /=.
-    unfold test_def in *. solve_all.
-Qed.
-
-Lemma erase_wf_fixpoints (efl := all_env_flags) {Σ : wf_env} univs wfΣ {Γ t} wt
-  (Σ' := make_wf_env_ext Σ univs wfΣ) :
-  let t' := erase Σ' Γ t wt in
-  wf_fixpoints t'.
-Proof.
-  cbn.
-  eapply erases_wf_fixpoints.
-  eapply erases_erase.
-  specialize (wt (Σ, univs) eq_refl).
-  destruct wfΣ.
-  now unshelve eapply welltyped_wellformed in wt. 
-Qed.
-
-Lemma erase_wellformed (efl := all_env_flags) {Σ : wf_env} univs wfΣ {Γ t} wt
-  (Σ' := make_wf_env_ext Σ univs wfΣ) :
-  let t' := erase Σ' Γ t wt in
-  wellformed (erase_global (term_global_deps t') Σ) #|Γ| t'.
-Proof.
-  set (t' := erase _ _ _ _).
-  cbn.
-  epose proof (@erases_deps_erase Σ univs wfΣ Γ t wt).
-  cbn in H.
-  epose proof (erases_deps_wellformed _ H #|Γ|).
-  apply H0.
-  eapply (erases_closed _ Γ).
-  destruct (wt _ eq_refl).
-  cbn in X. destruct wfΣ.
-  now eapply PCUICClosedTyp.subject_closed in X.
-  eapply erases_erase.
-  eapply erase_wf_fixpoints.
-Qed.
-
-Lemma erase_wellformed_weaken (efl := all_env_flags) {Σ : wf_env} univs wfΣ {Γ t} wt deps
-  (Σ' := make_wf_env_ext Σ univs wfΣ) :
-  let t' := erase Σ' Γ t wt in
-  wellformed (erase_global (KernameSet.union deps (term_global_deps t')) Σ) #|Γ| t'.
-Proof.
-  set (t' := erase _ _ _ _).
-  cbn.
-  epose proof (@erases_deps_erase_weaken Σ univs wfΣ Γ t wt deps).
-  cbn in H.
-  epose proof (erases_deps_wellformed _ H #|Γ|).
-  apply H0.
-  eapply (erases_closed _ Γ).
-  - destruct (wt _ eq_refl).
-    cbn in X. destruct wfΣ.
-    now eapply PCUICClosedTyp.subject_closed in X.
-  - eapply erases_erase.
-  - eapply erase_wf_fixpoints.
-Qed.
-
-Lemma erase_constant_body_correct'' {Σ : wf_env} {cb} {univs wfΣ}
-(Σ' := make_wf_env_ext Σ univs wfΣ)
-{onc : ∥ on_constant_decl (lift_typing typing) Σ' cb ∥} {body} deps :  
-  EAst.cst_body (fst (erase_constant_body Σ' cb onc)) = Some body ->
-  ∥ ∑ t T, (Σ' ;;; [] |- t : T) * (Σ' ;;; [] |- t ⇝ℇ body) *
-      (term_global_deps body = snd (erase_constant_body Σ' cb onc)) *
-      wellformed (efl:=all_env_flags) (erase_global (KernameSet.union deps (term_global_deps body)) Σ) 0 body ∥.
-Proof.
-  intros. destruct cb as [name [bod|] udecl]; simpl. intros.
-  simpl in H. noconf H.
-  set (obl :=(erase_constant_body_obligation_1 Σ'
-  {|
-  cst_type := name;
-  cst_body := Some bod;
-  cst_universes := udecl |} onc bod eq_refl)). clearbody obl.
-  assert (wfΣ' : abstract_env_rel' Σ' Σ') by reflexivity.
-  destruct (obl _ wfΣ'). sq.
-  have er : (Σ, univs);;; [] |- bod ⇝ℇ erase (make_wf_env_ext Σ univs (sq wfΣ)) [] bod obl.
-  { eapply (erases_erase (Σ:=Σ')). }
-  exists bod, A; intuition auto. eapply erase_wellformed_weaken.
-  now simpl in H.
-Qed.
-
-Lemma erase_global_cst_decl_wf_glob Σ deps decls heq :
-  forall cb wfΣ hcb,
-  let ecb := erase_constant_body (make_wf_env_ext Σ (cst_universes cb) wfΣ) cb hcb in
-  let Σ' := erase_global_decls (KernameSet.union deps ecb.2) Σ decls heq in
-  @wf_global_decl all_env_flags Σ' (EAst.ConstantDecl ecb.1).
-Proof.
-  intros cb wfΣ hcb.
-  set (ecb := erase_constant_body _ _ _). cbn.
-  unfold wf_global_decl. cbn.
-  destruct wfΣ, hcb. red in o.
-  destruct EAst.cst_body eqn:hb => /= //. subst decls.
-  eapply (erase_constant_body_correct'') in hb.
-  destruct hb. destruct X as [t0 [T [[] ?]]].
-  set(Σext := make_wf_env_ext _ _ _) in *.
-  destruct p. rewrite e in i. exact i.  
-Qed.
-
-Lemma erase_global_ind_decl_wf_glob {Σ : wf_env} {deps decls kn m} (heq : declarations Σ = decls) :
-  on_inductive (lift_typing typing) (Σ, ind_universes m) kn m ->
-  let m' := erase_mutual_inductive_body m in
-  let Σ' := erase_global_decls deps Σ decls heq in
-  @wf_global_decl all_env_flags Σ' (EAst.InductiveDecl m').
-Proof.
-  set (m' := erase_mutual_inductive_body m).
-  set (Σ' := erase_global_decls _ _ _ _). simpl.
-  intros oni.
-  pose proof (referenced_impl_wf Σ) as [wfΣ].
-  assert (erases_mutual_inductive_body m (erase_mutual_inductive_body m)).
-  { eapply (erases_mutual (mdecl:=kn)); tea. }
-  eapply (erases_mutual_inductive_body_wf (univs := Σ.(universes)) (Σ := decls) (kn := kn) (Σ' := Σ')) in H; tea.
-  simpl. rewrite -heq.
-  destruct Σ ; cbn in *.
-  destruct wf_env_referenced; cbn in *.
-  now destruct referenced_impl_env; cbn in *.
-Qed.
-
-Lemma erase_global_decls_wf_glob Σ deps decls heq :
-  let Σ' := erase_global_decls deps Σ decls heq in
-  @wf_glob all_env_flags Σ'.
-Proof.
-  cbn.
-  revert deps Σ heq.
-  induction decls; [cbn; auto|].
-  { intros. constructor. }
-  intros. destruct a as [kn []]; simpl; destruct KernameSet.mem.
-  + constructor. eapply IHdecls => //. eapply erase_global_cst_decl_wf_glob; auto.
-    eapply erase_global_decls_fresh; auto.
-    destruct Σ.(referenced_impl_wf).
-    destruct X. rewrite heq in o0. now depelim o0.
-  + cbn.
-    eapply IHdecls.
-  + constructor. eapply IHdecls.
-    destruct Σ.(referenced_impl_wf) as [[onu ond]].
-    rewrite heq in ond. depelim ond.
-    eapply (erase_global_ind_decl_wf_glob (kn:=kn)); tea.
-    eapply erase_global_decls_fresh.
-    destruct Σ.(referenced_impl_wf) as [[onu ond]].
-    rewrite heq in ond. now depelim ond.
-  + eapply IHdecls.
-Qed.
-
-Lemma erase_global_wf_glob Σ deps :
-  let Σ' := erase_global deps Σ in
-  @wf_glob all_env_flags Σ'.
-Proof. eapply erase_global_decls_wf_glob. Qed.
-
-
-Lemma lookup_erase_global (cf := config.extraction_checker_flags) {Σ : wf_env} {deps deps'} :
-  KernameSet.Subset deps deps' ->
-  EExtends.global_subset (erase_global deps Σ) (erase_global deps' Σ).
-Proof.
-  unfold erase_global.
-  destruct Σ as [[[univs Σ] wfΣ G wfG] map repr]. cbn in *. clear G wfG.
-  revert deps deps' wfΣ map repr.
-  induction Σ. cbn => //.
-  intros deps deps' wfΣ map repr sub.
-  destruct a as [kn' []]; cbn;
-  (set (decl := E.ConstantDecl _) || set (decl := E.InductiveDecl _)); hidebody decl;
-  set (eg := erase_global_decls _ _ _ _); hidebody eg;
-  set (eg' := erase_global_decls _ _ _ _); hidebody eg';
-  try (set (eg'' := erase_global_decls _ _ _ _); hidebody eg'');
-  try (set (eg''' := erase_global_decls _ _ _ _); hidebody eg''').
-  { destruct (KernameSet.mem) eqn:knm => /=.
-    + eapply KernameSet.mem_spec, sub, KernameSet.mem_spec in knm. rewrite knm.
-      apply EExtends.global_subset_cons. eapply IHΣ.
-      intros x hin. eapply KernameSet.union_spec in hin.
-      eapply KernameSet.union_spec. destruct hin. left. now eapply sub.
-      right => //.
-    + destruct (KernameSet.mem kn' deps') eqn:eq'.
-      eapply EExtends.global_subset_cons_right.
-      eapply erase_global_wf_glob.
-      unfold decl. unfold hidebody.
-      constructor. eapply erase_global_wf_glob.
-      eapply erase_global_cst_decl_wf_glob.
-      depelim wfΣ. depelim w. cbn in o0. depelim o0.
-      eapply erase_global_decls_fresh => //.
-      unfold eg', eg''. unfold hidebody.
-      eapply IHΣ.
-      intros x hin.
-      eapply KernameSet.union_spec. left. now eapply sub.
-      eapply IHΣ => //. }
-  { destruct (KernameSet.mem) eqn:knm => /=.
-    + eapply KernameSet.mem_spec, sub, KernameSet.mem_spec in knm. rewrite knm.
-      apply EExtends.global_subset_cons. eapply IHΣ => //.
-    + destruct (KernameSet.mem kn' deps') eqn:eq'.
-      eapply EExtends.global_subset_cons_right. eapply erase_global_wf_glob.
-      constructor. eapply erase_global_wf_glob.
-      depelim wfΣ.
-      eapply (erase_global_ind_decl_wf_glob (kn:=kn')). cbn.
-      depelim w. now depelim o0.
-      eapply erase_global_decls_fresh => //.
-      clear -wfΣ. destruct wfΣ. destruct X as [onu ond]; cbn in *. now depelim ond.
-      eapply IHΣ. intros x hin. now eapply sub.
-      eapply IHΣ => //. }
-Qed.
-
-Lemma expanded_weakening_global Σ deps deps' Γ t : 
-  KernameSet.Subset deps deps' ->
-  expanded (erase_global deps Σ) Γ t ->
-  expanded (erase_global deps' Σ) Γ t.
-Proof.
-  intros hs.
-  eapply expanded_ind; intros; try solve [econstructor; eauto].
-  - eapply expanded_tFix; tea. solve_all.
-  - eapply expanded_tConstruct_app; tea.
-    destruct H. split; tea.
-    destruct d; split => //.
-    cbn in *. red in H.
-    eapply lookup_erase_global in H; tea.
-Qed.
-
-Lemma expanded_erase (cf := config.extraction_checker_flags) {Σ : wf_env} univs wfΣ t wtp :
-  PCUICEtaExpand.expanded Σ [] t ->
-  let Σ' := make_wf_env_ext Σ univs wfΣ in
-  let et := (erase Σ' [] t wtp) in
-  let deps := EAstUtils.term_global_deps et in
-  expanded (erase_global deps Σ) [] et.
-Proof.
-  intros hexp Σ'.
-  have [wf] : ∥ wf Σ ∥.
-  { destruct wfΣ. sq. exact w. }
-  eapply (expanded_erases (Σ := (Σ, univs))); tea.
-  eapply (erases_erase (Σ := Σ')). cbn.
-  eapply (erases_deps_erase (Σ := Σ) univs wfΣ).
-Qed.
-
-Lemma expanded_erase_global (cf := config.extraction_checker_flags) deps {Σ: wf_env} :
-  PCUICEtaExpand.expanded_global_env Σ ->
-  expanded_global_env (erase_global deps Σ).
-Proof.
-  intros etaΣ.
-  unfold erase_global.
-  destruct Σ as [Σ map repr]. cbn in *.
-  destruct Σ as [Σ wfΣ G isG]. cbn in *. clear G isG.
-  destruct Σ as [univs Σ]; cbn in *.
-  red. revert wfΣ. red in etaΣ. cbn in *.
-  revert deps map repr.
-  induction etaΣ; intros deps. cbn. constructor.
-  destruct decl as [kn []];
-  destruct (KernameSet.mem kn deps) eqn:eqkn; simpl; rewrite eqkn.
-  constructor; [eapply IHetaΣ; auto|].
-  red. cbn. red. cbn in *.
-  set (deps' := KernameSet.union _ _). hidebody deps'.
-  set (wfext := make_wf_env_ext _ _ _). hidebody wfext.
-  destruct H.
-  destruct c as [cst_na [cst_body|] cst_type cst_rel].
-  cbn in *.
-  eapply expanded_weakening_global. 
-  2:{ eapply expanded_erase; tea. }
-  set (et := erase _ _ _ _) in *.
-  unfold deps'. unfold hidebody. intros x hin.    
-  eapply KernameSet.union_spec. right => //.
-  now cbn.
-  intros.
-  eapply IHetaΣ.
-  intros map repr wfΣ.
-  constructor. eapply IHetaΣ.
-  red. cbn => //.
-  intros map repr wfΣ.
-  eapply IHetaΣ.
-Qed.
-
-(* Sanity checks: the [erase] function maximally erases terms *)
-Lemma erasable_tBox_value (wfl := Ee.default_wcbv_flags) (Σ : global_env_ext) (wfΣ : wf_ext Σ) t T v :
-  forall wt : Σ ;;; [] |- t : T,
-  Σ |-p t ▷ v -> erases Σ [] v E.tBox -> ∥ isErasable Σ [] t ∥.
-Proof.
-  intros.
-  depind H.
-  eapply Is_type_eval_inv; eauto. eexists; eauto.
-Qed.
-
-Lemma erase_eval_to_box (wfl := Ee.default_wcbv_flags) {Σ : wf_env} {univs wfext t v Σ' t' deps} :
-  let Σext := make_wf_env_ext Σ univs wfext in
-  forall wt : forall Σ0 : global_env_ext, abstract_env_rel' Σext Σ0 -> welltyped Σ0 [] t,
-  erase Σext [] t wt = t' ->
-  KernameSet.subset (term_global_deps t') deps ->
-  erase_global deps Σ = Σ' ->
-  PCUICWcbvEval.eval Σ t v ->
-  @Ee.eval Ee.default_wcbv_flags Σ' t' E.tBox -> ∥ isErasable Σext [] t ∥.
-Proof.
-  intros Σext wt.
-  intros.
-  destruct (erase_correct Σ univs wfext _ _ _ _ _ wt H H0 H1 X) as [ev [eg [eg']]].
-  pose proof (Ee.eval_deterministic H2 eg'). subst.
-  destruct wfext. destruct (wt _ eq_refl) as [T wt'].
-  eapply erasable_tBox_value; eauto.
-Qed.
-
-Lemma erase_eval_to_box_eager (wfl := Ee.default_wcbv_flags) {Σ : wf_env} {univs wfext t v Σ' t' deps} :
-  let Σext := make_wf_env_ext Σ univs wfext in
-  forall wt : forall Σ0 : global_env_ext, abstract_env_rel' Σext Σ0 -> welltyped Σ0 [] t,
-  erase Σext [] t wt = t' ->
-  KernameSet.subset (term_global_deps t') deps ->
-  erase_global deps Σ = Σ' ->
-  PCUICWcbvEval.eval Σ t v ->
-  @Ee.eval Ee.default_wcbv_flags Σ' t' E.tBox -> t' = E.tBox.
-Proof.
-  intros Σext wt.
-  intros.
-  destruct (erase_eval_to_box wt H H0 H1 X H2).
-  subst t'.
-  destruct (inspect_bool (is_erasableb Σext [] t wt)) eqn:heq.
-  - simp erase. rewrite heq.
-    simp erase => //.
-  - elimtype False.
-    destruct (@is_erasableP Σext [] t wt) => //. apply n. now sq.
-Qed.
-
-Section EraseGlobalFast.
-
-  Import PCUICEnvironment.
-
-Definition decls_prefix decls (Σ' : global_env) := 
-  ∑ Σ'', declarations Σ' = Σ'' ++ decls.
-
-Lemma on_global_decls_prefix {cf} P univs decls decls' :
-  on_global_decls P univs (decls ++ decls') ->
-  on_global_decls P univs decls'.
-Proof.
-  induction decls => //.
-  intros ha; depelim ha.
-  now apply IHdecls.
-Qed.
-
-Lemma decls_prefix_wf {decls Σ} : 
-  decls_prefix decls Σ -> wf Σ -> wf {| universes := Σ.(universes); declarations := decls |}.
-Proof.
-  intros [Σ' hd] wfΣ.
-  split. apply wfΣ.
-  cbn. destruct wfΣ as [_ ond]. rewrite hd in ond.
-  now eapply on_global_decls_prefix in ond.
-Qed.
-
-Lemma weaken_prefix {decls Σ kn decl} :
-  decls_prefix decls Σ ->
-  wf Σ -> 
-  lookup_env {| universes := Σ; declarations := decls |} kn = Some decl ->
-  on_global_decl (lift_typing typing) (Σ, universes_decl_of_decl decl) kn decl.
-Proof.
-  intros prefix wfΣ.
-  have wfdecls := decls_prefix_wf prefix wfΣ.
-  epose proof (weakening_env_lookup_on_global_env (lift_typing typing) _ Σ kn decl 
-    weaken_env_prop_typing wfdecls wfΣ).
-  forward X. red; split => //. cbn. apply incl_cs_refl.
-  now apply (X wfdecls).
-Qed.
-
-(* This version of global environment erasure keeps the same global environment throughout the whole 
-   erasure, while folding over the list of declarations. *)
-
-Program Fixpoint erase_global_decls_fast (deps : KernameSet.t) (Σ : wf_env) (decls : global_declarations) 
-  (prop : ∥ decls_prefix decls Σ.(referenced_impl_env) ∥) : E.global_declarations :=
-  match decls with
-  | [] => []
-  | (kn, ConstantDecl cb) :: decls =>
-    if KernameSet.mem kn deps then
-      let wfΣext' := make_wf_env_ext Σ (cst_universes cb) _ in
-      let cb' := erase_constant_body wfΣext' cb _ in
-      let deps := KernameSet.union deps (snd cb') in
-      let Σ' := erase_global_decls_fast deps Σ decls _ in
-      ((kn, E.ConstantDecl (fst cb')) :: Σ')
-    else
-      erase_global_decls_fast deps Σ decls _
-
-  | (kn, InductiveDecl mib) :: decls =>
-    if KernameSet.mem kn deps then
-      let mib' := erase_mutual_inductive_body mib in
-      let Σ' := erase_global_decls_fast deps Σ decls _ in
-      ((kn, E.InductiveDecl mib') :: Σ')
-    else erase_global_decls_fast deps Σ decls _
-  end.
-Next Obligation.
-  epose proof Σ.(referenced_impl_wf).
-  sq. split. cbn. apply H. cbn.
-  eapply decls_prefix_wf in prop as [onu ond]; tea. cbn in ond.
-  now depelim ond.
-Qed.
-Next Obligation.
-  epose proof Σ.(referenced_impl_wf).
-  sq. eapply (weaken_prefix (kn := kn)) in prop; tea.
-  2:{ cbn. rewrite eqb_refl //. }
-  apply prop.
-Qed.
-Next Obligation.
-  sq. red. destruct prop as [Σ' ->].
-  eexists (Σ' ++ [(kn, ConstantDecl cb)]); rewrite -app_assoc //.
-Qed.
-Next Obligation.
-  sq. red. destruct prop as [Σ' ->].
-  eexists (Σ' ++ [(kn, ConstantDecl cb)]); rewrite -app_assoc //.
-Qed.
-Next Obligation.
-  sq. red. destruct prop as [Σ' ->].
-  eexists (Σ' ++ [(kn, _)]); rewrite -app_assoc //.
-Qed.
-Next Obligation.
-  sq. red. destruct prop as [Σ' ->].
-  eexists (Σ' ++ [(kn, _)]); rewrite -app_assoc //.
-Qed.
-
-Import PCUICAst PCUICEnvironment.
-
-Lemma wf_lookup Σ kn d suffix g : 
-  wf Σ ->
-  declarations Σ = suffix ++ (kn, d) :: g ->
-  lookup_env Σ kn = Some d.
-Proof.
-  unfold lookup_env.
-  intros [_ ond] eq. rewrite eq in ond |- *.
-  move: ond; clear.
-  induction suffix.
-  - cbn. rewrite eqb_refl //.
-  - cbn. intros ond.
-    depelim ond. cbn. red in f.
-    eapply Forall_app in f as []. depelim H0. cbn in H0.
-    destruct (eqb_spec kn kn0); [contradiction|].
-    now apply IHsuffix.
-Qed.
-
-Definition add_suffix suffix Σ :=
-  {| universes := Σ.(universes); declarations := suffix ++ Σ.(declarations) |}.
-
-Lemma add_suffix_cons d suffix Σ : add_suffix (d :: suffix) Σ = add_global_decl (add_suffix suffix Σ) d. 
-Proof. reflexivity. Qed.
-
-Lemma global_erased_with_deps_weaken_prefix suffix Σ Σ' kn : 
-  wf (add_suffix suffix Σ) ->
-  global_erased_with_deps Σ Σ' kn ->
-  global_erased_with_deps (add_suffix suffix Σ) Σ' kn.
-Proof.
-  induction suffix.
-  - unfold add_suffix; cbn. intros wf hg.
-    now rewrite -eta_global_env.
-  - rewrite add_suffix_cons. intros wf H.
-    destruct a as [kn' d]. eapply global_erases_with_deps_weaken => //.
-    apply IHsuffix => //.
-    destruct wf as [onu ond]. now depelim ond.
-Qed.
-
-Definition build_wf_env_from_env {cf : checker_flags} (Σ : global_env) (wfΣ : ∥ PCUICTyping.wf Σ ∥) : wf_env := 
-  let Σm := EnvMap.of_global_env Σ.(declarations) in
-  {| wf_env_referenced := {| referenced_impl_env := Σ; referenced_impl_wf := wfΣ |} ;
-     wf_env_map := Σm;
-     wf_env_map_repr := EnvMap.repr_global_env Σ.(declarations);
- |}.
-
-(* Using weakening it is trivial to show that a term found to be erasable in Σ 
-  will be found erasable in any well-formed extension. The converse is not so trivial:
-  some valid types in the extension are not valid in the restricted global context.
-  So, we will rather show that the erasure function is invariant under extension. *) 
-
-Lemma isErasable_irrel_global_env {Σ Σ' : global_env_ext} {Γ t} :
-  wf Σ ->
-  extends_decls Σ' Σ ->
-  Σ.2 = Σ'.2 ->
-  isErasable Σ' Γ t -> isErasable Σ Γ t.
-Proof.
-  unfold isErasable.
-  intros wfΣ ext eqext [T [ht isar]].
-  destruct Σ as [Σ decl], Σ' as [Σ' decl']. cbn in eqext; subst decl'.
-  exists T; split.
-  eapply (env_prop_typing weakening_env (Σ', decl)) => //=.
-  eapply extends_decls_wf; tea.
-  now eapply extends_decls_extends.
-  destruct isar as [|s]; [left|right] => //.
-  destruct s as [u [Hu isp]].
-  exists u; split => //.
-  eapply (env_prop_typing weakening_env (Σ', decl)) => //=.
-  eapply extends_decls_wf; tea.
-  now eapply extends_decls_extends.
-Qed. 
 
 (** As erasure relies on reduction of types to check the erasability of types and proofs, we also show 
   that safe reduction is invariant under extension.
@@ -2284,14 +795,6 @@ Definition same_principal_type {cf}
   {Γ : context} {t} (p : PCUICSafeRetyping.principal_type X_type X Γ t) (p' : PCUICSafeRetyping.principal_type X_type' X' Γ t) :=
   p.π1 = p'.π1.
 
-Definition Hlookup {cf} (X_type : abstract_env_ext_impl) (X : X_type.π1)
-  (X_type' : abstract_env_ext_impl) (X' : X_type'.π1) := 
-  forall Σ : global_env_ext, abstract_env_ext_rel X Σ ->
-  forall Σ' : global_env_ext, abstract_env_ext_rel X' Σ' ->
-  forall kn decl decl',
-    lookup_env Σ kn = Some decl ->
-    lookup_env Σ' kn = Some decl' ->
-    abstract_env_lookup X kn = abstract_env_lookup X' kn.
 
 Lemma welltyped_mkApps_inv {cf} {Σ : global_env_ext} Γ f args :  ∥ wf Σ ∥ ->
   welltyped Σ Γ (mkApps f args) -> welltyped Σ Γ f /\ Forall (welltyped Σ Γ) args.
@@ -2319,7 +822,7 @@ Section infer_irrel.
     : same_prod Γ pf pf' -> pf.π2.π2.π1 = pf'.π2.π2.π1.
   Proof.
     destruct pf as [na [A [B prf]]].
-    destruct pf' as [na' [A' [B' prf']]].
+    destruct pf' as [na' [A' []]].
     cbn. congruence.
   Qed.
   
@@ -2734,7 +1237,7 @@ Proof.
     { unfold t', t''. apply H; eauto. }
     clearbody t''. clearbody obl1 obl2. clearbody t'.
     destruct t', t''. cbn in H0. subst x0. cbn.
-    eapply same_prod_last => //.
+    eapply same_prod_last; eauto.
     now eapply infer_as_prod_irrel.
   - unfold infer. rewrite Heq /= //.
   - assert (abstract_env_lookup X cst = abstract_env_lookup X' cst).
@@ -2761,11 +1264,11 @@ Proof.
       epose proof (abstract_env_ext_wf X' wfΣ') as [hwfΣ'].
       destruct (wi' _ wfΣ'). inv X0.
       pose proof (hd _ wfΣ).
-      destruct isdecl, H0.
+      destruct isdecl, H.
       unfold declared_minductive in *.
-      now eapply (hl Σ wfΣ Σ' wfΣ'). }        
+      now eapply (hl Σ wfΣ Σ' wfΣ').  }        
     destruct (PCUICSafeReduce.inspect (lookup_ind_decl _ X' ind)).
-    generalize (same_lookup_ind_decl hl _ H). rewrite -{1}e0 -{1}e.
+    generalize (same_lookup_ind_decl hl ind H). rewrite -{1}e0 -{1}e.
     destruct x => //. cbn. cbn.
     destruct a as [decl' [body' ?]]; cbn.
     congruence.
@@ -2778,8 +1281,8 @@ Proof.
       epose proof (abstract_env_ext_wf X' wfΣ') as [hwfΣ'].
       destruct (wi' _ wfΣ'). inv X0.
       pose proof (wt _ wfΣ).
-      destruct isdecl, H0. inv X0.
-      destruct H1. destruct isdecl as [[] ?].
+      destruct isdecl, H. inv X0.
+      destruct H0. destruct isdecl as [[] ?].
       unfold declared_minductive in *.
       now eapply (hl Σ wfΣ Σ' wfΣ'). }        
     destruct (PCUICSafeReduce.inspect (lookup_ind_decl _ X' ind)).
@@ -2821,7 +1324,7 @@ Proof.
       epose proof (abstract_env_ext_wf X' wfΣ') as [hwfΣ'].
       destruct (wi' _ wfΣ'). inv X0.
       pose proof (wt _ wfΣ).
-      inv H1. inv X0. destruct H as [[[]]]. destruct H1 as [[[]]].
+      inv H. inv X0. destruct H1 as [[[]]]. destruct H2 as [[[]]].
       unfold declared_minductive in *.
       now eapply (hl Σ wfΣ Σ' wfΣ'). } 
     generalize (same_lookup_ind_decl hl _ H). rewrite -{1}eq -{1}e.
@@ -2883,13 +1386,13 @@ Proof.
   cbn. bang.
 Qed.
 
-(* From here on we are not abstract on the environment *)
-Lemma is_arity_irrel {Σ Σ' : wf_env_ext} {Γ h h' t wt wt'} : 
-  Hlookup optimized_abstract_env_ext_impl Σ optimized_abstract_env_ext_impl Σ' ->
-  is_arity Σ Γ h t wt = is_arity Σ' Γ h' t wt'.
+Lemma is_arity_irrel {X_type : abstract_env_ext_impl} {X : X_type.π1}
+  {X_type' : abstract_env_ext_impl} {X' : X_type'.π1} {Γ h h' t wt wt'} : 
+  Hlookup X_type X X_type' X' ->
+  is_arity X_type X Γ h t wt = is_arity X_type' X' Γ h' t wt'.
 Proof.
   intros hl.
-  funelim (is_arity Σ _ _ _ _).
+  funelim (is_arity X_type X _ _ _ _).
   - epose proof (reduce_to_sort_irrel hl eq_refl HT wt').
     rewrite -rsort in H1.
     simp is_arity.
@@ -2899,7 +1402,7 @@ Proof.
     destruct x => //.
   - epose proof (reduce_to_sort_irrel hl eq_refl HT wt').
     rewrite -rsort in H3.
-    rewrite [is_arity Σ' _ _ _ _]is_arity_equation_1.
+    rewrite [is_arity X_type' X' _ _ _ _]is_arity_equation_1.
     epose proof (reduce_to_sort_irrel hl eq_refl HT wt').
     destruct (PCUICSafeReduce.inspect) eqn:hi.
     rewrite -rsort -e in H4.
@@ -2925,104 +1428,101 @@ Proof.
     destruct x => //.
 Qed.
 
-Lemma extends_lookup_env {cf Σ Σ' kn d} : wf Σ' -> extends_decls Σ Σ' -> 
-  lookup_env Σ kn = Some d -> lookup_env Σ' kn = Some d.
+  Lemma extends_lookup_env {cf Σ Σ' kn d} : wf Σ' -> extends_decls Σ Σ' -> 
+    lookup_env Σ kn = Some d -> lookup_env Σ' kn = Some d.
+  Proof.
+    destruct Σ as [univs Σ].
+    destruct Σ' as [univs' Σ'].
+    intros wf [Σ'' []]. cbn in *. subst univs'.
+    induction x in Σ, Σ', e, wf |- *. cbn in e. now subst Σ'.
+    intros hl.
+    rewrite e; cbn. 
+    case: eqb_spec.
+    intros ->. 
+    eapply lookup_global_Some_fresh in hl.
+    rewrite e in wf. destruct wf as [_ ond]; depelim ond.
+    cbn in *. eapply Forall_app in f as []. contradiction.
+    intros _.
+    eapply IHx; trea.
+    rewrite e in wf. destruct wf as [onu ond]; depelim ond.
+    split => //.
+  Qed.
+
+Lemma is_erasableb_irrel_global_env {X_type X X_type' X'} {Γ t wt wt'} :
+  (forall Σ Σ' : global_env_ext, abstract_env_ext_rel X Σ -> 
+      abstract_env_ext_rel X' Σ' -> ∥ extends_decls Σ' Σ ∥ /\ (Σ.2 = Σ'.2)) ->
+  is_erasableb X_type X Γ t wt = is_erasableb X_type' X' Γ t wt'.
 Proof.
-  destruct Σ as [univs Σ].
-  destruct Σ' as [univs' Σ'].
-  intros wf [Σ'' []]. cbn in *. subst univs'.
-  induction x in Σ, Σ', e, wf |- *. cbn in e. now subst Σ'.
-  intros hl.
-  rewrite e; cbn. 
-  case: eqb_spec.
-  intros ->. 
-  eapply lookup_global_Some_fresh in hl.
-  rewrite e in wf. destruct wf as [_ ond]; depelim ond.
-  cbn in *. eapply Forall_app in f as []. contradiction.
-  intros _.
-  eapply IHx; trea.
-  rewrite e in wf. destruct wf as [onu ond]; depelim ond.
-  split => //.
-Qed.
-  
-Lemma is_erasableb_irrel_global_env {Σ Σ' : wf_env_ext} {Γ t wt wt'} :
-  wf Σ ->
-  extends_decls Σ' Σ ->
-  (Σ : global_env_ext).2 = (Σ' : global_env_ext).2 ->
-  is_erasableb Σ Γ t wt = is_erasableb Σ' Γ t wt'.
-Proof.
-  intros wf ext eqext.
-  assert (hl : Hlookup optimized_abstract_env_ext_impl Σ optimized_abstract_env_ext_impl Σ').
+  intro ext. 
+  (* ext eqext. *)
+  assert (hl : Hlookup X_type X X_type' X').
   { red. intros.
     rewrite -(abstract_env_lookup_correct _ _ H).
     rewrite -(abstract_env_lookup_correct _ _ H0).
-    rewrite H1 H2. cbn in H. cbn in H0. subst Σ0 Σ'0.
-    eapply extends_lookup_env in H2; tea. congruence. }
+    rewrite H1 H2. specialize (ext _ _ H H0) as [[?] ?]. pose proof (abstract_env_ext_wf _ H) as [?].
+    eapply extends_lookup_env in H2; try apply e; eauto. clear -H1 H2. congruence. }
   simp is_erasableb.
   set (obl := is_erasableb_obligation_2 _ _ _ _). clearbody obl.
-  set(ty := (type_of_typing optimized_abstract_env_ext_impl _ _ _ wt')) in *.
-  set(ty' := (type_of_typing optimized_abstract_env_ext_impl _ _ _ wt)) in *.
+  set(ty := (type_of_typing X_type' _ _ _ wt')) in *.
+  set(ty' := (type_of_typing X_type _ _ _ wt)) in *.
   assert (ty.π1 = ty'.π1).
   { subst ty ty'. unfold type_of_typing. symmetry. 
     eapply infer_irrel => //. }
   clearbody ty. clearbody ty'.
   destruct ty, ty'. cbn in H. subst x0.
   cbn -[is_arity] in obl |- *.
-  set (obl' := is_erasableb_obligation_1 Σ' Γ t wt').
-  set (obl'' := is_erasableb_obligation_2 Σ' Γ t _).
+  set (obl' := is_erasableb_obligation_1 X_type' X' Γ t wt').
+  set (obl'' := is_erasableb_obligation_2 X_type' X' Γ t _).
   clearbody obl'. clearbody obl''.
-  rewrite (is_arity_irrel (Σ' := Σ')) //.
-  destruct is_arity => //. simp is_erasableb.
-  set (obl2 := is_erasableb_obligation_3 _ _ _ _).
-  set (obl2' := is_erasableb_obligation_3 _ _ _ _).
-  simpl. f_equal.
-  apply (sort_of_type_irrel (X_type := optimized_abstract_env_ext_impl)
-    (X_type' := optimized_abstract_env_ext_impl) hl obl2 obl2').
+  rewrite (is_arity_irrel (X:=X) (X' := X') (wt' := obl'' (x; s))) => //.
+  destruct is_arity  => //. simp is_erasableb.
+  set (obl2 := is_erasableb_obligation_3 _ _ _ _ _).
+  set (obl2' := is_erasableb_obligation_3 _ _ _ _ _).
+  simpl. f_equal. now apply sort_of_type_irrel.
 Qed.
 
 Ltac iserasableb_irrel_env :=
   match goal with
-  [ H : context [is_erasableb ?Σ ?Γ ?t ?wt], Heq : inspect_bool _ = _ |- context [ is_erasableb _ _ _ ?wt'] ] => 
-    generalize dependent H; rewrite (@is_erasableb_irrel_global_env _ _ _ _ wt wt') //; intros; rewrite Heq
+  [ H : context [is_erasableb ?X_type ?X ?Γ ?t ?wt], Heq : inspect_bool _ = _ |- context [ is_erasableb _ _ _ _ ?wt'] ] => 
+    generalize dependent H; rewrite (@is_erasableb_irrel_global_env _ _ _ _ _ _ wt wt') //; intros; rewrite Heq
   end.
 
-Lemma erase_irrel_global_env {Σ Σ' : wf_env_ext} {Γ t wt wt'} :
-  wf Σ ->
-  extends_decls Σ' Σ ->
-  (Σ : global_env_ext).2 = (Σ' : global_env_ext).2 ->
-  erase Σ Γ t wt = erase Σ' Γ t wt'.
+Lemma erase_irrel_global_env {X_type X X_type' X'} {Γ t wt wt'} :
+  (forall Σ Σ' : global_env_ext, abstract_env_ext_rel X Σ -> 
+    abstract_env_ext_rel X' Σ' -> ∥ extends_decls Σ' Σ ∥ /\ (Σ.2 = Σ'.2)) ->
+  erase X_type X Γ t wt = erase X_type' X' Γ t wt'.
 Proof.
-  intros wfΣ ext eq.
+  intros ext. 
   move: wt'.
-  eapply (erase_elim Σ
+  eapply (erase_elim X_type X
   (fun Γ t wt e => 
-    forall (wt' : forall Σ0 : global_env_ext, abstract_env_rel' Σ' Σ0 ->  welltyped Σ0 Γ t), 
-    e = erase Σ' Γ t wt')
+    forall (wt' : forall Σ' : global_env_ext, abstract_env_ext_rel X' Σ' ->  welltyped Σ' Γ t), 
+    e = erase X_type' X' Γ t wt')
   (fun Γ l awt e => forall wt',
-    e = erase_terms Σ' Γ l wt')
+    e = erase_terms X_type' X' Γ l wt')
   (fun Γ p l awt e => forall wt', 
-    e = erase_brs Σ' Γ p l wt')
+    e = erase_brs X_type' X'  Γ p l wt')
   (fun Γ l awt e => forall wt', 
-    e = erase_fix Σ' Γ l wt')
+    e = erase_fix X_type' X'  Γ l wt')
   (fun Γ l awt e => forall wt', 
-    e = erase_cofix Σ' Γ l wt')).
+    e = erase_cofix X_type' X'  Γ l wt')).
   all:intros *; intros; simp_erase.
   simp erase.
   all:try simp erase; try iserasableb_irrel_env; simp_erase => //.
   all:try clear he Heq.
   all:try bang.
-  all:try solve [cbn; f_equal; eauto].
   all:try solve [cbn; repeat (f_equal; eauto)].
   cbn. f_equal. eauto. f_equal.
-  now rewrite (H (erase_obligation_19 Σ' Γ0 d mfix wt')).
-  now rewrite (H0 (erase_obligation_20 Σ' Γ0 d mfix wt')).
+  now rewrite (H (erase_obligation_19 X_type' X' Γ0 d mfix wt')).
+  now rewrite (H0 (erase_obligation_20 X_type' X'  Γ0 d mfix wt')).
 Qed.
 
-Lemma erase_constant_body_suffix {Σ Σ' : wf_env_ext} {cb ondecl ondecl'} :
-  wf Σ -> extends_decls Σ' Σ -> (Σ : global_env_ext).2 = (Σ' : global_env_ext).2 ->
-  erase_constant_body Σ cb ondecl = erase_constant_body Σ' cb ondecl'.
+Lemma erase_constant_body_suffix {X_type X X_type' X'} {cb ondecl ondecl'} :
+(forall Σ Σ' : global_env_ext, abstract_env_ext_rel X Σ -> 
+  abstract_env_ext_rel X' Σ' -> ∥ extends_decls Σ' Σ ∥ /\ (Σ.2 = Σ'.2)) ->
+erase_constant_body X_type X cb ondecl = erase_constant_body X_type' X' cb ondecl'.
 Proof.
-  intros wfΣ ext eqext.
+  intros ext.
   destruct cb => //=.
   destruct cst_body0 => //=.
   unfold erase_constant_body; simpl => /=.
@@ -3031,6 +1531,1636 @@ Proof.
   f_equal.
   eapply erase_irrel_global_env; tea.
 Qed.
+
+Require Import Morphisms.
+From MetaCoq.Template Require Import uGraph.
+Global Instance proper_pair_levels_gcs : Proper ((=_lset) ==> GoodConstraintSet.Equal ==> (=_gcs)) (@pair LevelSet.t GoodConstraintSet.t).
+Proof.
+  intros l l' eq gcs gcs' eq'.
+  split; cbn; auto.
+Qed.
+
+Program Fixpoint erase_global_decls {X_type : abstract_env_impl} (deps : KernameSet.t) (X : X_type.π1) (decls : global_declarations) 
+  (prop : forall Σ : global_env, abstract_env_rel X Σ -> Σ.(declarations) = decls) : E.global_declarations :=
+  match decls with
+  | [] => []
+  | (kn, ConstantDecl cb) :: decls =>
+    let X' := abstract_pop_decls X in
+    if KernameSet.mem kn deps then
+      let Xext := abstract_make_wf_env_ext X' (cst_universes cb) _ in
+      let cb' := erase_constant_body X_type.π2.π1 Xext cb _ in
+      let deps := KernameSet.union deps (snd cb') in
+      let X'' := erase_global_decls deps X' decls _ in
+      ((kn, E.ConstantDecl (fst cb')) :: X'')
+    else
+      erase_global_decls deps X' decls _
+
+  | (kn, InductiveDecl mib) :: decls =>
+    let X' := abstract_pop_decls X in
+    if KernameSet.mem kn deps then
+      let mib' := erase_mutual_inductive_body mib in
+      let X'' := erase_global_decls deps X' decls _ in
+      ((kn, E.InductiveDecl mib') :: X'')
+    else erase_global_decls deps X' decls _
+  end.
+Next Obligation. 
+  pose proof (abstract_env_wf _ H) as [wf]. 
+  pose proof (abstract_env_exists X) as [[? HX]]. 
+  pose proof (abstract_env_wf _ HX) as [wfX].
+  assert (prop': forall Σ : global_env, abstract_env_rel X Σ -> exists d, Σ.(declarations) = d :: decls).
+  { now eexists. }
+  pose proof (abstract_pop_decls_correct X decls prop' _ _ HX H). 
+  clear H. specialize (prop _ HX). destruct x, Σ, H0; cbn in *.
+  subst. sq. destruct wfX. depelim o0. split => //.
+Qed.
+Next Obligation.
+  pose proof (abstract_env_ext_wf _ H) as [wf]. 
+  pose proof (abstract_env_exists (abstract_pop_decls X)) as [[? HX']]. 
+  pose proof (abstract_env_wf _ HX') as [wfX'].
+  pose proof (abstract_env_exists X) as [[? HX]]. 
+  pose proof (abstract_env_wf _ HX) as [wfX].
+  assert (prop': forall Σ : global_env, abstract_env_rel X Σ -> exists d, Σ.(declarations) = d :: decls).
+  { now eexists. }
+  pose proof (abstract_pop_decls_correct X decls prop' _ _ HX HX'). 
+  pose proof (abstract_make_wf_env_ext_correct _ _ _ _ _ HX' H). 
+  clear H HX'. specialize (prop _ HX). destruct x, Σ as [[] u], H0; cbn in *.
+  subst. sq. inversion H1. subst. clear H1. destruct wfX. cbn in *.
+  rewrite prop in o0. depelim o0. apply o2.
+Qed.
+Next Obligation.
+  pose proof (abstract_env_exists X) as [[? HX]]. 
+  assert (prop': forall Σ : global_env, abstract_env_rel X Σ -> exists d, Σ.(declarations) = d :: decls).
+  { now eexists. }
+  now pose proof (abstract_pop_decls_correct X decls prop' _ _ HX H).
+Qed.  
+Next Obligation.  
+pose proof (abstract_env_exists X) as [[? HX]]. 
+assert (prop': forall Σ : global_env, abstract_env_rel X Σ -> exists d, Σ.(declarations) = d :: decls).
+{ now eexists. }
+now pose proof (abstract_pop_decls_correct X decls prop' _ _ HX H).
+Qed.  
+Next Obligation.
+  pose proof (abstract_env_exists X) as [[? HX]]. 
+  assert (prop': forall Σ : global_env, abstract_env_rel X Σ -> exists d, Σ.(declarations) = d :: decls).
+  { now eexists. }
+  now pose proof (abstract_pop_decls_correct X decls prop' _ _ HX H).
+Qed.  
+Next Obligation.
+pose proof (abstract_env_exists X) as [[? HX]]. 
+assert (prop': forall Σ : global_env, abstract_env_rel X Σ -> exists d, Σ.(declarations) = d :: decls).
+{ now eexists. }
+now pose proof (abstract_pop_decls_correct X decls prop' _ _ HX H).
+Qed.  
+
+Lemma erase_global_decls_irr X_type deps (X:X_type.π1) decls prf prf' :
+  erase_global_decls deps X decls prf =
+  erase_global_decls deps X decls prf'.
+Proof. 
+  revert X deps prf prf'.
+  induction decls; eauto. intros. destruct a as [kn []]; cbn.
+  - destruct KernameSet.mem; cbn.
+    erewrite erase_constant_body_suffix. f_equal.
+    eapply IHdecls. intros. 
+    pose proof (abstract_env_exists (abstract_pop_decls X)) as [[env wf]].
+    rewrite (abstract_make_wf_env_ext_correct (abstract_pop_decls X) (cst_universes c) _ _ _ wf H). 
+    now rewrite (abstract_make_wf_env_ext_correct (abstract_pop_decls X) (cst_universes c) _ _ _ wf H0). 
+    apply IHdecls.
+  - destruct KernameSet.mem; cbn. f_equal. eapply IHdecls.
+    apply IHdecls. 
+Qed.
+
+Definition global_erased_with_deps (Σ : global_env) (Σ' : EAst.global_declarations) kn :=
+  (exists cst, declared_constant Σ kn cst /\
+   exists cst' : EAst.constant_body,
+    EGlobalEnv.declared_constant Σ' kn cst' /\
+    erases_constant_body (Σ, cst_universes cst) cst cst' /\
+    (forall body : EAst.term,
+     EAst.cst_body cst' = Some body -> erases_deps Σ Σ' body)) \/
+  (exists mib mib', declared_minductive Σ kn mib /\ 
+    EGlobalEnv.declared_minductive Σ' kn mib' /\
+    erases_mutual_inductive_body mib mib').
+
+Definition includes_deps (Σ : global_env) (Σ' : EAst.global_declarations) deps :=  
+  forall kn, 
+    KernameSet.In kn deps ->
+    global_erased_with_deps Σ Σ' kn.
+
+Lemma includes_deps_union (Σ : global_env) (Σ' : EAst.global_declarations) deps deps' :
+  includes_deps Σ Σ' (KernameSet.union deps deps') ->
+  includes_deps Σ Σ' deps /\ includes_deps Σ Σ' deps'.
+Proof.
+  intros.
+  split; intros kn knin; eapply H; rewrite KernameSet.union_spec; eauto.
+Qed.
+
+Lemma includes_deps_fold {A} (Σ : global_env) (Σ' : EAst.global_declarations) brs deps (f : A -> EAst.term) :
+  includes_deps Σ Σ'
+  (fold_left
+    (fun (acc : KernameSet.t) (x : A) =>
+      KernameSet.union (term_global_deps (f x)) acc) brs
+      deps) ->
+  includes_deps Σ Σ' deps /\
+  (forall x, In x brs ->
+    includes_deps Σ Σ' (term_global_deps (f x))).
+Proof.
+  intros incl; split.
+  intros kn knin; apply incl.
+  rewrite knset_in_fold_left. left; auto.
+  intros br brin. intros kn knin. apply incl.
+  rewrite knset_in_fold_left. right.
+  now exists br.
+Qed.
+
+Definition declared_kn Σ kn :=
+  ∥ ∑ decl, lookup_env Σ kn = Some decl ∥.
+
+Lemma term_global_deps_spec {cf} {Σ : global_env_ext} {Γ t et T} : 
+  wf Σ.1 ->
+  Σ ;;; Γ |- t : T ->
+  Σ;;; Γ |- t ⇝ℇ et ->
+  forall x, KernameSet.In x (term_global_deps et) -> declared_kn Σ x.
+Proof.
+  intros wf wt er.
+  induction er in T, wt |- * using erases_forall_list_ind;
+    cbn in *; try solve [constructor]; intros kn' hin;
+    repeat match goal with 
+    | [ H : KernameSet.In _ KernameSet.empty |- _ ] =>
+      now apply KernameSet.empty_spec in hin
+    | [ H : KernameSet.In _ (KernameSet.union _ _) |- _ ] =>
+      apply KernameSet.union_spec in hin as [?|?]
+    end.
+  - apply inversion_Lambda in wt as (? & ? & ? & ? & ?); eauto.
+  - apply inversion_LetIn in wt as (? & ? & ? & ? & ? & ?); eauto.
+  - apply inversion_LetIn in wt as (? & ? & ? & ? & ? & ?); eauto.
+  - apply inversion_App in wt as (? & ? & ? & ? & ? & ?); eauto.
+  - apply inversion_App in wt as (? & ? & ? & ? & ? & ?); eauto.
+  - apply inversion_Const in wt as (? & ? & ? & ? & ?); eauto.
+    eapply KernameSet.singleton_spec in hin; subst.
+    red in d. red. sq. rewrite d. intuition eauto.
+  - apply inversion_Construct in wt as (? & ? & ? & ? & ? & ? & ?); eauto.
+    destruct kn.
+    eapply KernameSet.singleton_spec in hin; subst.
+    destruct d as [[H' _] _]. red in H'. simpl in *.
+    red. sq. rewrite H'. intuition eauto.
+  - apply inversion_Case in wt as (? & ? & ? & ? & [] & ?); eauto.
+    destruct ci as [kn i']; simpl in *.
+    eapply KernameSet.singleton_spec in H1; subst.
+    destruct x1 as [d _]. red in d.
+    simpl in *. eexists; intuition eauto.
+
+  - apply inversion_Case in wt as (? & ? & ? & ? & [] & ?); eauto.
+    eapply knset_in_fold_left in H1.
+    destruct H1. eapply IHer; eauto.
+    destruct H1 as [br [inbr inkn]].
+    eapply Forall2_All2 in H0.
+    assert (All (fun br => ∑ T, Σ ;;; Γ ,,, inst_case_branch_context p br |- br.(bbody) : T) brs).
+    eapply All2i_All_right. eapply brs_ty.
+    simpl. intuition auto. eexists ; eauto.
+    now rewrite -(PCUICCasesContexts.inst_case_branch_context_eq a).
+    eapply All2_All_mix_left in H0; eauto. simpl in H0.
+    eapply All2_In_right in H0; eauto.
+    destruct H0.
+    destruct X1 as [br' [[T' HT] ?]].
+    eauto.
+  
+  - eapply KernameSet.singleton_spec in H0; subst.
+    apply inversion_Proj in wt as (?&?&?&?&?&?&?&?&?&?); eauto.
+    destruct d as [[[d _] _] _]. red in d. eexists; eauto.
+
+  - apply inversion_Proj in wt as (?&?&?&?&?&?&?&?&?); eauto.
+
+  - apply inversion_Fix in wt as (?&?&?&?&?&?&?); eauto.
+    eapply knset_in_fold_left in hin as [|].
+    now eapply KernameSet.empty_spec in H0.
+    destruct H0 as [? [ina indeps]].
+    eapply Forall2_All2 in H.
+    eapply All2_All_mix_left in H; eauto.
+    eapply All2_In_right in H; eauto.
+    destruct H as [[def [Hty Hdef]]].
+    eapply Hdef; eauto.
+
+  - apply inversion_CoFix in wt as (?&?&?&?&?&?&?); eauto.
+    eapply knset_in_fold_left in hin as [|].
+    now eapply KernameSet.empty_spec in H0.
+    destruct H0 as [? [ina indeps]].
+    eapply Forall2_All2 in H.
+    eapply All2_All_mix_left in H; eauto.
+    eapply All2_In_right in H; eauto.
+    destruct H as [[def [Hty Hdef]]].
+    eapply Hdef; eauto.
+Qed.
+
+Global Remove Hints erases_deps_eval : core.
+
+Lemma erase_global_erases_deps {Σ} {Σ' : EAst.global_declarations} {Γ t et T} : 
+  wf_ext Σ ->
+  Σ;;; Γ |- t : T ->
+  Σ;;; Γ |- t ⇝ℇ et ->
+  includes_deps Σ Σ' (term_global_deps et) ->
+  erases_deps Σ Σ' et.
+Proof.
+  intros wf wt er.
+  induction er in er, t, T, wf, wt |- * using erases_forall_list_ind;
+    cbn in *; try solve [constructor]; intros Σer;
+    repeat match goal with 
+    | [ H : includes_deps _ _ (KernameSet.union _ _ ) |- _ ] =>
+      apply includes_deps_union in H as [? ?]
+    end.
+  - now apply inversion_Evar in wt.
+  - constructor.
+    now apply inversion_Lambda in wt as (? & ? & ? & ? & ?); eauto.
+  - apply inversion_LetIn in wt as (? & ? & ? & ? & ? & ?); eauto.
+    constructor; eauto.
+  - apply inversion_App in wt as (? & ? & ? & ? & ? & ?); eauto.
+    now constructor; eauto.
+  - apply inversion_Const in wt as (? & ? & ? & ? & ?); eauto.
+    specialize (Σer kn).
+    forward Σer. rewrite KernameSet.singleton_spec //.
+    destruct Σer as [[c' [declc' (? & ? & ? & ?)]]|].
+    pose proof (declared_constant_inj _ _ d declc'). subst x.
+    now econstructor; eauto.
+    destruct H as [mib [mib' [declm declm']]].
+    red in declm, d. rewrite d in declm. noconf declm.
+  - apply inversion_Construct in wt as (? & ? & ? & ? & ? & ?); eauto.
+    red in Σer. destruct kn.
+    setoid_rewrite KernameSetFact.singleton_iff in Σer.
+    destruct (Σer _ eq_refl) as [ (? & ? & ? & ? & ? & ?) | (? & ? & ? & ? & ?) ].
+    + red in H0. destruct d as [[]]. red in H4. cbn in *. unfold PCUICEnvironment.fst_ctx in *. congruence.
+    + pose proof H2 as H2'. destruct d. cbn in *. destruct H3. cbn in *. red in H3. red in H0. rewrite H0 in H3. invs H3.
+      destruct H2.
+      red in H1.
+      eapply Forall2_nth_error_Some_l in H2 as (? & ? & ?); eauto. pose proof H6 as H6'. destruct H6 as (? & ? & ? & ? & ?); eauto.
+      eapply Forall2_nth_error_Some_l in H6 as ([] & ? & ? & ?); subst; eauto.
+      econstructor. repeat eapply conj; eauto.
+      repeat eapply conj; cbn; eauto. eauto. eauto.
+  - apply inversion_Case in wt as (? & ? & ? & ? & [] & ?); eauto.
+    destruct ci as [[kn i'] ? ?]; simpl in *.
+    apply includes_deps_fold in H2 as [? ?].
+
+    specialize (H1 kn). forward H1.
+    now rewrite KernameSet.singleton_spec. red in H1. destruct H1.
+    elimtype False. destruct H1 as [cst [declc _]].
+    { red in declc. destruct x1 as [d _]. red in d. rewrite d in declc. noconf declc. }
+    destruct H1 as [mib [mib' [declm [declm' em]]]].
+    pose proof em as em'. destruct em'.
+    destruct x1 as [x1 hnth].
+    red in x1, declm. rewrite x1 in declm. noconf declm.
+    eapply Forall2_nth_error_left in H1; eauto. destruct H1 as [? [? ?]].
+    eapply erases_deps_tCase; eauto. 
+    split; eauto. split; eauto.
+    destruct H1.
+    eapply In_Forall in H3.
+    eapply All_Forall. eapply Forall_All in H3.
+    eapply Forall2_All2 in H0.
+    eapply All2_All_mix_right in H0; eauto.
+    assert (All (fun br => ∑ T, Σ ;;; Γ ,,, inst_case_branch_context p br |- br.(bbody) : T) brs).
+    eapply All2i_All_right. eapply brs_ty.
+    simpl. intuition auto. eexists ; eauto.
+    now rewrite -(PCUICCasesContexts.inst_case_branch_context_eq a).
+    ELiftSubst.solve_all. destruct a0 as [T' HT]. eauto.
+    
+  - apply inversion_Proj in wt as (?&?&?&?&?&?&?&?&?&?); eauto.
+    destruct (proj1 d).
+    specialize (H0 (inductive_mind p.(proj_ind))). forward H0.
+    now rewrite KernameSet.singleton_spec. red in H0. destruct H0.
+    elimtype False. destruct H0 as [cst [declc _]].
+    { red in declc. destruct d as [[[d _] _] _]. red in d. rewrite d in declc. noconf declc. }
+    destruct H0 as [mib [mib' [declm [declm' em]]]].
+    assert (mib = x0).
+    { destruct d as [[[]]].
+      red in H0, declm. rewrite H0 in declm. now noconf declm. } 
+    subst x0.
+    pose proof em as em'. destruct em'.
+    eapply Forall2_nth_error_left in H0 as (x' & ? & ?); eauto.
+    2:{ apply d. }
+    simpl in *.
+    destruct (ind_ctors x1) => //. noconf H3.
+    set (H1' := H5). destruct H1' as [].
+    set (d' := d). destruct d' as [[[]]].
+    eapply Forall2_All2 in H3. eapply All2_nth_error_Some in H3 as [? [? []]]; tea.
+    destruct H6 as [Hprojs _].
+    eapply Forall2_All2 in Hprojs. eapply All2_nth_error_Some in Hprojs as [? []]; tea.
+    2:eapply d.
+    econstructor; tea. all:eauto.
+    split => //. 2:split; eauto.
+    split; eauto. split; eauto.
+    rewrite -H4. symmetry; apply d.
+    
+  - constructor.
+    apply inversion_Fix in wt as (?&?&?&?&?&?&?); eauto.
+    eapply All_Forall. eapply includes_deps_fold in Σer as [_ Σer].
+    eapply In_Forall in Σer.
+    eapply Forall_All in Σer.
+    eapply Forall2_All2 in H.
+    ELiftSubst.solve_all.
+  - constructor.
+    apply inversion_CoFix in wt as (?&?&?&?&?&?&?); eauto.
+    eapply All_Forall. eapply includes_deps_fold in Σer as [_ Σer].
+    eapply In_Forall in Σer.
+    eapply Forall_All in Σer.
+    eapply Forall2_All2 in H.
+    ELiftSubst.solve_all. Unshelve. 
+Qed.
+
+Lemma erases_weakeninv_env {Σ Σ' : global_env_ext} {Γ t t' T} :
+  wf Σ' -> extends_decls Σ Σ' -> 
+  Σ ;;; Γ |- t : T ->
+  erases Σ Γ t t' -> erases (Σ'.1, Σ.2) Γ t t'.
+Proof.
+  intros wfΣ' ext Hty.
+  eapply (env_prop_typing ESubstitution.erases_extends); tea.
+  eapply extends_decls_wf; tea.
+Qed.  
+ 
+Lemma erases_deps_weaken kn d (Σ : global_env) (Σ' : EAst.global_declarations) t : 
+  wf (add_global_decl Σ (kn, d)) ->
+  erases_deps Σ Σ' t ->
+  erases_deps (add_global_decl Σ (kn, d)) Σ' t.
+Proof.
+  intros wfΣ er.
+  induction er using erases_deps_forall_ind; try solve [now constructor].
+  - assert (kn <> kn0).
+    { inv wfΣ. inv X. intros <-.
+      eapply lookup_env_Some_fresh in H. contradiction. }
+    eapply erases_deps_tConst with cb cb'; eauto.
+    red. rewrite /lookup_env lookup_env_cons_fresh //.
+    red.
+    red in H1.
+    destruct (cst_body cb) eqn:cbe;
+    destruct (E.cst_body cb') eqn:cbe'; auto.
+    specialize (H3 _ eq_refl).
+    eapply on_declared_constant in H; auto.
+    2:{ inv wfΣ. now inv X. }
+    red in H. rewrite cbe in H. simpl in H.
+    eapply (erases_weakeninv_env (Σ := (Σ, cst_universes cb))
+       (Σ' := (add_global_decl Σ (kn, d), cst_universes cb))); eauto.
+    simpl.
+    split => //; eexists [(kn, d)]; intuition eauto.
+  - econstructor; eauto. eapply weakening_env_declared_constructor; eauto.
+    eapply extends_decls_extends. econstructor; try reflexivity. eexists [(_, _)]; reflexivity. 
+  - econstructor; eauto.
+    red. destruct H. split; eauto.
+    red in H. red.
+    inv wfΣ. inv X.
+    rewrite -H. simpl. unfold lookup_env; simpl. destruct (eqb_spec (inductive_mind p.1) kn); try congruence.
+    eapply lookup_env_Some_fresh in H. subst kn; contradiction.
+  - econstructor; eauto.
+    red. destruct H. split; eauto.
+    destruct d0; split; eauto.
+    destruct d0; split; eauto.
+    inv wfΣ. inv X.
+    red in H |- *.
+    rewrite -H. simpl. unfold lookup_env; simpl; destruct (eqb_spec (inductive_mind p.(proj_ind)) kn); try congruence.
+    eapply lookup_env_Some_fresh in H. subst kn. contradiction.
+Qed.
+
+Lemma lookup_env_ext {Σ kn kn' d d'} : 
+  wf (add_global_decl Σ (kn', d')) ->
+  lookup_env Σ kn = Some d ->
+  kn <> kn'.
+Proof.
+  intros wf hl. 
+  eapply lookup_env_Some_fresh in hl.
+  inv wf. inv X.
+  destruct (eqb_spec kn kn'); subst; congruence.
+Qed.
+
+Lemma lookup_env_cons_disc {Σ kn kn' d} : 
+  kn <> kn' ->
+  lookup_env (add_global_decl Σ (kn', d)) kn = lookup_env Σ kn.
+Proof.
+  intros Hk. simpl; unfold lookup_env; simpl.
+  destruct (eqb_spec kn kn'); congruence.
+Qed.
+
+Lemma elookup_env_cons_disc {Σ kn kn' d} : 
+  kn <> kn' ->
+  EGlobalEnv.lookup_env ((kn', d) :: Σ) kn = EGlobalEnv.lookup_env Σ kn.
+Proof.
+  intros Hk. simpl.
+  destruct (eqb_spec kn kn'); congruence.
+Qed.
+
+Lemma global_erases_with_deps_cons kn kn' d d' Σ Σ' : 
+  wf (add_global_decl Σ (kn', d)) ->
+  global_erased_with_deps Σ Σ' kn ->
+  global_erased_with_deps (add_global_decl Σ (kn', d)) ((kn', d') :: Σ') kn.
+Proof.
+  intros wf [[cst [declc [cst' [declc' [ebody IH]]]]]|].
+  red. inv wf. inv X. left.
+  exists cst. split.
+  red in declc |- *. unfold lookup_env in *.
+  rewrite lookup_env_cons_fresh //.
+  { eapply lookup_env_Some_fresh in declc.
+    intros <-; contradiction. }
+  exists cst'.
+  unfold EGlobalEnv.declared_constant. rewrite EGlobalEnv.elookup_env_cons_fresh //.
+  { eapply lookup_env_Some_fresh in declc.
+    intros <-; contradiction. }
+  red in ebody. unfold erases_constant_body.
+  destruct (cst_body cst) eqn:bod; destruct (E.cst_body cst') eqn:bod' => //.
+  intuition auto.
+  eapply (erases_weakeninv_env (Σ  := (_, cst_universes cst)) (Σ' := (add_global_decl Σ (kn', d), cst_universes cst))); eauto.
+  constructor; eauto. constructor; eauto.
+  split => //. exists [(kn', d)]; intuition eauto.
+  eapply on_declared_constant in declc; auto.
+  red in declc. rewrite bod in declc. eapply declc.
+  split => //.
+  noconf H0.
+  eapply erases_deps_cons; eauto.
+  constructor; auto.
+
+  right. destruct H as [mib [mib' [? [? ?]]]].
+  exists mib, mib'. intuition eauto.
+  * red. red in H. pose proof (lookup_env_ext wf H).
+    now rewrite lookup_env_cons_disc.
+  * red. pose proof (lookup_env_ext wf H).
+    now rewrite elookup_env_cons_disc.
+Qed.
+
+Lemma global_erases_with_deps_weaken kn kn' d Σ Σ' : 
+  wf (add_global_decl Σ (kn', d)) ->
+  global_erased_with_deps Σ Σ' kn ->
+  global_erased_with_deps (add_global_decl Σ (kn', d)) Σ' kn.
+Proof.
+  intros wf [[cst [declc [cst' [declc' [ebody IH]]]]]|].
+  red. inv wf. inv X. left.
+  exists cst. split.
+  red in declc |- *.
+  unfold lookup_env in *.
+  rewrite lookup_env_cons_fresh //.
+  { eapply lookup_env_Some_fresh in declc.
+    intros <-. contradiction. }
+  exists cst'.
+  unfold EGlobalEnv.declared_constant.
+  red in ebody. unfold erases_constant_body.
+  destruct (cst_body cst) eqn:bod; destruct (E.cst_body cst') eqn:bod' => //.
+  intuition auto.
+  eapply (erases_weakeninv_env (Σ  := (Σ, cst_universes cst)) (Σ' := (add_global_decl Σ (kn', d), cst_universes cst))). 4:eauto.
+  split; auto. constructor; eauto.
+  split; auto; exists [(kn', d)]; intuition eauto.
+  eapply on_declared_constant in declc; auto.
+  red in declc. rewrite bod in declc. eapply declc. split => //.
+  noconf H0.
+  apply erases_deps_weaken.
+  { split; auto. cbn. constructor; auto. }
+  auto.
+
+  right. destruct H as [mib [mib' [Hm [? ?]]]].
+  exists mib, mib'; intuition auto.
+  red. unfold lookup_env in *.
+  rewrite lookup_env_cons_fresh //.
+  now epose proof (lookup_env_ext wf Hm).
+Qed.
+
+Lemma erase_constant_body_correct X_type X cb 
+  (onc : forall Σ : global_env_ext, abstract_env_ext_rel X Σ -> ∥ on_constant_decl (lift_typing typing) Σ cb ∥) :
+  forall Σ Σ', abstract_env_ext_rel X Σ -> 
+  wf Σ' -> extends_decls Σ Σ' ->
+  erases_constant_body (Σ', Σ.2) cb (fst (erase_constant_body X_type X cb onc)).
+Proof.
+  red. destruct cb as [name [bod|] univs]; simpl; eauto. intros.
+  set (ecbo := erase_constant_body_obligation_1 X_type X _ _ _ _). clearbody ecbo.
+  cbn in *. specialize_Σ H. sq.  
+  eapply (erases_weakeninv_env (Σ := Σ) (Σ' := (Σ', univs))); simpl; eauto.
+  now eapply erases_erase.
+Qed.
+
+Lemma erase_constant_body_correct' {X_type X} {cb} 
+  {onc : forall Σ : global_env_ext, abstract_env_ext_rel X Σ -> ∥ on_constant_decl (lift_typing typing) Σ cb ∥} 
+  {body} :
+  EAst.cst_body (fst (erase_constant_body X_type X cb onc)) = Some body ->
+  forall Σ : global_env_ext, abstract_env_ext_rel X Σ -> 
+  ∥ ∑ t T, (Σ ;;; [] |- t : T) * (Σ ;;; [] |- t ⇝ℇ body) *
+    (term_global_deps body = snd (erase_constant_body X_type X cb onc)) ∥.
+Proof.
+  intros. destruct cb as [name [bod|] univs]; simpl; [| now simpl in H].
+  simpl in H. noconf H. 
+  set (obl :=(erase_constant_body_obligation_1 X_type X
+  {|
+  cst_type := name;
+  cst_body := Some bod;
+  cst_universes := univs |} onc bod eq_refl)). clearbody obl. cbn in *. 
+  specialize_Σ H0. destruct (obl _ H0). sq.
+  exists bod, A; intuition auto. now eapply erases_erase. 
+Qed.
+
+Lemma erases_mutual {Σ mdecl m} : 
+  on_inductive (lift_typing typing) (Σ, ind_universes m) mdecl m ->
+  erases_mutual_inductive_body m (erase_mutual_inductive_body m).
+Proof.
+  intros oni.
+  destruct m; constructor; simpl; auto.
+  eapply onInductives in oni; simpl in *.
+  assert (Alli (fun i oib => 
+    match destArity [] oib.(ind_type) with Some _ => True | None => False end) 0 ind_bodies0).
+  { eapply Alli_impl; eauto.
+    simpl. intros n x []. simpl in *. rewrite ind_arity_eq.
+    rewrite !destArity_it_mkProd_or_LetIn /= //. } clear oni.
+  induction X; constructor; auto.
+  destruct hd; constructor; simpl; auto.
+  clear.
+  induction ind_ctors0; constructor; auto.
+  cbn in *.
+  intuition auto.
+  induction ind_projs0; constructor; auto.
+  unfold isPropositionalArity.
+  destruct destArity as [[? ?]|] eqn:da; auto.
+Qed.
+
+Lemma erase_global_includes X_type (X:X_type.π1) deps decls prf deps' :
+  (forall d, KernameSet.In d deps' -> 
+    forall Σ : global_env, abstract_env_rel X Σ -> ∥ ∑ decl, lookup_env Σ d = Some decl ∥) ->
+  KernameSet.subset deps' deps ->
+  forall Σ : global_env, abstract_env_rel X Σ ->
+  let Σ' := erase_global_decls deps X decls prf in
+  includes_deps Σ Σ' deps'.
+Proof.
+  intros ? sub Σ wfΣ; cbn. induction decls in X, H, sub, prf, deps, deps', Σ , wfΣ |- *.
+  - simpl. intros i hin. elimtype False.
+    specialize (H i hin) as [[decl Hdecl]]; eauto.
+    rewrite /lookup_env (prf _ wfΣ) in Hdecl. noconf Hdecl.
+  - intros i hin.
+    destruct (abstract_env_wf _ wfΣ) as [wf].
+    destruct a as [kn d].
+    eapply KernameSet.subset_spec in sub.
+    edestruct (H i hin) as [[decl Hdecl]]; eauto. unfold lookup_env in Hdecl.
+    pose proof (eqb_spec i kn).
+    rewrite (prf _ wfΣ) in Hdecl. move: Hdecl. cbn -[erase_global_decls].
+    elim: H0. intros -> [= <-].
+    * destruct d as [|]; [left|right].
+      { cbn. set (Xpop := abstract_pop_decls X).
+        set (Xmake :=  abstract_make_wf_env_ext Xpop (cst_universes c) _).
+        epose proof (abstract_env_exists Xpop) as [[Σpop wfpop]].
+        epose proof (abstract_env_ext_exists Xmake) as [[Σmake wfmake]].
+        exists c. split; auto. red.
+        unfold lookup_env; simpl; rewrite (prf _ wfΣ). cbn. rewrite eq_kername_refl //.
+        pose proof (sub _ hin) as indeps.
+        eapply KernameSet.mem_spec in indeps.
+        unfold EGlobalEnv.declared_constant. 
+        edestruct (H _ hin) as [[decl hd]]; eauto. 
+        eexists; intuition eauto.
+        rewrite indeps. cbn.
+        rewrite eq_kername_refl. reflexivity.
+        eapply (erase_constant_body_correct _ _ _ _ (Σpop , _)); eauto.
+        rewrite <- (abstract_make_wf_env_ext_correct Xpop (cst_universes c) _ Σpop Σmake wfpop wfmake); eauto. 
+        red. simpl. unshelve epose (abstract_pop_decls_correct X decls _ Σ Σpop wfΣ wfpop).
+        { intros. now eexists. }
+        split => //. intuition eauto.
+        exists [(kn, ConstantDecl c)]; intuition eauto. rewrite H0; eauto.  
+        rewrite indeps. unshelve epose proof (abstract_pop_decls_correct X decls _ Σ Σpop wfΣ wfpop) as [Hpop Hpop'].
+        { intros. now eexists. }
+        pose (prf' := prf _ wfΣ).
+        destruct Σ. cbn in *. rewrite Hpop' prf'. rewrite <- Hpop at 1.  
+        eapply (erases_deps_cons Σpop). 
+          rewrite <- Hpop'. apply wf.
+          rewrite Hpop. rewrite prf' in wf. destruct wf. now rewrite Hpop' in o0. 
+
+        pose proof (erase_constant_body_correct' H0). specialize_Σ wfmake. 
+        sq. destruct H1 as [bod [bodty [[Hbod Hebod] Heqdeps]]].
+        rewrite (abstract_make_wf_env_ext_correct Xpop (cst_universes c) _ Σpop Σmake wfpop wfmake) in Hbod, Hebod. 
+        eapply (erase_global_erases_deps (Σ := (Σpop, cst_universes c))); simpl; auto.
+        { constructor; simpl; auto. depelim wf. rewrite Hpop' in o0.
+          cbn in o0, o. rewrite prf' in o0. rewrite  <- Hpop in o0. rewrite Hpop' in o. clear -o o0. 
+          now depelim o0.
+          depelim wf. rewrite Hpop' in o0.
+          cbn in o0, o. rewrite prf' in o0.  rewrite <- Hpop in o0. clear -o0.  now depelim o0. }
+        all: eauto. 
+        apply IHdecls; eauto. 
+        { intros. pose proof (abstract_env_wf _ wfpop) as [wf'].
+          destruct Σpop. cbn in *. clear prf'.  subst. 
+          unshelve epose proof (abstract_pop_decls_correct X decls _ _ _ wfΣ H2) as [Hpop Hpop'].
+          { intros. now eexists. }
+          destruct Σ.  cbn in *. subst.
+          eapply term_global_deps_spec in Hebod; eauto. }
+        {  eapply KernameSet.subset_spec.
+          intros x hin'. eapply KernameSet.union_spec. right; auto.
+          now rewrite -Heqdeps. } }
+        { eexists m, _; intuition eauto.
+          simpl. rewrite /declared_minductive /lookup_env prf; eauto. 
+          simpl. rewrite eq_kername_refl. reflexivity.
+          specialize (sub _ hin).
+          eapply KernameSet.mem_spec in sub.
+          simpl. rewrite sub.
+          red. cbn. rewrite eq_kername_refl.
+          reflexivity.
+          assert (declared_minductive Σ kn m).
+          { red. unfold lookup_env. rewrite prf; eauto. cbn. now rewrite eqb_refl. }
+          eapply on_declared_minductive in H0; tea.
+          now eapply erases_mutual. }
+
+    * intros ikn Hi. 
+      destruct d as [|].
+      ++ simpl. destruct (KernameSet.mem kn deps) eqn:eqkn.
+        set (Xpop := abstract_pop_decls X).
+        set (Xmake :=  abstract_make_wf_env_ext Xpop (cst_universes c) _).
+        epose proof (abstract_env_exists Xpop) as [[Σp wfpop]].
+        pose proof (abstract_env_wf _ wfpop) as [wfΣp].
+        unshelve epose proof (abstract_pop_decls_correct X decls _ _ _ wfΣ wfpop) as [Hpop Hpop'].
+        { intros. now eexists. }
+        pose proof (prf _ wfΣ). destruct Σ. cbn in *. subst.
+        eapply global_erases_with_deps_cons; eauto.
+        eapply (IHdecls Xpop _ _ (KernameSet.singleton i)); auto.
+        3:{ eapply KernameSet.singleton_spec => //. }
+        intros.
+        eapply KernameSet.singleton_spec in H0.
+        pose proof (abstract_env_irr _ H1 wfpop). subst. 
+        sq; exists decl; eauto.
+        eapply KernameSet.subset_spec. intros ? ?.
+        eapply KernameSet.union_spec. left.
+        eapply KernameSet.singleton_spec in H0; subst.
+        now eapply sub.
+      
+        cbn. set (Xpop := abstract_pop_decls X).
+        epose proof (abstract_env_exists Xpop) as [[Σp wfpop]].
+        pose proof (abstract_env_wf _ wfpop) as [wfΣp].   
+        unshelve epose proof (abstract_pop_decls_correct X decls _ Σ Σp wfΣ wfpop) as [Hpop Hpop'].
+        { intros. now eexists. }
+        pose proof (prf _ wfΣ). destruct Σ. cbn in *. subst.
+        eapply global_erases_with_deps_weaken. eauto.
+        eapply IHdecls => //.
+        3:now eapply KernameSet.singleton_spec.
+        intros d ind%KernameSet.singleton_spec.
+        intros. pose proof (abstract_env_irr _ H0 wfpop). subst. 
+        sq; eexists; eauto.
+        eapply KernameSet.subset_spec.
+        intros ? hin'. eapply sub. eapply KernameSet.singleton_spec in hin'. now subst.
+
+      ++ simpl. set (Xpop := abstract_pop_decls X).
+      epose proof (abstract_env_exists Xpop) as [[Σp wfpop]].
+      pose proof (abstract_env_wf _ wfpop) as [wfΣp].      
+      unshelve epose proof (abstract_pop_decls_correct X decls _ Σ Σp wfΣ wfpop) as [Hpop Hpop'].
+      { intros. now eexists. }
+      pose proof (prf _ wfΣ). destruct Σ. cbn in *. subst.
+      destruct (KernameSet.mem kn deps) eqn:eqkn.
+        { eapply (global_erases_with_deps_cons _ kn (InductiveDecl _) _ Σp); eauto.
+          eapply (IHdecls Xpop _ _ (KernameSet.singleton i)); auto.
+          3:{ eapply KernameSet.singleton_spec => //. }
+          intros.
+          eapply KernameSet.singleton_spec in H0. subst.
+          pose proof (abstract_env_irr _ H1 wfpop). subst. 
+          sq; eexists; eauto.
+          eapply KernameSet.subset_spec. intros ? ?.
+          eapply KernameSet.singleton_spec in H0; subst.
+          now eapply sub. }
+    
+        { eapply (global_erases_with_deps_weaken _ kn (InductiveDecl _) Σp). eauto.
+          eapply (IHdecls Xpop _ _  (KernameSet.singleton i)) => //.
+          3:now eapply KernameSet.singleton_spec.
+          intros d ind%KernameSet.singleton_spec.
+          intros. pose proof (abstract_env_irr _ H0 wfpop). subst. 
+          sq; eexists; eauto.
+          eapply KernameSet.subset_spec.
+          intros ? hin'. eapply sub. eapply KernameSet.singleton_spec in hin'. now subst. }
+Qed.
+
+Lemma erase_correct (wfl := Ee.default_wcbv_flags) X_type (X : X_type.π1) 
+  univs wfext t v Σ' t' deps decls prf :
+  let Xext :=  abstract_make_wf_env_ext X univs wfext in
+  forall wt : forall Σ : global_env_ext, abstract_env_ext_rel Xext Σ -> welltyped Σ [] t,
+  erase X_type.π2.π1 Xext [] t wt = t' ->
+  KernameSet.subset (term_global_deps t') deps ->
+  erase_global_decls deps X decls prf = Σ' ->
+  (forall Σ : global_env, abstract_env_rel X Σ -> Σ |-p t ▷ v) ->
+  forall Σ : global_env_ext, abstract_env_ext_rel Xext Σ -> 
+  exists v', Σ ;;; [] |- v ⇝ℇ v' /\ ∥ Σ' ⊢ t' ▷ v' ∥.
+Proof.
+  intros Xext wt.
+  intros HΣ' Hsub Ht' ev Σext wfΣex.
+  pose proof (erases_erase (X := Xext) wt).
+  rewrite HΣ' in H.
+  destruct (wt _ wfΣex) as [T wt'].
+  pose proof (abstract_env_ext_wf _ wfΣex) as [wfΣ].
+  specialize (H _ wfΣex).
+  unshelve epose proof (erase_global_erases_deps (Σ' := Σ') wfΣ wt' H _); cycle 2.
+  rewrite <- Ht'.
+  eapply erase_global_includes; eauto. 
+  intros. eapply term_global_deps_spec in H; eauto.
+  now rewrite (abstract_make_wf_env_ext_correct X univs wfext Σ _ H1 wfΣex) in H.
+  
+  epose proof (abstract_env_exists X) as [[Σ wfΣX]].
+  now rewrite (abstract_make_wf_env_ext_correct X univs wfext Σ _ wfΣX wfΣex).
+  epose proof (abstract_env_exists X) as [[Σ wfΣX]].
+  eapply erases_correct; tea.
+  rewrite (abstract_make_wf_env_ext_correct X univs wfext _ _ wfΣX wfΣex); eauto.
+Qed.
+
+Lemma global_env_ind (P : global_env -> Type) (Pnil : forall univs, P {| universes := univs; declarations := [] |})
+  (Pcons : forall (Σ : global_env) d, P Σ -> P (add_global_decl Σ d))
+  (Σ : global_env) : P Σ.
+Proof.
+  destruct Σ as [univs Σ].
+  induction Σ; cbn. apply Pnil.
+  now apply (Pcons {| universes := univs; declarations := Σ |} a).
+Qed.
+
+Lemma on_global_env_ind (P : forall Σ : global_env, wf Σ -> Type)
+  (Pnil : forall univs (onu : on_global_univs univs), P {| universes := univs; declarations := [] |}
+    (onu, globenv_nil _ _))
+  (Pcons : forall (Σ : global_env) kn d (wf : wf Σ) 
+    (Hfresh : fresh_global kn Σ.(declarations))
+    (udecl := PCUICLookup.universes_decl_of_decl d)
+    (onud : on_udecl Σ.(universes) udecl)
+    (pd : on_global_decl (lift_typing typing) ({| universes := Σ.(universes); declarations := Σ.(declarations) |}, udecl) kn d),
+    P Σ wf -> P (add_global_decl Σ (kn, d)) 
+    (fst wf, globenv_decl _ Σ.(universes) Σ.(declarations) kn d (snd wf) Hfresh onud pd))
+  (Σ : global_env) (wfΣ : wf Σ) : P Σ wfΣ.
+Proof.
+  destruct Σ as [univs Σ]. destruct wfΣ; cbn in *.
+  induction o0. apply Pnil.
+  apply (Pcons {| universes := univs; declarations := Σ |} kn d (o, o0)).
+  exact IHo0.
+Qed.
+
+Ltac inv_eta :=
+  lazymatch goal with
+  | [ H : PCUICEtaExpand.expanded _ _ |- _ ] => depelim H
+  end.
+
+
+Lemma leq_term_propositional_sorted_l {Σ Γ v v' u u'} :
+   wf_ext Σ ->
+   PCUICEquality.leq_term Σ (global_ext_constraints Σ) v v' ->
+   Σ;;; Γ |- v : tSort u ->
+   Σ;;; Γ |- v' : tSort u' -> is_propositional u -> 
+   leq_universe (global_ext_constraints Σ) u' u.
+Proof.
+  intros wfΣ leq hv hv' isp.
+  eapply orb_true_iff in isp as [isp | isp].
+  - eapply leq_term_prop_sorted_l; eauto.
+  - eapply leq_term_sprop_sorted_l; eauto.
+Qed.
+
+Fixpoint map_erase X_type (X : X_type.π1) Γ 
+  (ts : list term) 
+  (H2 : forall Σ : global_env_ext, abstract_env_ext_rel X Σ -> 
+    Forall (welltyped Σ Γ) ts) {struct ts}: list E.term.
+destruct ts as [ | t ts].
+- exact [].
+- eapply cons. refine (erase X_type X Γ t _). 
+  2: eapply (map_erase X_type X Γ ts).
+  all: intros; specialize_Σ H; now inversion H2; subst.
+Defined.
+
+Lemma map_erase_irrel X_type X Γ t H1 H2 : 
+        map_erase X_type X Γ t H1 = map_erase X_type X Γ t H2.
+Proof.
+  epose proof (abstract_env_ext_exists X) as [[Σ wfΣX]].
+  induction t.
+  - reflexivity.
+  - cbn. f_equal.
+    + eapply erase_irrel.
+    + eapply IHt.
+Qed.
+
+Arguments map_erase _ _ _ _, _ _ _ {_}.
+
+Lemma erase_mkApps {X_type X} Γ t args H2 Ht Hargs :
+  (forall Σ : global_env_ext, abstract_env_ext_rel X Σ -> wf_local Σ Γ) ->
+  (forall Σ : global_env_ext, abstract_env_ext_rel X Σ -> ~ ∥ isErasable Σ Γ (mkApps t args) ∥) ->
+  erase X_type X Γ (mkApps t args) H2 = 
+  E.mkApps (erase X_type X Γ t Ht) (map_erase X_type X Γ args Hargs).
+Proof.
+  epose proof (abstract_env_ext_exists X) as [[Σ wfΣX]].
+  pose proof (abstract_env_ext_wf X wfΣX) as [wf]. 
+  intros Hwflocal Herasable. induction args in t, H2, Ht, Hargs, Herasable |- *.
+  - cbn. eapply erase_irrel.
+  - cbn [mkApps]. 
+    rewrite IHargs; clear IHargs.
+    all: intros; specialize_Σ H; try pose proof (abstract_env_ext_wf _ H) as [wfH].
+    1: inversion Hargs; eauto.
+    2: eauto.
+    2:{ destruct H2. cbn in X0. eapply inversion_mkApps in X0 as (? & ? & ?).
+        econstructor. eauto. }
+    etransitivity. simp erase. reflexivity. unfold erase_clause_1.
+    unfold inspect. unfold erase_clause_1_clause_2.
+    Unshelve.
+    elim: is_erasableP.
+    + intros. exfalso. 
+      eapply Herasable; eauto. specialize_Σ wfΣX. destruct p.
+      cbn. destruct H2. eapply Is_type_app; eauto.
+    + cbn [map_erase]. 
+      epose proof (fst (erase_irrel _ _)). cbn.
+      intros he. f_equal => //. f_equal.
+      eapply erase_irrel. eapply erase_irrel.
+      eapply map_erase_irrel. 
+      Unshelve. 2: exact X. 
+Qed.
+
+Lemma map_erase_length X_type X Γ t H1 : length (map_erase X_type X Γ t H1) = length t.
+Proof.
+  induction t; cbn; f_equal; eauto.
+Qed.
+
+Local Hint Constructors expanded : expanded.
+
+Local Arguments erase_global_decls _ _ _ : clear implicits.
+
+Lemma lookup_env_erase X_type X deps decls prf kn d :
+  KernameSet.In kn deps -> 
+  forall Σ : global_env, abstract_env_rel X Σ -> lookup_env Σ kn = Some (InductiveDecl d) ->
+  EGlobalEnv.lookup_env (erase_global_decls X_type deps X decls prf) kn = Some (EAst.InductiveDecl (erase_mutual_inductive_body d)).
+Proof.
+  intros hin Σ wfΣ. pose proof (prf _ wfΣ). unfold lookup_env. rewrite H. clear H.
+  rewrite /lookup_env. 
+  induction decls in X, Σ , wfΣ ,prf, deps, hin |- *.
+  - move=> /= //.
+  - destruct a as [kn' d'].
+    cbn -[erase_global_decls].
+    case: (eqb_spec kn kn'); intros e'; subst.
+    intros [= ->].
+    unfold erase_global_decls.
+    eapply KernameSet.mem_spec in hin. rewrite hin /=.
+    now rewrite eq_kername_refl.
+    intros hl. destruct d'. simpl.
+    set (Xpop := abstract_pop_decls X).
+    set (Xmake :=  abstract_make_wf_env_ext Xpop (cst_universes c) _).
+    epose proof (abstract_env_exists Xpop) as [[Σp wfpop]].
+    destruct KernameSet.mem. cbn.
+    rewrite (negbTE (proj2 (neqb _ _) e')).
+    eapply IHdecls => //; eauto. eapply KernameSet.union_spec. left => //.
+    eapply IHdecls => //; eauto.
+    simpl.
+    set (Xpop := abstract_pop_decls X).
+    epose proof (abstract_env_exists Xpop) as [[Σp wfpop]].
+    destruct KernameSet.mem. cbn.
+    rewrite (negbTE (proj2 (neqb _ _) e')).
+    eapply IHdecls => //; eauto.
+    eapply IHdecls => //; eauto. 
+Qed.
+
+Lemma erase_global_declared_constructor X_type X ind c mind idecl cdecl deps decls prf:
+   forall Σ : global_env, abstract_env_rel X Σ -> declared_constructor Σ (ind, c) mind idecl cdecl ->
+   KernameSet.In ind.(inductive_mind) deps -> 
+   EGlobalEnv.declared_constructor (erase_global_decls X_type deps X decls prf) (ind, c) 
+    (erase_mutual_inductive_body mind) (erase_one_inductive_body idecl) 
+    (EAst.mkConstructor cdecl.(cstr_name) cdecl.(cstr_arity)).
+Proof.
+  intros Σ wfΣ [[]] Hin.
+  cbn in *. split. split. 
+  - red in H |- *. now eapply lookup_env_erase.
+  - cbn. now eapply map_nth_error.
+  - cbn. erewrite map_nth_error; eauto.
+Qed.
+
+Import EGlobalEnv.
+Lemma erase_global_decls_fresh X_type kn deps X decls heq : 
+  let Σ' := erase_global_decls X_type deps X decls heq in
+  PCUICTyping.fresh_global kn decls ->
+  fresh_global kn Σ'.
+Proof.
+  cbn.
+  revert deps X heq.
+  induction decls; [cbn; auto|].
+  - intros. red. constructor.
+  - destruct a as [kn' d]. intros. depelim H.
+    cbn in H, H0.
+    destruct d as []; simpl; destruct KernameSet.mem.
+    + cbn [EGlobalEnv.closed_env forallb]. cbn.
+      constructor => //. eapply IHdecls => //.
+    + eapply IHdecls => //.
+    + constructor; auto.
+      eapply IHdecls => //.
+    + eapply IHdecls => //.
+Qed.
+
+From MetaCoq.Erasure Require Import EEtaExpandedFix.
+
+Lemma erase_brs_eq X_type X Γ p ts wt : 
+  erase_brs X_type X Γ p ts wt = 
+  map_All (fun br wt => (erase_context (bcontext br), erase X_type X _ (bbody br) wt)) ts wt.
+Proof.
+  funelim (map_All _ ts wt); cbn; auto.
+  f_equal => //. f_equal => //. apply erase_irrel.
+  rewrite -H. eapply erase_irrel.
+Qed.
+
+Lemma erase_fix_eq X_type X Γ ts wt : 
+  erase_fix X_type X Γ ts wt = map_All (fun d wt => 
+    let dbody' := erase X_type X _ (dbody d) (fun Σ abs => proj2 (wt Σ abs)) in
+    let dbody' := if isBox dbody' then
+        match d.(dbody) with
+        | tLambda na _ _ => E.tLambda (binder_name na) E.tBox
+        | _ => dbody'
+        end else dbody' 
+    in
+    {| E.dname := d.(dname).(binder_name); E.rarg := d.(rarg); E.dbody := dbody' |}) ts wt.
+Proof.
+  funelim (map_All _ ts wt); cbn; auto.
+  f_equal => //. f_equal => //.
+  rewrite (fst (erase_irrel _ _) _ _ _ (fun (Σ : global_env_ext) (abs : abstract_env_ext_rel X Σ) =>
+    (map_All_obligation_1 x xs h Σ abs).p2)).
+  destruct erase => //.
+  rewrite -H. eapply erase_irrel.
+Qed.
+
+Lemma erase_cofix_eq X_type X Γ ts wt : 
+  erase_cofix X_type X Γ ts wt = map_All (fun d wt => 
+    let dbody' := erase X_type X _ (dbody d) wt in
+    {| E.dname := d.(dname).(binder_name); E.rarg := d.(rarg); E.dbody := dbody' |}) ts wt.
+Proof.
+  funelim (map_All _ ts wt); cbn; auto.
+  f_equal => //. f_equal => //.
+  apply erase_irrel.
+  rewrite -H. eapply erase_irrel.
+Qed.
+
+Lemma isConstruct_erase X_type X Γ t wt : 
+  ~ (PCUICEtaExpand.isConstruct t || PCUICEtaExpand.isFix t || PCUICEtaExpand.isRel t) ->
+  ~ (isConstruct (erase X_type X Γ t wt) || isFix (erase X_type X Γ t wt) || isRel (erase X_type X Γ t wt)).
+Proof.
+  apply (erase_elim X_type X
+    (fun Γ t wt e => ~ (PCUICEtaExpand.isConstruct t || PCUICEtaExpand.isFix t || PCUICEtaExpand.isRel t) -> ~ (isConstruct e || isFix e || isRel e))
+    (fun Γ l awt e => True)
+    (fun Γ p l awt e => True)
+    (fun Γ l awt e => True)
+    (fun Γ l awt e => True)); intros => //. bang.
+Qed.
+
+Lemma apply_expanded Σ Γ Γ' t t' :
+  expanded Σ Γ t -> Γ = Γ' -> t = t' -> expanded Σ Γ' t'.
+Proof. intros; now subst. Qed.
+
+Lemma isLambda_inv t : isLambda t -> exists na ty bod, t = tLambda na ty bod.
+Proof. destruct t => //; eauto. Qed.
+
+Lemma erases_deps_erase (cf := config.extraction_checker_flags) 
+  {X_type X} univs 
+  (wfΣ : forall Σ, (abstract_env_rel X Σ) -> ∥ wf_ext (Σ, univs) ∥) decls prf
+  (X' :=  abstract_make_wf_env_ext X univs wfΣ) Γ t 
+  (wt : forall Σ : global_env_ext, abstract_env_ext_rel X' Σ -> welltyped Σ Γ t) :
+  let et := erase X_type.π2.π1 X' Γ t wt in
+  let deps := EAstUtils.term_global_deps et in
+  forall Σ, (abstract_env_rel X Σ) -> 
+  erases_deps Σ (erase_global_decls X_type deps X decls prf) et.
+Proof.
+  intros et deps Σ wf. 
+  pose proof (abstract_env_ext_exists X') as [[Σ' wfΣ']].
+  pose proof (wt _ wfΣ'). destruct H. pose proof (wfΣ _ wf) as [w].
+  rewrite (abstract_make_wf_env_ext_correct X univs wfΣ _ _ wf wfΣ') in X0.
+  eapply (erase_global_erases_deps w); tea.
+  eapply (erases_erase (X := X') (Γ := Γ)).
+  now rewrite <- (abstract_make_wf_env_ext_correct X univs wfΣ _ _ wf wfΣ').
+  eapply erase_global_includes.
+  intros. rewrite (abstract_env_irr _ H0 wf).
+  eapply term_global_deps_spec in H; eauto.
+  assumption.
+  eapply (erases_erase (X := X') (Γ := Γ)). 
+  now rewrite <- (abstract_make_wf_env_ext_correct X univs wfΣ _ _ wf wfΣ').
+  eapply KernameSet.subset_spec. reflexivity. 
+  now cbn.  
+Qed.
+
+Lemma erases_deps_erase_weaken (cf := config.extraction_checker_flags) 
+  {X_type X} univs 
+  (wfΣ : forall Σ, (abstract_env_rel X Σ) -> ∥ wf_ext (Σ, univs) ∥) decls prf
+  (X' :=  abstract_make_wf_env_ext X univs wfΣ) Γ t 
+  (wt : forall Σ : global_env_ext, abstract_env_ext_rel X' Σ -> welltyped Σ Γ t) 
+  deps :
+  let et := erase X_type.π2.π1 X'  Γ t wt in
+  let tdeps := EAstUtils.term_global_deps et in
+  forall Σ, (abstract_env_rel X Σ) -> 
+  erases_deps Σ (erase_global_decls X_type (KernameSet.union deps tdeps) X decls prf) et.
+Proof.
+  intros et tdeps Σ wf.
+  pose proof (abstract_env_ext_exists X') as [[Σ' wfΣ']].
+  pose proof (wt _ wfΣ'). destruct H. pose proof (wfΣ _ wf) as [w].
+  rewrite (abstract_make_wf_env_ext_correct X univs wfΣ _ _ wf wfΣ') in X0.
+  eapply (erase_global_erases_deps w); tea.
+  eapply (erases_erase (X := X') (Γ := Γ)).
+  now rewrite <- (abstract_make_wf_env_ext_correct X univs wfΣ _ _ wf wfΣ').
+  eapply erase_global_includes.
+  intros. rewrite (abstract_env_irr _ H0 wf).
+  eapply term_global_deps_spec in H; eauto.
+  assumption.
+  eapply (erases_erase (X := X') (Γ := Γ)).
+  now rewrite <- (abstract_make_wf_env_ext_correct X univs wfΣ _ _ wf wfΣ').
+  eapply KernameSet.subset_spec. intros x hin.
+  eapply KernameSet.union_spec. now right.
+  now cbn.
+Qed.
+
+Lemma eta_expand_erase {X_type X} Σ' {Γ t} 
+  (wt : forall Σ : global_env_ext, abstract_env_ext_rel X Σ -> welltyped Σ Γ t) Γ' :
+  forall Σ : global_env_ext, abstract_env_ext_rel X Σ -> 
+  PCUICEtaExpand.expanded Σ Γ' t ->
+  erases_global Σ Σ' ->
+  expanded Σ' Γ' (erase X_type X Γ t wt).
+Proof.
+  intros Σ wfΣ exp deps.
+  pose proof (abstract_env_ext_wf _ wfΣ) as [wf]. 
+  eapply expanded_erases. apply wf.
+  eapply erases_erase; eauto. assumption.
+  pose proof (wt _ wfΣ). destruct H as [T ht].
+  eapply erases_global_erases_deps; tea.
+  eapply erases_erase; eauto.
+Qed.
+
+Lemma erase_global_closed X_type X deps decls prf :
+  let X' := erase_global_decls X_type deps X decls prf in
+  EGlobalEnv.closed_env X'.
+Proof.
+  revert X prf deps.
+  induction decls; [cbn; auto|].
+  intros X prf deps. 
+  destruct a as [kn d].
+  destruct d as []; simpl; destruct KernameSet.mem;
+  set (Xpop := abstract_pop_decls X);
+  try set (Xmake :=  abstract_make_wf_env_ext Xpop (cst_universes c) _).
+  + cbn [EGlobalEnv.closed_env forallb]. cbn.
+    rewrite [forallb _ _](IHdecls) // andb_true_r.
+    rewrite /test_snd /EGlobalEnv.closed_decl /=.
+    destruct c as [ty [] univs]; cbn.
+    set (obl := erase_constant_body_obligation_1 _ _ _ _ _).
+    unfold erase_constant_body. cbn. clearbody obl. cbn in obl.
+    2:auto.
+    unshelve epose proof (erases_erase (X := Xmake) (obl eq_refl)); eauto.
+    pose proof (abstract_env_ext_exists Xmake) as [[Σmake wfmake]].
+    pose proof (abstract_env_ext_wf _ wfmake) as [[?]].
+    eapply erases_closed in H => //; eauto.
+    cbn. destruct (obl eq_refl _ wfmake). clear H. 
+    now eapply PCUICClosedTyp.subject_closed in X0.
+  + eapply IHdecls => //.
+  + cbn [EGlobalEnv.closed_env forallb].
+    rewrite {1}/test_snd {1}/EGlobalEnv.closed_decl /=.
+    eapply IHdecls => //.
+  + eapply IHdecls => //.
+  Unshelve. eauto.  
+Qed.
+
+Import EWellformed.
+
+Section wffix.
+  Import EAst.
+  Fixpoint wf_fixpoints (t : term) : bool :=
+    match t with
+    | tRel i => true
+    | tEvar ev args => List.forallb (wf_fixpoints) args
+    | tLambda N M => wf_fixpoints M
+    | tApp u v => wf_fixpoints u && wf_fixpoints v
+    | tLetIn na b b' => wf_fixpoints b && wf_fixpoints b'
+    | tCase ind c brs => 
+      let brs' := forallb (wf_fixpoints ∘ snd) brs in
+      wf_fixpoints c && brs'
+    | tProj p c => wf_fixpoints c
+    | tFix mfix idx => 
+      (idx <? #|mfix|) && List.forallb (fun d => (isLambda d.(dbody) || isBox d.(dbody)) && wf_fixpoints d.(dbody)) mfix
+    | tCoFix mfix idx =>
+      (idx <? #|mfix|) && List.forallb (wf_fixpoints ∘ dbody) mfix
+    | tConst kn => true
+    | tConstruct ind c => true
+    | tVar _ => true
+    | tBox => true
+    end.
+
+End wffix.
+
+Lemma erases_deps_wellformed (cf := config.extraction_checker_flags) (efl := all_env_flags) {Σ} {Σ'} et :
+  erases_deps Σ Σ' et ->
+  forall n, ELiftSubst.closedn n et ->
+  wf_fixpoints et ->
+  wellformed Σ' n et.
+Proof.
+  intros ed.
+  induction ed using erases_deps_forall_ind; intros => //; 
+   try solve [cbn in *; unfold wf_fix in *; rtoProp; intuition eauto; solve_all].
+  - cbn. red in H0. rewrite H0 //.
+  - cbn -[lookup_constructor].
+    cbn. now destruct H0 as [[-> ->] ->].
+  - cbn in *. move/andP: H5 => [] cld clbrs.
+    cbn. apply/andP; split. apply/andP; split. 
+    * now destruct H0 as [-> ->].
+    * now move/andP: H6.
+    * move/andP: H6; solve_all.
+  - cbn -[lookup_projection] in *. apply/andP; split; eauto.
+    now rewrite (declared_projection_lookup H0).
+Qed.
+
+Lemma erases_wf_fixpoints Σ Γ t t' : Σ;;; Γ |- t ⇝ℇ t' -> 
+  ErasureProperties.wellformed Σ t -> wf_fixpoints t'.
+Proof.
+  induction 1 using erases_forall_list_ind; cbn; auto; try solve [rtoProp; repeat solve_all].
+  - move/andP => []. rewrite (All2_length X) => -> /=. unfold test_def in *.
+    eapply Forall2_All2 in H.
+    eapply All2_All2_mix in X; tea. solve_all.
+    destruct b0; eapply erases_isLambda in H1; tea.
+  - move/andP => []. rewrite (All2_length X) => -> /=.
+    unfold test_def in *. solve_all.
+Qed.
+
+Lemma erase_wf_fixpoints (efl := all_env_flags) {X_type X} univs wfΣ {Γ t} wt
+  (X' :=  abstract_make_wf_env_ext X univs wfΣ) :
+  let t' := erase X_type.π2.π1 X' Γ t wt in
+  wf_fixpoints t'.
+Proof.
+  cbn. pose proof (abstract_env_ext_exists X') as [[Σ' wf']].
+  pose proof (abstract_env_exists X) as [[Σ wf]].
+  eapply erases_wf_fixpoints.
+  eapply erases_erase; eauto.
+  specialize (wt _ wf'). destruct (wfΣ _ wf).
+  unshelve eapply welltyped_wellformed in wt; eauto. 
+  now rewrite (abstract_make_wf_env_ext_correct X univs wfΣ _ _ wf wf'). 
+Qed.
+
+Lemma erase_wellformed (efl := all_env_flags) {X_type X} decls prf univs wfΣ {Γ t} wt
+(X' :=  abstract_make_wf_env_ext X univs wfΣ) :
+let t' := erase X_type.π2.π1 X' Γ t wt in
+wellformed (erase_global_decls X_type (term_global_deps t') X decls prf) #|Γ| t'.
+Proof.
+  set (t' := erase _ _ _ _ _). cbn.
+  epose proof (@erases_deps_erase X_type X univs wfΣ decls prf Γ t wt).
+  pose proof (abstract_env_exists X) as [[Σ wf]]. specialize_Σ wf. 
+  pose proof (abstract_env_ext_exists X') as [[Σ' wf']].
+  pose proof (abstract_env_ext_wf _ wf') as [[?]].
+  epose proof (erases_deps_wellformed _ H #|Γ|).
+  apply H0.
+  eapply (erases_closed _ Γ).
+  destruct (wt _ wf').
+  cbn in X. destruct (wfΣ _ wf).
+  eapply PCUICClosedTyp.subject_closed in X0. eassumption. 
+  eapply erases_erase; eauto. 
+  eapply erase_wf_fixpoints. Unshelve. eauto.  
+Qed.
+
+Lemma erase_wellformed_weaken (efl := all_env_flags) {X_type X} decls prf univs wfΣ {Γ t} wt
+(X' :=  abstract_make_wf_env_ext X univs wfΣ) deps:
+let t' := erase X_type.π2.π1 X' Γ t wt in
+  wellformed (erase_global_decls X_type (KernameSet.union deps (term_global_deps t')) X decls prf) #|Γ| t'.
+Proof.
+  set (t' := erase _ _ _ _ _). cbn.
+  epose proof (@erases_deps_erase_weaken _ X univs wfΣ decls prf Γ t wt deps).
+  pose proof (abstract_env_exists X) as [[Σ wf]]. specialize_Σ wf. 
+  pose proof (abstract_env_ext_exists X') as [[Σ' wf']].
+  pose proof (abstract_env_ext_wf _ wf') as [[?]].
+  epose proof (erases_deps_wellformed _ H #|Γ|).
+  apply H0.
+  eapply (erases_closed _ Γ).
+  - destruct (wt _ wf').
+    destruct (wfΣ _ wf).
+    eapply PCUICClosedTyp.subject_closed in X0. eassumption.
+  - eapply erases_erase; eauto. 
+  - eapply erase_wf_fixpoints.
+  Unshelve. eauto.  
+Qed.
+
+Lemma erase_constant_body_correct'' {X_type X} {cb} {decls prf} {univs wfΣ}
+(X' :=  abstract_make_wf_env_ext X univs wfΣ)
+{onc : forall Σ' : global_env_ext, abstract_env_ext_rel X' Σ' -> ∥ on_constant_decl (lift_typing typing) Σ' cb ∥} {body} deps :  
+  EAst.cst_body (fst (erase_constant_body X_type.π2.π1 X' cb onc)) = Some body ->
+  forall Σ' : global_env_ext, abstract_env_ext_rel X' Σ' -> 
+  ∥ ∑ t T, (Σ' ;;; [] |- t : T) * (Σ' ;;; [] |- t ⇝ℇ body) *
+      (term_global_deps body = snd (erase_constant_body X_type.π2.π1 X'  cb onc)) *
+      wellformed (efl:=all_env_flags) (erase_global_decls X_type (KernameSet.union deps (term_global_deps body)) X decls prf) 0 body ∥.
+Proof.
+  intros ? Σ' wfΣ'. pose proof (abstract_env_exists X) as [[Σ wf]]. 
+  destruct cb as [name [bod|] udecl]; simpl.
+  simpl in H. noconf H.
+  set (obl :=(erase_constant_body_obligation_1 (X_type.π2).π1 X'
+  {|
+  cst_type := name;
+  cst_body := Some bod;
+  cst_universes := udecl |} onc bod eq_refl)). clearbody obl.
+  destruct (obl _ wfΣ'). sq.
+  have er : (Σ, univs);;; [] |- bod ⇝ℇ erase X_type.π2.π1 X' [] bod obl.
+  { eapply (erases_erase (X:=X')). 
+    now rewrite <- (abstract_make_wf_env_ext_correct X univs wfΣ _ _ wf wfΣ'). 
+   }
+  exists bod, A; intuition auto.
+  now rewrite (abstract_make_wf_env_ext_correct X univs wfΣ _ _ wf wfΣ'). 
+  eapply erase_wellformed_weaken.
+  now simpl in H.
+Qed.
+
+Lemma erase_global_cst_decl_wf_glob X_type X deps decls heq :
+  forall cb wfΣ hcb,
+  let X' :=  abstract_make_wf_env_ext X (cst_universes cb) wfΣ in
+  let ecb := erase_constant_body X_type.π2.π1 X' cb hcb in
+  let Σ' := erase_global_decls X_type (KernameSet.union deps ecb.2) X decls heq in
+  (@wf_global_decl all_env_flags Σ' (EAst.ConstantDecl ecb.1) : Prop).
+Proof.
+  intros cb wfΣ hcb X' ecb Σ'. 
+  unfold wf_global_decl. cbn.
+  pose proof (abstract_env_exists X) as [[Σ wf]]. specialize_Σ wf. 
+  pose proof (abstract_env_ext_exists X') as [[Σmake wfmake]].
+  destruct (wfΣ _ wf), (hcb _ wfmake). red in X1.
+  destruct EAst.cst_body eqn:hb => /= //.
+  eapply (erase_constant_body_correct'') in hb; eauto. 
+  destruct hb as [[t0 [T [[] ?]]]]. rewrite e in i. exact i. 
+Qed.
+
+Lemma erase_global_ind_decl_wf_glob {X_type X} {deps decls kn m} heq :
+  (forall Σ : global_env, abstract_env_rel X Σ -> on_inductive (lift_typing typing) (Σ, ind_universes m) kn m) ->  let m' := erase_mutual_inductive_body m in
+  let Σ' := erase_global_decls X_type deps X decls heq in
+  @wf_global_decl all_env_flags Σ' (EAst.InductiveDecl m').
+Proof.
+  set (m' := erase_mutual_inductive_body m).
+  set (Σ' := erase_global_decls _ _ _ _ _). simpl.
+  intros oni.
+  pose proof (abstract_env_exists X) as [[Σ wf]]. specialize_Σ wf.
+  pose proof (abstract_env_wf _ wf) as [wfΣ].
+  assert (erases_mutual_inductive_body m (erase_mutual_inductive_body m)).
+  { eapply (erases_mutual (mdecl:=kn)); tea. }
+  eapply (erases_mutual_inductive_body_wf (univs := Σ.(universes)) (Σ := decls) (kn := kn) (Σ' := Σ')) in H; tea.
+  rewrite -(heq _ wf). now destruct Σ.
+Qed.
+
+Lemma erase_global_decls_wf_glob X_type X deps decls heq :
+  let Σ' := erase_global_decls X_type deps X decls heq in
+  @wf_glob all_env_flags Σ'.
+Proof.
+  cbn.
+  pose proof (abstract_env_exists X) as [[Σ wf]].
+  pose proof (abstract_env_wf _ wf) as [wfΣ].
+  revert deps X Σ wf wfΣ heq.
+  induction decls; [cbn; auto|].
+  { intros. constructor. }
+  intros. destruct a as [kn []]; simpl; destruct KernameSet.mem; set (Xpop := abstract_pop_decls X);
+  try set (Xmake :=  abstract_make_wf_env_ext Xpop (cst_universes c) _);
+  epose proof (abstract_env_exists Xpop) as [[Σpop wfpop]]; 
+  pose proof (abstract_env_wf _ wfpop) as [wfΣpop].
+  + constructor. eapply IHdecls => //; eauto. eapply erase_global_cst_decl_wf_glob; auto.
+    eapply erase_global_decls_fresh; auto.
+    destruct wfΣ. destruct wfΣpop.
+    rewrite (heq _ wf) in o0. now depelim o0.
+  + cbn. eapply IHdecls; eauto. 
+  + constructor. eapply IHdecls; eauto. 
+    destruct wfΣ as [[onu ond]]. 
+    rewrite (heq _ wf) in o. depelim o.
+    eapply (erase_global_ind_decl_wf_glob (kn:=kn)); tea.
+    intros. rewrite (abstract_env_irr _ H wfpop). 
+    unshelve epose proof (abstract_pop_decls_correct X decls _ _ _ wf wfpop) as [? ?].
+    {intros; now eexists. }
+    destruct Σpop, Σ; cbn in *. now subst.
+    eapply erase_global_decls_fresh.
+    destruct wfΣ as [[onu ond]].
+    rewrite (heq _ wf) in o. now depelim o.
+  + eapply IHdecls; eauto. 
+Qed.
+
+Lemma lookup_erase_global (cf := config.extraction_checker_flags) {X_type X} {deps deps' decls prf} :
+  KernameSet.Subset deps deps' ->
+  EExtends.global_subset (erase_global_decls X_type deps X decls prf) (erase_global_decls X_type deps' X decls prf).
+Proof.
+  revert deps deps' X prf.
+  induction decls. cbn => //.
+  intros ? ? ? ? sub. 
+  epose proof (abstract_env_exists X) as [[Σ wf]]. 
+  destruct a as [kn' []]; cbn;
+  ( set (decl := E.ConstantDecl _) || 
+    set (decl := E.InductiveDecl _)); hidebody decl;
+  set (eg := erase_global_decls _ _ _ _ _); hidebody eg;
+  set (eg' := erase_global_decls _ _ _ _ _); hidebody eg';
+  try (set (eg'' := erase_global_decls _ _ _ _ _); hidebody eg'');
+  try (set (eg''' := erase_global_decls _ _ _ _ _); hidebody eg''').
+  { destruct (KernameSet.mem) eqn:knm => /=.
+    + eapply KernameSet.mem_spec, sub, KernameSet.mem_spec in knm. rewrite knm.
+      apply EExtends.global_subset_cons. eapply IHdecls; eauto. 
+      intros x hin. eapply KernameSet.union_spec in hin.
+      eapply KernameSet.union_spec. destruct hin. left. now eapply sub.
+      right => //.
+    + destruct (KernameSet.mem kn' deps') eqn:eq'.
+      eapply EExtends.global_subset_cons_right; eauto. 
+      eapply erase_global_decls_wf_glob.
+      unfold decl. unfold hidebody.
+      constructor. eapply erase_global_decls_wf_glob.
+      eapply erase_global_cst_decl_wf_glob. 
+      eapply erase_global_decls_fresh => //.
+      pose proof (abstract_env_wf _ wf) as [wfΣ].
+      depelim wfΣ. rewrite (prf _ wf) in o0. clear - o0. now depelim o0.
+      unfold eg', eg'', hidebody. 
+      erewrite erase_global_decls_irr.
+      eapply IHdecls.
+      intros x hin.
+      eapply KernameSet.union_spec. left. now eapply sub.
+      eapply IHdecls => //. }
+  { destruct (KernameSet.mem) eqn:knm => /=.
+    + eapply KernameSet.mem_spec, sub, KernameSet.mem_spec in knm. rewrite knm.
+      apply EExtends.global_subset_cons. eapply IHdecls => //.
+    + destruct (KernameSet.mem kn' deps') eqn:eq'.
+      eapply EExtends.global_subset_cons_right. eapply erase_global_decls_wf_glob.
+      constructor. eapply erase_global_decls_wf_glob.
+      pose proof (abstract_env_wf _ wf) as [wfΣ].
+      pose proof (prf _ wf) as prf'.
+      eapply (erase_global_ind_decl_wf_glob (kn:=kn')).
+      intros. 
+      unshelve epose proof (abstract_pop_decls_correct X decls _ _ _ wf H) as [? ?].
+      { now eexists. }
+      destruct Σ, Σ0. cbn in *. rewrite prf' in wfΣ.
+      depelim wfΣ. cbn in *. rewrite <- H1, H0. 
+      now depelim o0.
+      eapply erase_global_decls_fresh => //.
+      pose proof (abstract_env_wf _ wf) as [wfΣ].
+      pose proof (prf _ wf) as prf'.
+      destruct Σ. cbn in *. rewrite prf' in wfΣ.
+      clear -wfΣ. destruct wfΣ. cbn in *. now depelim o0.
+      unfold eg'', hidebody. erewrite erase_global_decls_irr.
+      eapply IHdecls. intros x hin. now eapply sub.
+      eapply IHdecls => //. }
+Qed.
+
+Lemma expanded_weakening_global X_type X deps deps' decls prf Γ t : 
+  KernameSet.Subset deps deps' ->
+  expanded (erase_global_decls X_type deps X decls prf) Γ t ->
+  expanded (erase_global_decls X_type deps' X decls prf) Γ t.
+Proof.
+  intros hs.
+  eapply expanded_ind; intros; try solve [econstructor; eauto].
+  - eapply expanded_tFix; tea. solve_all.
+  - eapply expanded_tConstruct_app; tea.
+    destruct H. split; tea.
+    destruct d; split => //.
+    cbn in *. red in H.
+    eapply lookup_erase_global in H; tea.
+Qed.
+
+Lemma expanded_erase (cf := config.extraction_checker_flags) 
+  {X_type X decls prf} univs wfΣ t wtp :
+  forall Σ : global_env, abstract_env_rel X Σ -> PCUICEtaExpand.expanded Σ [] t ->
+  let X' :=  abstract_make_wf_env_ext X univs wfΣ in
+  let et := (erase X_type.π2.π1 X' [] t wtp) in
+  let deps := EAstUtils.term_global_deps et in
+  expanded (erase_global_decls X_type deps X decls prf) [] et.
+Proof.
+  intros Σ wf hexp X'.
+  pose proof (abstract_env_wf _ wf) as [wf'].
+  pose proof (abstract_env_ext_exists X') as [[? wfmake]].
+  eapply (expanded_erases (Σ := (Σ, univs))); tea.
+  eapply (erases_erase (X := X')); eauto.
+  now erewrite <- (abstract_make_wf_env_ext_correct X univs wfΣ).
+  cbn.
+  eapply (erases_deps_erase (X := X) univs wfΣ); eauto. 
+Qed.
+
+Lemma expanded_erase_global (cf := config.extraction_checker_flags) 
+  deps {X_type X decls prf} :
+  forall Σ : global_env, abstract_env_rel X Σ -> 
+    PCUICEtaExpand.expanded_global_env Σ ->
+    expanded_global_env (erase_global_decls X_type deps X decls prf).
+Proof.
+  intros Σ wf etaΣ. pose proof (prf _ wf).
+  destruct Σ as [univ decls']. 
+  red. revert wf. red in etaΣ. cbn in *. subst. 
+  revert deps X prf.
+  induction etaΣ; intros deps. intros. constructor. intros.
+  pose proof (abstract_env_exists (abstract_pop_decls X)) as [[Σpop wfpop]]. 
+  unshelve epose proof (abstract_pop_decls_correct X Σ _ _ _ wf wfpop) as [? ?].
+  { now eexists. }
+  destruct Σpop. cbn in H0, H1.  subst. 
+  destruct decl as [kn []];
+  destruct (KernameSet.mem kn deps) eqn:eqkn; simpl; rewrite eqkn.
+  constructor; [eapply IHetaΣ; auto|].
+  red. cbn. red. cbn in *.
+  set (deps' := KernameSet.union _ _). hidebody deps'.
+  set (wfext :=  abstract_make_wf_env_ext _ _ _). hidebody wfext.
+  destruct H.
+  destruct c as [cst_na [cst_body|] cst_type cst_rel].
+  cbn in *.
+  eapply expanded_weakening_global. 
+  2:{ eapply expanded_erase; tea. }
+  set (et := erase _ _ _ _) in *.
+  unfold deps'. unfold hidebody. intros x hin.    
+  eapply KernameSet.union_spec. right => //.
+  now cbn.
+  eapply IHetaΣ; eauto. 
+  constructor. eapply IHetaΣ; eauto. 
+  red. cbn => //.
+  eapply IHetaΣ; eauto. 
+Qed.
+
+(* Sanity checks: the [erase] function maximally erases terms *)
+Lemma erasable_tBox_value (wfl := Ee.default_wcbv_flags) (Σ : global_env_ext) (wfΣ : wf_ext Σ) t T v :
+  forall wt : Σ ;;; [] |- t : T,
+  Σ |-p t ▷ v -> erases Σ [] v E.tBox -> ∥ isErasable Σ [] t ∥.
+Proof.
+  intros.
+  depind H.
+  eapply Is_type_eval_inv; eauto. eexists; eauto.
+Qed.
+
+Lemma erase_eval_to_box (wfl := Ee.default_wcbv_flags) 
+  {X_type X} {univs wfext t v Σ' t' deps decls prf} :
+  let Xext :=  abstract_make_wf_env_ext X univs wfext in
+  forall wt : forall Σ : global_env_ext, abstract_env_ext_rel Xext Σ -> welltyped Σ [] t,
+  erase X_type.π2.π1 Xext [] t wt = t' ->
+  KernameSet.subset (term_global_deps t') deps ->
+  erase_global_decls X_type deps X decls prf = Σ' ->
+  forall Σext : global_env_ext, abstract_env_ext_rel Xext Σext -> 
+  (forall Σ : global_env, abstract_env_rel X Σ -> 
+    PCUICWcbvEval.eval Σ t v) ->
+    @Ee.eval Ee.default_wcbv_flags Σ' t' E.tBox -> ∥ isErasable Σext [] t ∥.
+Proof.
+  intros Xext wt.
+  intros.
+  destruct (erase_correct X_type X univs wfext _ _ Σ' _ _ decls prf wt H H0 H1 X0 _ H2) as [ev [eg [eg']]].
+  pose proof (Ee.eval_deterministic H3 eg'). subst.
+  pose proof (abstract_env_exists X) as [[? wf]].
+  destruct (wfext _ wf). destruct (wt _ H2) as [T wt'].
+  pose proof (abstract_env_ext_wf _ H2) as [?].
+  eapply erasable_tBox_value; eauto. 
+  pose proof (abstract_make_wf_env_ext_correct X univs wfext _ _ wf H2). subst. 
+  apply X0; eauto. 
+Qed.
+
+Lemma erase_eval_to_box_eager (wfl := Ee.default_wcbv_flags) 
+{X_type X} {univs wfext t v Σ' t' deps decls prf} :
+  let Xext :=  abstract_make_wf_env_ext X univs wfext in
+  forall wt : forall Σ : global_env_ext, abstract_env_ext_rel Xext Σ -> welltyped Σ [] t,
+  erase X_type.π2.π1 Xext [] t wt = t' ->
+  KernameSet.subset (term_global_deps t') deps ->
+  erase_global_decls X_type deps X decls prf = Σ' ->
+  forall Σext : global_env_ext, abstract_env_ext_rel Xext Σext -> 
+  (forall Σ : global_env, abstract_env_rel X Σ -> 
+    PCUICWcbvEval.eval Σ t v) ->
+  @Ee.eval Ee.default_wcbv_flags Σ' t' E.tBox -> t' = E.tBox.
+Proof.
+  intros Xext wt.
+  intros.
+  destruct (erase_eval_to_box wt H H0 H1 _ H2 X0 H3).
+  subst t'.
+  destruct (inspect_bool (is_erasableb X_type.π2.π1 Xext [] t wt)) eqn:heq.
+  - simp erase. rewrite heq.
+    simp erase => //.
+  - elimtype False.
+    pose proof (abstract_env_exists X) as [[? wf]].
+    destruct (@is_erasableP X_type.π2.π1 Xext [] t wt) => //. apply n. 
+    intros. sq. now rewrite (abstract_env_ext_irr _ H H2).  
+Qed.
+
+Section EraseGlobalFast.
+
+  Import PCUICEnvironment.
+
+Definition decls_prefix decls (Σ' : global_env) := 
+  ∑ Σ'', declarations Σ' = Σ'' ++ decls.
+
+Lemma on_global_decls_prefix {cf} P univs decls decls' :
+  on_global_decls P univs (decls ++ decls') ->
+  on_global_decls P univs decls'.
+Proof.
+  induction decls => //.
+  intros ha; depelim ha.
+  now apply IHdecls.
+Qed.
+
+Lemma decls_prefix_wf {decls Σ} : 
+  decls_prefix decls Σ -> wf Σ -> wf {| universes := Σ.(universes); declarations := decls |}.
+Proof.
+  intros [Σ' hd] wfΣ.
+  split. apply wfΣ.
+  cbn. destruct wfΣ as [_ ond]. rewrite hd in ond.
+  now eapply on_global_decls_prefix in ond.
+Qed.
+
+Lemma incl_cs_refl cs : cs ⊂_cs cs.
+Proof.
+  split; [lsets|csets].
+Qed.
+
+Lemma weaken_prefix {decls Σ kn decl} :
+  decls_prefix decls Σ ->
+  wf Σ -> 
+  lookup_env {| universes := Σ; declarations := decls |} kn = Some decl ->
+  on_global_decl (lift_typing typing) (Σ, universes_decl_of_decl decl) kn decl.
+Proof.
+  intros prefix wfΣ.
+  have wfdecls := decls_prefix_wf prefix wfΣ.
+  epose proof (weakening_env_lookup_on_global_env (lift_typing typing) _ Σ kn decl 
+    weaken_env_prop_typing wfdecls wfΣ).
+  forward X. red; split => //. cbn. apply incl_cs_refl.
+  now apply (X wfdecls).
+Qed.
+
+(* This version of global environment erasure keeps the same global environment throughout the whole 
+   erasure, while folding over the list of declarations. *)
+
+Program Fixpoint erase_global_decls_fast (deps : KernameSet.t) 
+  X_type (X:X_type.π1) (decls : global_declarations) 
+  (prop : forall Σ : global_env, abstract_env_rel X Σ -> ∥ decls_prefix decls Σ ∥) : E.global_declarations :=
+  match decls with
+  | [] => []
+  | (kn, ConstantDecl cb) :: decls =>
+    if KernameSet.mem kn deps then
+      let Xext' :=  abstract_make_wf_env_ext X (cst_universes cb) _ in
+      let cb' := erase_constant_body X_type.π2.π1 Xext' cb _ in
+      let deps := KernameSet.union deps (snd cb') in
+      let Σ' := erase_global_decls_fast deps X_type X decls _ in
+      ((kn, E.ConstantDecl (fst cb')) :: Σ')
+    else
+      erase_global_decls_fast deps X_type X decls _
+
+  | (kn, InductiveDecl mib) :: decls =>
+    if KernameSet.mem kn deps then
+      let mib' := erase_mutual_inductive_body mib in
+      let Σ' := erase_global_decls_fast deps X_type X decls _ in
+      ((kn, E.InductiveDecl mib') :: Σ')
+    else erase_global_decls_fast deps X_type X decls _
+  end.
+Next Obligation.
+  pose proof (abstract_env_wf _ H) as [?].
+  specialize_Σ H. sq. split. cbn. apply X3. cbn. 
+  eapply decls_prefix_wf in X3; tea.
+  destruct X3 as [onu ond]. cbn in ond.
+  now depelim ond.
+Qed.
+Next Obligation.
+  pose proof (abstract_env_ext_wf _ H) as [?].
+  pose proof (abstract_env_exists X) as [[? wf]].
+  pose proof (abstract_env_wf _ wf) as [?].
+  pose proof (prop' := prop _ wf).
+  sq. eapply (weaken_prefix (kn := kn)) in prop'; tea.
+  2:{ cbn. rewrite eqb_refl //. }
+  epose proof (abstract_make_wf_env_ext_correct X (cst_universes cb) _ _ _ wf H). subst. 
+  apply prop'.
+Qed.
+Next Obligation.
+  specialize_Σ H. sq; red. destruct prop as [Σ' ->].
+  eexists (Σ' ++ [(kn, ConstantDecl cb)]); rewrite -app_assoc //.
+Qed.
+Next Obligation.
+  specialize_Σ H. sq; red. destruct prop as [Σ' ->].
+  eexists (Σ' ++ [(kn, ConstantDecl cb)]); rewrite -app_assoc //.
+Qed.
+Next Obligation.
+  specialize_Σ H. sq; red. destruct prop as [Σ' ->].
+  eexists (Σ' ++ [(kn, _)]); rewrite -app_assoc //.
+Qed.
+Next Obligation.
+  specialize_Σ H. sq; red. destruct prop as [Σ' ->].
+  eexists (Σ' ++ [(kn, _)]); rewrite -app_assoc //.
+Qed.
+
+Import PCUICAst PCUICEnvironment.
+
+Lemma wf_lookup Σ kn d suffix g : 
+  wf Σ ->
+  declarations Σ = suffix ++ (kn, d) :: g ->
+  lookup_env Σ kn = Some d.
+Proof.
+  unfold lookup_env.
+  intros [_ ond] eq. rewrite eq in ond |- *.
+  move: ond; clear.
+  induction suffix.
+  - cbn. rewrite eqb_refl //.
+  - cbn. intros ond.
+    depelim ond. cbn. red in f.
+    eapply Forall_app in f as []. depelim H0. cbn in H0.
+    destruct (eqb_spec kn kn0); [contradiction|].
+    now apply IHsuffix.
+Qed.
+
+Definition add_suffix suffix Σ :=
+  {| universes := Σ.(universes); declarations := suffix ++ Σ.(declarations) |}.
+
+Lemma eta_global_env Σ : Σ = {| universes := Σ.(universes); declarations := Σ.(declarations) |}.
+Proof. now destruct Σ. Qed.
+  
+Lemma add_suffix_cons d suffix Σ : add_suffix (d :: suffix) Σ = add_global_decl (add_suffix suffix Σ) d. 
+Proof. reflexivity. Qed.
+
+Lemma global_erased_with_deps_weaken_prefix suffix Σ Σ' kn : 
+  wf (add_suffix suffix Σ) ->
+  global_erased_with_deps Σ Σ' kn ->
+  global_erased_with_deps (add_suffix suffix Σ) Σ' kn.
+Proof.
+  induction suffix.
+  - unfold add_suffix; cbn. intros wf hg.
+    now rewrite -eta_global_env.
+  - rewrite add_suffix_cons. intros wf H.
+    destruct a as [kn' d]. eapply global_erases_with_deps_weaken => //.
+    apply IHsuffix => //.
+    destruct wf as [onu ond]. now depelim ond.
+Qed.
+
+
+(* Using weakening it is trivial to show that a term found to be erasable in Σ 
+  will be found erasable in any well-formed extension. The converse is not so trivial:
+  some valid types in the extension are not valid in the restricted global context.
+  So, we will rather show that the erasure function is invariant under extension. *) 
+
+Lemma isErasable_irrel_global_env {Σ Σ' : global_env_ext} {Γ t} :
+  wf Σ ->
+  extends_decls Σ' Σ ->
+  Σ.2 = Σ'.2 ->
+  isErasable Σ' Γ t -> isErasable Σ Γ t.
+Proof.
+  unfold isErasable.
+  intros wfΣ ext eqext [T [ht isar]].
+  destruct Σ as [Σ decl], Σ' as [Σ' decl']. cbn in eqext; subst decl'.
+  exists T; split.
+  eapply (env_prop_typing weakening_env (Σ', decl)) => //=.
+  eapply extends_decls_wf; tea.
+  now eapply extends_decls_extends.
+  destruct isar as [|s]; [left|right] => //.
+  destruct s as [u [Hu isp]].
+  exists u; split => //.
+  eapply (env_prop_typing weakening_env (Σ', decl)) => //=.
+  eapply extends_decls_wf; tea.
+  now eapply extends_decls_extends.
+Qed. 
+
+
+  
+
 
 (*Lemma erase_global_deps_suffix {deps} {Σ Σ' : wf_env} {decls hprefix hprefix'} :
   wf Σ -> wf Σ' ->
@@ -3048,8 +3178,8 @@ Proof.
   set (eb' := erase_constant_body _ _ _).
   assert (eb = eb') as <-.
   { subst eb eb'.
-    set (wfΣx := make_wf_env_ext _ _ _).
-    set (wfΣ'x := make_wf_env_ext _ _ _).
+    set (wfΣx :=  abstract_make_wf_env_ext _ _ _).
+    set (wfΣ'x :=  abstract_make_wf_env_ext _ _ _).
     set (obl' := erase_global_decls_fast_obligation_2 _ _ _ _ _ _ _).
     clearbody obl'.
     set (Σd := {| universes := Σ.(universes); declarations := decls |}).
@@ -3061,7 +3191,7 @@ Proof.
     set (wfΣdwfe := build_wf_env_from_env _ (sq wfΣd)).
     assert (wfextΣd : wf_ext (Σd, cst_universes c)).
     { split => //. cbn. apply w. }
-    set (wfΣdw := make_wf_env_ext wfΣdwfe (cst_universes c) (sq wfextΣd)).
+    set (wfΣdw :=  abstract_make_wf_env_ext wfΣdwfe (cst_universes c) (sq wfextΣd)).
     assert (ond' : ∥ on_constant_decl (lift_typing typing) (Σd, cst_universes c) c ∥ ).
     { pose proof (decls_prefix_wf hprefix wfΣ).
       destruct X as [onu ond]. depelim ond. sq. apply o0. }
@@ -3081,89 +3211,107 @@ Proof.
   eapply IHdecls.
 Qed.*)
   
-Lemma erase_global_deps_fast_spec_gen {deps} {Σ Σ' : wf_env} {decls hprefix hprefix'} :
-  universes Σ = universes Σ' -> 
-  erase_global_decls_fast deps Σ decls hprefix = 
-  erase_global_decls deps Σ' decls hprefix'.
+Lemma erase_global_deps_fast_spec_gen {deps} 
+  {X_type X X'} {decls hprefix hprefix'} :
+  (forall Σ Σ', abstract_env_rel X Σ -> abstract_env_rel X' Σ' -> universes Σ = universes Σ') -> 
+  erase_global_decls_fast deps X_type X decls hprefix = 
+  erase_global_decls X_type deps X' decls hprefix'.
 Proof.
-  assert (wf : ∥ wf Σ ∥) by exact (referenced_impl_wf Σ).
-  destruct wf as [wf].
   intros equ.
-  induction decls in Σ', equ, deps, hprefix, hprefix' |- * => //.
+  induction decls in X, X', equ, deps, hprefix, hprefix' |- * => //.
+  pose proof (abstract_env_exists X) as [[Σ wfΣ]].  
+  pose proof (abstract_env_exists X') as [[Σ' wfΣ']].
+  pose proof (abstract_env_wf _ wfΣ) as [wf]. 
+  pose proof (abstract_env_exists (abstract_pop_decls X')) as [[? wfpop]].
+  unshelve epose proof (abstract_pop_decls_correct X' decls _ _ _ wfΣ' wfpop) as [? ?].
+  { now eexists. }
+
   destruct a as [kn []].
-  - set (obl := (erase_global_decls_fast_obligation_1 Σ ((kn, ConstantDecl c) :: decls)
-             hprefix kn c decls eq_refl)). clearbody obl.
-    destruct obl.
-    cbn.
-    set (eb := erase_constant_body _ _ _).
-    set (eb' := erase_constant_body _ _ _).
+  - cbn. 
+    set (obl := (erase_global_decls_fast_obligation_1 X_type X ((kn, ConstantDecl c) :: decls)
+             hprefix kn c decls eq_refl)).
+    set (eb := erase_constant_body _ _ _ _).
+    set (eb' := erase_constant_body _ _ _ _).
     assert (eb = eb') as <-.
     { subst eb eb'.
-      destruct hprefix as [[Σ'' eq]].
+      destruct (hprefix _ wfΣ) as [[Σ'' eq]].
       eapply erase_constant_body_suffix; cbn => //.
-      red. split => //. cbn.
-      rewrite eq.
-      eexists (Σ'' ++ [(kn, ConstantDecl c)]). now rewrite -app_assoc. }
-    destruct KernameSet.mem => //; f_equal; eauto.
-  - cbn.
-    destruct KernameSet.mem => //; f_equal; eauto.
+      intros.
+      epose proof (abstract_make_wf_env_ext_correct X (cst_universes c) _ _ _ wfΣ H1).
+      epose proof (abstract_make_wf_env_ext_correct (abstract_pop_decls X') (cst_universes c) _ _ _ wfpop H2).
+      subst. split => //. 
+      sq; red. cbn. 
+      rewrite eq. rewrite <- H0. split. symmetry. apply equ; eauto.
+      eexists (Σ'' ++ [(kn, ConstantDecl c)]). subst. now rewrite -app_assoc. }
+    destruct KernameSet.mem => //; f_equal; eapply IHdecls.
+    intros. unshelve epose proof (abstract_pop_decls_correct X' decls _ _ _ wfΣ' H2) as [? ?].
+    { now eexists. } rewrite <- H4. apply equ; eauto.
+    intros. unshelve epose proof (abstract_pop_decls_correct X' decls _ _ _ wfΣ' H2) as [? ?].
+    { now eexists. } rewrite <- H4. apply equ; eauto.
+  
+    - cbn.
+    destruct KernameSet.mem => //; f_equal; eapply IHdecls.
+    intros. unshelve epose proof (abstract_pop_decls_correct X' decls _ _ _ wfΣ' H2) as [? ?].
+    { now eexists. } rewrite <- H4. apply equ; eauto.
+    intros. unshelve epose proof (abstract_pop_decls_correct X' decls _ _ _ wfΣ' H2) as [? ?].
+    { now eexists. } rewrite <- H4. apply equ; eauto.
 Qed.
 
-Lemma erase_global_deps_fast_spec {deps} {Σ : wf_env} {decls hprefix hprefix'} :
-  erase_global_decls_fast deps Σ decls hprefix = 
-  erase_global_decls deps Σ decls hprefix'.
+Lemma erase_global_deps_fast_spec {deps} {X_type X} {decls hprefix hprefix'} :
+  erase_global_decls_fast deps X_type X decls hprefix = 
+  erase_global_decls X_type deps X decls hprefix'.
 Proof.
-  eapply erase_global_deps_fast_spec_gen; auto.
+  eapply erase_global_deps_fast_spec_gen; intros.
+  rewrite (abstract_env_irr _ H H0); eauto.  
 Qed.
 
-Definition erase_global_fast deps Σ :=
-  erase_global_decls_fast deps Σ Σ.(declarations) (sq ([]; eq_refl)).
+Definition erase_global_fast X_type deps X decls (prf:forall Σ : global_env, abstract_env_rel X Σ -> declarations Σ = decls) :=
+  erase_global_decls_fast deps X_type X decls (fun _ H => sq ([] ; prf _ H)).
 
-Lemma erase_global_fast_spec {deps} {Σ : wf_env} :
-  erase_global_fast deps Σ = 
-  erase_global deps Σ.
-Proof.
-  rewrite /erase_global_fast erase_global_deps_fast_spec //.
-Qed.
-
-Lemma expanded_erase_global_fast (cf := config.extraction_checker_flags) deps {Σ: wf_env} :
+Lemma expanded_erase_global_fast (cf := config.extraction_checker_flags) deps 
+  {X_type X decls prf} :
+  forall Σ : global_env, abstract_env_rel X Σ -> 
   PCUICEtaExpand.expanded_global_env Σ ->
-  expanded_global_env (erase_global_fast deps Σ).
+  expanded_global_env (erase_global_fast X_type deps X decls prf).
 Proof.
-  rewrite erase_global_fast_spec.
+  unfold erase_global_fast.
+  rewrite erase_global_deps_fast_spec. 
   eapply expanded_erase_global.
 Qed.
 
-Lemma expanded_erase_fast (cf := config.extraction_checker_flags) {Σ : wf_env} univs wfΣ t wtp :
+Lemma expanded_erase_fast (cf := config.extraction_checker_flags) 
+  {X_type X decls prf} univs wfΣ t wtp :
+  forall Σ : global_env, abstract_env_rel X Σ -> 
   PCUICEtaExpand.expanded Σ [] t ->
-  let Σ' := make_wf_env_ext Σ univs wfΣ in
-  let et := (erase Σ' [] t wtp) in
+  let X' :=  abstract_make_wf_env_ext X univs wfΣ in
+  let et := (erase X_type.π2.π1 X' [] t wtp) in
   let deps := EAstUtils.term_global_deps et in
-  expanded (erase_global_fast deps Σ) [] et.
+  expanded (erase_global_fast X_type deps X decls prf) [] et.
 Proof.
-  intros hexp Σ'.
-  have [wf] : ∥ wf Σ ∥.
-  { destruct wfΣ. sq. exact w. }
+  intros Σ wf hexp X'. pose proof (abstract_env_wf _ wf) as [?].
   eapply (expanded_erases (Σ := (Σ, univs))); tea.
-  eapply (erases_erase (Σ := Σ')). cbn.
-  rewrite erase_global_fast_spec //.
-  eapply (erases_deps_erase (Σ := Σ) univs wfΣ).
+  eapply (erases_erase (X := X')). 
+  pose proof (abstract_env_ext_exists X') as [[? wfmake]].
+  now rewrite <- (abstract_make_wf_env_ext_correct X univs _ _ _ wf wfmake).
+  cbn. unfold erase_global_fast. rewrite erase_global_deps_fast_spec //.
+  eapply (erases_deps_erase (X := X) univs wfΣ); eauto. 
 Qed.
 
-Lemma erase_global_fast_wf_glob Σ deps :
-  @wf_glob all_env_flags (erase_global_fast deps Σ).
+Lemma erase_global_fast_wf_glob X_type X deps decls prf :
+  @wf_glob all_env_flags (erase_global_fast X_type X deps decls prf).
 Proof.
-  rewrite erase_global_fast_spec.
-  eapply erase_global_wf_glob.
+  unfold erase_global_fast; rewrite erase_global_deps_fast_spec.
+  eapply erase_global_decls_wf_glob.
 Qed.
 
-Lemma erase_wellformed_fast (efl := all_env_flags) {Σ : wf_env} univs wfΣ {Γ t} wt
-  (Σ' := make_wf_env_ext Σ univs wfΣ) :
-  let t' := erase Σ' Γ t wt in
-  wellformed (erase_global_fast (term_global_deps t') Σ) #|Γ| t'.
+Lemma erase_wellformed_fast (efl := all_env_flags) 
+  {X_type X decls prf} univs wfΣ {Γ t} wt
+  (X' :=  abstract_make_wf_env_ext X univs wfΣ) :
+  let t' := erase X_type.π2.π1 X' Γ t wt in
+  wellformed (erase_global_fast X_type (term_global_deps t') X decls prf) #|Γ| t'.
 Proof.
   intros. 
-  cbn. rewrite erase_global_fast_spec.
+  cbn. unfold erase_global_fast. rewrite erase_global_deps_fast_spec.
   eapply erase_wellformed.
 Qed.
 
