examples/typing_correctness.v
@@ -31,6 +31,10 @@ Definition gctx : global_env_ext :=
 Definition kername_of_string (s : string) : kername :=
   (MPfile [], s).
 
+Global Program Instance fake_guard_impl : abstract_guard_impl :=
+{| guard_impl := fake_guard_impl |}.
+Next Obligation. Admitted.  
+
 Definition make_wf_env_ext (Σ : global_env_ext) : EnvCheck wf_env_ext wf_env_ext :=
   '(exist Σ' pf) <- check_wf_ext optimized_abstract_env_impl Σ ;;
   ret Σ'.
